@base <https://bigg-project.eu/ontology#> .
@prefix bigg: <http://bigg-project.eu/ontology#> .
@prefix skos: <http://www.w3.org/2004/02/skos/core#> .
@prefix rdfs: <http://www.w3.org/2000/01/rdf-schema#> .
@prefix rdf: <http://www.w3.org/1999/02/22-rdf-syntax-ns#> .


bigg:GrossFloorArea a bigg:AreaType, skos:Concept;
  rdfs:comment "Sum of the floor areas of all building spaces measured from the external faces of the exterior walls" .

bigg:GrossFloorAreaAboveGround a bigg:AreaType, skos:Concept;
  rdfs:comment "Part of the gross floor area above ground" .

bigg:GrossFloorAreaUnderGround a bigg:AreaType, skos:Concept;
  rdfs:comment "Part of the gross floor area below ground" .

bigg:NetFloorArea a bigg:AreaType, skos:Concept;
  rdfs:comment "Gross floor area, excluding the area occupied by walls and partitions, the circulation area (where people walk), and the mechanical area (where there is mechanical equipment), i.e., gross floor area reduced by the area for structural components" .

bigg:CooledFloorArea a bigg:AreaType, skos:Concept;
  rdfs:comment "Part of the net floor area that is cooled or air conditioned" .

bigg:HeatedFloorArea a bigg:AreaType, skos:Concept;
  rdfs:comment "Part of the net floor area that is heated" .

bigg:CadastralParcelArea a bigg:AreaType, skos:Concept;
  rdfs:comment "The area of the cadastral parcel over which the building is constriucted" .

bigg:HeatingDegreeDays a bigg:BaselineInfluenceFactor, skos:Concept .

bigg:CoolingDegreeDays a bigg:BaselineInfluenceFactor, skos:Concept .

bigg:Occupancy a bigg:BaselineInfluenceFactor, skos:Concept .

bigg:ProductionLevel a bigg:BaselineInfluenceFactor, skos:Concept .

bigg:owned a bigg:BuildingOwnership, skos:Concept .

bigg:rented a bigg:BuildingOwnership, skos:Concept .

bigg:IfcWall a bigg:BuildingConstructionElementType, skos:Concept;
  rdfs:comment "A vertical construction in a premises that creates an enclosed building space" .

bigg:IfcWall.ExternalWall a bigg:BuildingConstructionElementType, skos:Concept;
  rdfs:comment "Outer walls of a building including the ones adjoining to another building and the ones abutting on an interior open space";
  skos:broader bigg:IfcWall .

bigg:IfcWall.ExternalWall.IfcCurtainWall a bigg:BuildingConstructionElementType, skos:Concept;
  rdfs:comment "Outer covering of a building in which the outer walls are non-structural, utilized only to keep the weather out and the occupants in";
  skos:broader bigg:IfcWall.ExternalWall .

bigg:IfcWall.InternalWall a bigg:BuildingConstructionElementType, skos:Concept;
  rdfs:comment "Walls providing separation between the internal spaces of a building";
  skos:broader bigg:IfcWall .

bigg:RoofOrCeiling a bigg:BuildingConstructionElementType, skos:Concept;
  rdfs:comment "The exterior (roof) or internal (ceiling) structure forming the upper covering of the building" .

bigg:RoofOrCeiling.PitchedRoof a bigg:BuildingConstructionElementType, skos:Concept;
  rdfs:comment "A roof that is formed by surfaces sloping downward with an angle of more than 20°";
  skos:broader bigg:RoofOrCeiling .

bigg:RoofOrCeiling.FlatRoof a bigg:BuildingConstructionElementType, skos:Concept;
  rdfs:comment "A roof that is flat or formed by surfaces sloping downward with an angle of less than 20°";
  skos:broader bigg:RoofOrCeiling .

bigg:RoofOrCeiling.ReflectiveRoof a bigg:BuildingConstructionElementType, skos:Concept;
  rdfs:comment "A reflective or cool roof is a roof coated with a high solar reflectance material that reflects sunlight and reduces the temperature and heat gain of the struture";
  skos:broader bigg:RoofOrCeiling .

bigg:RoofOrCeiling.GreenRoof a bigg:BuildingConstructionElementType, skos:Concept;
  rdfs:comment "A roof that is partially or completely covered with vegetation and a growing medium, planted over a waterproofing membrane";
  skos:broader bigg:RoofOrCeiling .

bigg:RoofOrCeiling.LoftCeiling a bigg:BuildingConstructionElementType, skos:Concept;
  rdfs:comment "The covering ceiling of the space located inside the sloping roof of a building";
  skos:broader bigg:RoofOrCeiling .

bigg:Floor a bigg:BuildingConstructionElementType, skos:Concept;
  rdfs:comment "A horizontal construction in a building that creates the base of an enclosed space" .

bigg:Floor.SuspendedFloor a bigg:BuildingConstructionElementType, skos:Concept;
  rdfs:comment "A ground floor with a void underneath the structure";
  skos:broader bigg:Floor .

bigg:Floor.SolidFloor a bigg:BuildingConstructionElementType, skos:Concept;
  rdfs:comment "A floor that consists of a layer of concrete";
  skos:broader bigg:Floor .

bigg:IfcSlab a bigg:BuildingConstructionElementType, skos:Concept;
  rdfs:comment "Provides the lower support (floor) or upper construction (roof slab) in any space in a building." .

bigg:IfcWindow a bigg:BuildingConstructionElementType, skos:Concept;
  rdfs:comment "An opening in the wall of a building fitted with glass in a frame" .

bigg:Skylight a bigg:BuildingConstructionElementType, skos:Concept;
  rdfs:comment "A window fitted in the roof or ceiling of a building, typically inclined or horizontal" .

bigg:IfcDoor a bigg:BuildingConstructionElementType, skos:Concept;
  rdfs:comment "A surface component that is operable and separates two spaces in a building" .

bigg:IfcDoor.AutomaticDoor a bigg:BuildingConstructionElementType, skos:Concept;
  rdfs:comment "A door equipped with a power-operated mechanism and controls that open and close the door automatically";
  skos:broader bigg:IfcDoor .

bigg:ShadingSystem a bigg:BuildingConstructionElementType, skos:Concept;
  rdfs:comment "A system that can be added inside or outside of a fenestration system to block or redirects some amount of the solar radiation coming through the fenestration system" .

bigg:OtherBuildingConstructionElement a bigg:BuildingConstructionElementType, skos:Concept;
  rdfs:comment "Other building construction element" .

bigg:Office a bigg:BuildingSpaceUseType, skos:Concept;
  rdfs:comment "Public or private structure where administrative work is performed" .

bigg:Office.PublicOffice a bigg:BuildingSpaceUseType, skos:Concept;
  rdfs:comment "Publicly owned structure where administrative work is performed";
  skos:broader bigg:Office .

bigg:Office.PrivateOffice a bigg:BuildingSpaceUseType, skos:Concept;
  rdfs:comment "Privetely owned structure where administrative work is performed";
  skos:broader bigg:Office .

bigg:Retail a bigg:BuildingSpaceUseType, skos:Concept;
  rdfs:comment "Wholesale and retail trade buildings" .

bigg:Retail.ShoppingMall a bigg:BuildingSpaceUseType, skos:Concept;
  rdfs:comment "Premises comprised of small to large retailers, restaurants, and entertainment establishments located indoor or outdoor";
  skos:broader bigg:Retail .

bigg:Retail.Supermarket a bigg:BuildingSpaceUseType, skos:Concept;
  rdfs:comment "Retailer supplying a wide range of products including groceries";
  skos:broader bigg:Retail .

bigg:Retail.Market a bigg:BuildingSpaceUseType, skos:Concept;
  rdfs:comment "Building for the gathering of people for the purchase and sale of provisions, livestock, and other commodities";
  skos:broader bigg:Retail .

bigg:Retail.CommercialActivity a bigg:BuildingSpaceUseType, skos:Concept;
  rdfs:comment "Premises for the retail of merchandise such as furniture , electronics and appliance, food and beverage, health and personal care , clothing, books and music, and office supplies, stationery and gift stores. Malls or shopping centers are excluded.";
  skos:broader bigg:Retail .

bigg:Retail.ExhibitionCenter a bigg:BuildingSpaceUseType, skos:Concept;
  rdfs:comment "Large building where major trade fairs are held";
  skos:broader bigg:Retail .

bigg:Retail.OtherRetail a bigg:BuildingSpaceUseType, skos:Concept;
  rdfs:comment "Other wholesale and retail buildings";
  skos:broader bigg:Retail .

bigg:Hospitality a bigg:BuildingSpaceUseType, skos:Concept;
  rdfs:comment "Building used to offer services including lodging, food and drink service, event planning, theme parks, and transportation. It includes hotels, restaurants and bars" .

bigg:Hospitality.CafeOrBar a bigg:BuildingSpaceUseType, skos:Concept;
  rdfs:comment "Premise where light food, alcoholic drinks or refreshments are served";
  skos:broader bigg:Hospitality .

bigg:Hospitality.Canteen a bigg:BuildingSpaceUseType, skos:Concept;
  rdfs:comment "Restaurant provided by an organization such as a college, factory, or company for its students or staff";
  skos:broader bigg:Hospitality .

bigg:Hospitality.Restaurant a bigg:BuildingSpaceUseType, skos:Concept;
  rdfs:comment "Premises for preparation and food service which includes waiting services";
  skos:broader bigg:Hospitality .

bigg:Hospitality.Hostel a bigg:BuildingSpaceUseType, skos:Concept;
  rdfs:comment "Lodging with limited amenities for a specific group of people, such as students, workers, or travellers";
  skos:broader bigg:Hospitality .

bigg:Hospitality.Guesthouse a bigg:BuildingSpaceUseType, skos:Concept;
  rdfs:comment "Small, privately owned homesteay that offers lodging";
  skos:broader bigg:Hospitality .

bigg:Hospitality.Hotel a bigg:BuildingSpaceUseType, skos:Concept;
  rdfs:comment "Lodging with extended amenities that includes resorts";
  skos:broader bigg:Hospitality .

bigg:Hospitality.OtherHospitality a bigg:BuildingSpaceUseType, skos:Concept;
  rdfs:comment "Building used to offer other hospitality services";
  skos:broader bigg:Hospitality .

bigg:RecreationAndCulture a bigg:BuildingSpaceUseType, skos:Concept;
  rdfs:comment "Cultural, entertainment, or recreational facilities" .

bigg:RecreationAndCulture.Cinema a bigg:BuildingSpaceUseType, skos:Concept;
  rdfs:comment "Building where films are shown for public entertainment";
  skos:broader bigg:RecreationAndCulture .

bigg:RecreationAndCulture.Theatre a bigg:BuildingSpaceUseType, skos:Concept;
  rdfs:comment "Building in which plays and other dramatic performances are given";
  skos:broader bigg:RecreationAndCulture .

bigg:RecreationAndCulture.Museum a bigg:BuildingSpaceUseType, skos:Concept;
  rdfs:comment "Building in which objects of historical, scientific, artistic, or cultural interest are stored and exhibited";
  skos:broader bigg:RecreationAndCulture .

bigg:RecreationAndCulture.CulturalOrSocialCenter a bigg:BuildingSpaceUseType, skos:Concept;
  rdfs:comment "Building or complex used to promotes culture and arts or to offer community services";
  skos:broader bigg:RecreationAndCulture .

bigg:RecreationAndCulture.Library a bigg:BuildingSpaceUseType, skos:Concept;
  rdfs:comment "Premises containing collections of books and periodicals for use or borrowing by the public or the members of an institution";
  skos:broader bigg:RecreationAndCulture .

bigg:RecreationAndCulture.ReligiousFacilities a bigg:BuildingSpaceUseType, skos:Concept;
  rdfs:comment "Religious public assembly premises including churches, monasteries, synagogues, mosques, and temples";
  skos:broader bigg:RecreationAndCulture .

bigg:RecreationAndCulture.OtherReacreationAndCulture a bigg:BuildingSpaceUseType,
    skos:Concept;
  rdfs:comment "Other facilities related to cultural, entertainment, or recreational activities";
  skos:broader bigg:RecreationAndCulture .

bigg:Healthcare a bigg:BuildingSpaceUseType, skos:Concept;
  rdfs:comment "Premises that host health care services for the maintenance and improvement of physical and mental health" .

bigg:Healthcare.PrimaryCareCenterOrClinic a bigg:BuildingSpaceUseType, skos:Concept;
  rdfs:comment "Premises to receive people making an initial approach to a medical practitioner or clinic for advice or treatment";
  skos:broader bigg:Healthcare .

bigg:Healthcare.DayCareHospital a bigg:BuildingSpaceUseType, skos:Concept;
  rdfs:comment "Premises that include urgent care centers and outpatient clinics";
  skos:broader bigg:Healthcare .

bigg:Healthcare.Hospital a bigg:BuildingSpaceUseType, skos:Concept;
  rdfs:comment "Premises that provide temporary to long-term inpatient services";
  skos:broader bigg:Healthcare .

bigg:Healthcare.NursingHome a bigg:BuildingSpaceUseType, skos:Concept;
  rdfs:comment "Facility for special care needs including senior care community and nursing homes for people with disabilities";
  skos:broader bigg:Healthcare .

bigg:Healthcare.HomelessShelter a bigg:BuildingSpaceUseType, skos:Concept;
  rdfs:comment "Temporary residence for homeless individuals and families";
  skos:broader bigg:Healthcare .

bigg:Healthcare.VeterinaryClinic a bigg:BuildingSpaceUseType, skos:Concept;
  rdfs:comment "Premises that provide services for the prevention, diagnosis, treatment, and health care of animal populations";
  skos:broader bigg:Healthcare .

bigg:Healthcare.Mortuary a bigg:BuildingSpaceUseType, skos:Concept;
  rdfs:comment "Premises that are used for the storage of human corpses awaiting identification, or removal for autopsy or disposal by burial, cremation or otherwise";
  skos:broader bigg:Healthcare .

bigg:Healthcare.OtherHealthcare a bigg:BuildingSpaceUseType, skos:Concept;
  rdfs:comment "Buildings dedicated to other health care services ";
  skos:broader bigg:Healthcare .

bigg:EducationAndResearch a bigg:BuildingSpaceUseType, skos:Concept;
  rdfs:comment "Facilities used for educational purposes and research" .

bigg:EducationAndResearch.Preschool a bigg:BuildingSpaceUseType, skos:Concept;
  rdfs:comment "Preschool education premises including kindergartens and daycare centers";
  skos:broader bigg:EducationAndResearch .

bigg:EducationAndResearch.PrimarySchool a bigg:BuildingSpaceUseType, skos:Concept;
  rdfs:comment "Education premises including primary schools and elementary schools";
  skos:broader bigg:EducationAndResearch .

bigg:EducationAndResearch.SecondarySchool a bigg:BuildingSpaceUseType, skos:Concept;
  rdfs:comment "Education premises including secondary schools, middle schools, high school";
  skos:broader bigg:EducationAndResearch .

bigg:EducationAndResearch.University a bigg:BuildingSpaceUseType, skos:Concept;
  rdfs:comment "Higher education premises including college, universities, technical schools, and professional schools";
  skos:broader bigg:EducationAndResearch .

bigg:EducationAndResearch.MilitaryOrPoliceAcademy a bigg:BuildingSpaceUseType, skos:Concept;
  rdfs:comment "Premises for the training of the military or police forces";
  skos:broader bigg:EducationAndResearch .

bigg:EducationAndResearch.ExtracurricularEducationCenter a bigg:BuildingSpaceUseType,
    skos:Concept;
  rdfs:comment "Education premises related to activities that fall outside the school, college, or university curriculum. This category includes music, language, and art schools";
  skos:broader bigg:EducationAndResearch .

bigg:EducationAndResearch.ResearchCenter a bigg:BuildingSpaceUseType, skos:Concept;
  rdfs:comment "Premises of a center or institute funded for doing research";
  skos:broader bigg:EducationAndResearch .

bigg:EducationAndResearch.Laboratory a bigg:BuildingSpaceUseType, skos:Concept;
  rdfs:comment "Building equipped for scientific experiments, research, or for the manufacture of drugs or chemicals";
  skos:broader bigg:EducationAndResearch .

bigg:EducationAndResearch.OtherEducationAndResearch a bigg:BuildingSpaceUseType, skos:Concept;
  rdfs:comment "Other facilities used for educational purposes and research";
  skos:broader bigg:EducationAndResearch .

bigg:SportsAndWellnessFacilities a bigg:BuildingSpaceUseType, skos:Concept;
  rdfs:comment "Facilities used for sports, physical activities and for body treatments " .

bigg:SportsAndWellnessFacilities.FitnessCenter a bigg:BuildingSpaceUseType, skos:Concept;
  rdfs:comment "Fitness center premises for active physical fitness conditioning including aerobic dance or exercise centers, or weight training centers";
  skos:broader bigg:SportsAndWellnessFacilities .

bigg:SportsAndWellnessFacilities.Spa a bigg:BuildingSpaceUseType, skos:Concept;
  rdfs:comment "Commercial establishment offering health and beauty treatment through such means as steam baths, exercise equipment, and massage";
  skos:broader bigg:SportsAndWellnessFacilities .

bigg:SportsAndWellnessFacilities.SwimmingPool a bigg:BuildingSpaceUseType, skos:Concept;
  rdfs:comment "Indoor or outdoor recreation premises for swimming or wave pool for fitness or recreational purposes";
  skos:broader bigg:SportsAndWellnessFacilities .

bigg:SportsAndWellnessFacilities.SportsHall a bigg:BuildingSpaceUseType, skos:Concept;
  rdfs:comment "A building or part of a building in which sports are played such as stadiums and arenas";
  skos:broader bigg:SportsAndWellnessFacilities .

bigg:SportsAndWellnessFacilities.SportsCenter a bigg:BuildingSpaceUseType, skos:Concept;
  rdfs:comment "A building where different sports can be played";
  skos:broader bigg:SportsAndWellnessFacilities .

bigg:Public a bigg:BuildingSpaceUseType, skos:Concept;
  rdfs:comment "Any other public building or structure that does not belong to the previous categories" .

bigg:Public.MonumentalComplex a bigg:BuildingSpaceUseType, skos:Concept;
  rdfs:comment "Monument building or monument complex";
  skos:broader bigg:Public .

bigg:Public.CourtHouse a bigg:BuildingSpaceUseType, skos:Concept;
  rdfs:comment "Building in which a judicial court is held";
  skos:broader bigg:Public .

bigg:Public.FireStation a bigg:BuildingSpaceUseType, skos:Concept;
  rdfs:comment "Structure for storing firefighting apparatus such as fire engines and related vehicles, personal protective equipment, and other specialized equipment";
  skos:broader bigg:Public .

bigg:Public.PoliceStation a bigg:BuildingSpaceUseType, skos:Concept;
  rdfs:comment "Headquarters of a police force";
  skos:broader bigg:Public .

bigg:Public.OtherPublicAuthorityFacilities a bigg:BuildingSpaceUseType, skos:Concept;
  rdfs:comment "Headquarters of other public authorities";
  skos:broader bigg:Public .

bigg:Public.Penitentiary a bigg:BuildingSpaceUseType, skos:Concept;
  rdfs:comment "Penitentiary or correctional facility";
  skos:broader bigg:Public .

bigg:Public.MunicipalHall a bigg:BuildingSpaceUseType, skos:Concept;
  rdfs:comment "Multi-use municipal space or hall";
  skos:broader bigg:Public .

bigg:Public.OtherPublic a bigg:BuildingSpaceUseType, skos:Concept;
  rdfs:comment "Any other public building or structure that does not belong to the previous categories";
  skos:broader bigg:Public .

bigg:ResidentialHousing a bigg:BuildingSpaceUseType, skos:Concept;
  rdfs:comment "Building designed to provide accomodation and related services to families and individuals" .

bigg:ResidentialHousing.DetachedSingleFamilyHousing a bigg:BuildingSpaceUseType, skos:Concept;
  rdfs:comment "A dwelling unit inhabited by a single family completely separated by open space on all sides";
  skos:broader bigg:ResidentialHousing .

bigg:ResidentialHousing.OtherSingleFamilyHousing a bigg:BuildingSpaceUseType, skos:Concept;
  rdfs:comment "Any other type of dwelling unit inhabited by a single family";
  skos:broader bigg:ResidentialHousing .

bigg:ResidentialHousing.MultiFamilyOneToFourStoreys a bigg:BuildingSpaceUseType, skos:Concept;
  rdfs:comment "A dwelling unit inhabited by multiple families that is developed on 1 to 4 storeys";
  skos:broader bigg:ResidentialHousing .

bigg:ResidentialHousing.MultiFamilyFiveOrMoreStoreys a bigg:BuildingSpaceUseType,
    skos:Concept;
  rdfs:comment "A dwelling unit inhabited by multiple families that is developed on 5 or more storeys";
  skos:broader bigg:ResidentialHousing .

bigg:ResidentialHousing.ResidentialGarage a bigg:BuildingSpaceUseType, skos:Concept;
  rdfs:comment "Structure for storing a vehicle or vehicles that may separate or attached to a home";
  skos:broader bigg:ResidentialHousing .

bigg:TransportRelated a bigg:BuildingSpaceUseType, skos:Concept;
  rdfs:comment "Building which use is related to transport and mobility" .

bigg:TransportRelated.BusStation a bigg:BuildingSpaceUseType, skos:Concept;
  rdfs:comment "Bus station building";
  skos:broader bigg:TransportRelated .

bigg:TransportRelated.TrainStation a bigg:BuildingSpaceUseType, skos:Concept;
  rdfs:comment "Train station building";
  skos:broader bigg:TransportRelated .

bigg:TransportRelated.PortBuilding a bigg:BuildingSpaceUseType, skos:Concept;
  rdfs:comment "Port building";
  skos:broader bigg:TransportRelated .

bigg:TransportRelated.AirportBuilding a bigg:BuildingSpaceUseType, skos:Concept;
  rdfs:comment "Airport building";
  skos:broader bigg:TransportRelated .

bigg:TransportRelated.ParkingGarage a bigg:BuildingSpaceUseType, skos:Concept;
  rdfs:comment "Enclosed, partially enclosed, or open parking premises including attached garage, underground parking, uncovered driveways or lots, and covered carports";
  skos:broader bigg:TransportRelated .

bigg:TransportRelated.OtherTransportRelatedBuilding a bigg:BuildingSpaceUseType, skos:Concept;
  rdfs:comment "Other building which use is related to transport and mobility";
  skos:broader bigg:TransportRelated .

bigg:Industrial a bigg:BuildingSpaceUseType, skos:Concept;
  rdfs:comment "Premises that include food processing, manufacturing, high tech, metal processing, pulp and paper firms" .

bigg:Industrial.WasteManagementFacility a bigg:BuildingSpaceUseType, skos:Concept;
  rdfs:comment "Premises designed to perform the activities and actions required to manage waste from its inception to its final disposal";
  skos:broader bigg:Industrial .

bigg:Industrial.Warehouse a bigg:BuildingSpaceUseType, skos:Concept;
  rdfs:comment "Premises with warehousing and storage facilities such as bulk farm products";
  skos:broader bigg:Industrial .

bigg:Other a bigg:BuildingSpaceUseType, skos:Concept;
  rdfs:comment "Building dedicated to other uses" .

bigg:Multi-use a bigg:BuildingSpaceUseType, skos:Concept;
  rdfs:comment "Building dedicated to multiple uses" .

bigg:Unknown a bigg:BuildingSpaceUseType, skos:Concept;
  rdfs:comment "Building which use or purpose is unknow to the user" .

bigg:LightingElement a bigg:BuildingSystemElementType, skos:Concept;
  rdfs:comment "Element used for the lighting of the building" .

bigg:LightingElement.Luminaire a bigg:BuildingSystemElementType, skos:Concept;
  rdfs:comment "A complete lighting module consisting of lamp(s) and ballast(s), together with the parts designed to distribute the light, to position and protect the lamps, and to connect the lamps to the power supply";
  skos:broader bigg:LightingElement .

bigg:LightingElement.Luminaire.IfcLamp a bigg:BuildingSystemElementType, skos:Concept;
  rdfs:comment "A light source element sometimes also referred to as bulb or tube";
  skos:broader bigg:LightingElement.Luminaire .

bigg:LightingElement.Luminaire.IfcLamp.IncandescentLamp a bigg:BuildingSystemElementType,
    skos:Concept;
  rdfs:comment "An electric light which produces light with a wire filament heated to a high temperature by an electric current passing through it, until it glows";
  skos:broader bigg:LightingElement.Luminaire.IfcLamp .

bigg:LightingElement.Luminaire.IfcLamp.FluorescentLamp a bigg:BuildingSystemElementType,
    skos:Concept;
  rdfs:comment "A low pressure mercury-vapor gas-discharge lamp that uses fluorescence to produce visible light";
  skos:broader bigg:LightingElement.Luminaire.IfcLamp .

bigg:LightingElement.Luminaire.IfcLamp.LEDLamp a bigg:BuildingSystemElementType, skos:Concept;
  rdfs:comment "An ensamble of light-emitting diode chips which together emit electric light";
  skos:broader bigg:LightingElement.Luminaire.IfcLamp .

bigg:LightingElement.Luminaire.IfcLamp.T5Lamp a bigg:BuildingSystemElementType, skos:Concept;
  rdfs:comment "A fluorescent tube with a 5/8 inch (15.9 mm) diameter";
  skos:broader bigg:LightingElement.Luminaire.IfcLamp .

bigg:LightingElement.Luminaire.IfcLamp.HIDLamp a bigg:BuildingSystemElementType, skos:Concept;
  rdfs:comment "A type of electrical gas-discharge lamp that produces light by means of an electric arc between tungsten electrodes housed inside a translucent or transparent fused quartz or fused alumina arc tube";
  skos:broader bigg:LightingElement.Luminaire.IfcLamp .

bigg:LightingElement.Luminaire.IfcLamp.OtherLamp a bigg:BuildingSystemElementType,
    skos:Concept;
  rdfs:comment "Other type of lamp";
  skos:broader bigg:LightingElement.Luminaire.IfcLamp .

bigg:LightingElement.Luminaire.IfcLightFixture a bigg:BuildingSystemElementType, skos:Concept;
  rdfs:comment "A light fixture is a container that is designed for the purpose of housing one or more lamps and optionally devices that control, restrict or vary their emission.";
  skos:broader bigg:LightingElement.Luminaire .

bigg:LightingElement.Luminaire.Ballast a bigg:BuildingSystemElementType, skos:Concept;
  rdfs:comment "A piece of equipment required to control the starting and operating voltages of electrical gas discharge lights.";
  skos:broader bigg:LightingElement.Luminaire .

bigg:LightingElement.Luminaire.Reflector a bigg:BuildingSystemElementType, skos:Concept;
  rdfs:comment "Luminaire component that serves the purpose of light guidance";
  skos:broader bigg:LightingElement.Luminaire .

bigg:LightingElement.LightDimmer a bigg:BuildingSystemElementType, skos:Concept;
  rdfs:comment "A device connected to a light fixture used to vary the brightness of light";
  skos:broader bigg:LightingElement .

bigg:LightingElement.OtherLightingElement a bigg:BuildingSystemElementType, skos:Concept;
  rdfs:comment "Other element of the lighting system";
  skos:broader bigg:LightingElement .

bigg:HVACAndHotWaterElement a bigg:BuildingSystemElementType, skos:Concept;
  rdfs:comment "Elements used for HVAC and/or hot water necessities of the building" .

bigg:HVACAndHotWaterElement.ProductionElements a bigg:BuildingSystemElementType, skos:Concept;
  rdfs:comment "Elements of the HVAC and hot water system involved in the heat/cool production process";
  skos:broader bigg:HVACAndHotWaterElement .

bigg:HVACAndHotWaterElement.ProductionElements.HeatPump a bigg:BuildingSystemElementType,
    skos:Concept;
  rdfs:comment "A device capable of extracting heat from an ambient at lower temperature and delivering it to another ambient at a higher temperature";
  skos:broader bigg:HVACAndHotWaterElement.ProductionElements .

bigg:HVACAndHotWaterElement.ProductionElements.Furnace a bigg:BuildingSystemElementType,
    skos:Concept;
  rdfs:comment "Packaged assembly of components that includes a heating source, a fan and an air filter, that relies on convection for heating delivery";
  skos:broader bigg:HVACAndHotWaterElement.ProductionElements .

bigg:HVACAndHotWaterElement.ProductionElements.EvaporativeCooler a bigg:BuildingSystemElementType,
    skos:Concept;
  rdfs:comment "A cooler that cools indoor air by moisture evaporation, thereby lowering its dry-bulb temperature and raising its wet-bulb temperature, all at a constant energy level";
  skos:broader bigg:HVACAndHotWaterElement.ProductionElements .

bigg:HVACAndHotWaterElement.ProductionElements.AirConditioner a bigg:BuildingSystemElementType,
    skos:Concept;
  rdfs:comment "A device that operated in an enclosed area via a refrigeration cycle in which heat is extracted from the air";
  skos:broader bigg:HVACAndHotWaterElement.ProductionElements .

bigg:HVACAndHotWaterElement.ProductionElements.DistrictHeating a bigg:BuildingSystemElementType,
    skos:Concept;
  rdfs:comment "A system used for the centralized production and distribution of heating energy";
  skos:broader bigg:HVACAndHotWaterElement.ProductionElements .

bigg:HVACAndHotWaterElement.ProductionElements.DisctrictCooling a bigg:BuildingSystemElementType,
    skos:Concept;
  rdfs:comment "A system used for the centralized production and distribution of cooling energy";
  skos:broader bigg:HVACAndHotWaterElement.ProductionElements .

bigg:HVACAndHotWaterElement.ProductionElements.DistrictCombinedHeatingAndCooling a
    bigg:BuildingSystemElementType, skos:Concept;
  rdfs:comment "A system used for the centralized production and distribution of both heating and cooling energy";
  skos:broader bigg:HVACAndHotWaterElement.ProductionElements .

bigg:HVACAndHotWaterElement.ProductionElements.CoolingTower a bigg:BuildingSystemElementType,
    skos:Concept;
  rdfs:comment "Heat exchanger that use water and air to transfer heat from air-conditioning systems to the outdoor environment";
  skos:broader bigg:HVACAndHotWaterElement.ProductionElements .

bigg:HVACAndHotWaterElement.ProductionElements.AirTerminalBox a bigg:BuildingSystemElementType,
    skos:Concept;
  rdfs:comment "A flow controller that participates in an HVAC duct distribution system and is used to control or modulate the amount of air delivered to its downstream ductwork";
  skos:broader bigg:HVACAndHotWaterElement.ProductionElements .

bigg:HVACAndHotWaterElement.ProductionElements.OtherProductionSystemElement a bigg:BuildingSystemElementType,
    skos:Concept;
  rdfs:comment "Other elements of the HVAC and hot water system involved in the heat/cool production process";
  skos:broader bigg:HVACAndHotWaterElement.ProductionElements .

bigg:HVACAndHotWaterElement.DistributionAndStorageElements a bigg:BuildingSystemElementType,
    skos:Concept;
  rdfs:comment "Elements of the HVAC and hot water system involved in the distribution process";
  skos:broader bigg:HVACAndHotWaterElement .

bigg:HVACAndHotWaterElement.DistributionAndStorageElements.Motor a bigg:BuildingSystemElementType,
    skos:Concept;
  rdfs:comment "An engine that converts electrical energy into mechanical energy";
  skos:broader bigg:HVACAndHotWaterElement.DistributionAndStorageElements .

bigg:HVACAndHotWaterElement.DistributionAndStorageElements.VariableSpeedDrive a bigg:BuildingSystemElementType,
    skos:Concept;
  rdfs:comment "A type of adjustable-speed drive used in electro-mechanical drive systems to control AC motor speed and torque by varying motor input frequency and voltage";
  skos:broader bigg:HVACAndHotWaterElement.DistributionAndStorageElements .

bigg:HVACAndHotWaterElement.DistributionAndStorageElements.Valve a bigg:BuildingSystemElementType,
    skos:Concept;
  rdfs:comment "An element of the building piping distribution system used to control or modulate the flow of the fluid";
  skos:broader bigg:HVACAndHotWaterElement.DistributionAndStorageElements .

bigg:HVACAndHotWaterElement.DistributionAndStorageElements.Filter a bigg:BuildingSystemElementType,
    skos:Concept;
  rdfs:comment "An apparatus used to remove particulate or gaseous matter from fluids and gases";
  skos:broader bigg:HVACAndHotWaterElement.DistributionAndStorageElements .

bigg:HVACAndHotWaterElement.DistributionAndStorageElements.Pipes a bigg:BuildingSystemElementType,
    skos:Concept;
  rdfs:comment "Tube used to convey water, gas, or other fluid substances in the distribution system of the building";
  skos:broader bigg:HVACAndHotWaterElement.DistributionAndStorageElements .

bigg:HVACAndHotWaterElement.DistributionAndStorageElements.Ducts a bigg:BuildingSystemElementType,
    skos:Concept;
  rdfs:comment "Conduits used in the distribution system of the building to deliver and remove air";
  skos:broader bigg:HVACAndHotWaterElement.DistributionAndStorageElements .

bigg:HVACAndHotWaterElement.DistributionAndStorageElements.StorageTank a bigg:BuildingSystemElementType,
    skos:Concept;
  rdfs:comment "A vessel or container in which water or another fluid stored for later use";
  skos:broader bigg:HVACAndHotWaterElement.DistributionAndStorageElements .

bigg:HVACAndHotWaterElement.DistributionAndStorageElements.HeatRecoveryUnit a bigg:BuildingSystemElementType,
    skos:Concept;
  rdfs:comment "An apparatus that extracts moist and stale air from the building, recovers heat from it, and uses it to supply clean, filtered, and pre-heated fresh air";
  skos:broader bigg:HVACAndHotWaterElement.DistributionAndStorageElements .

bigg:HVACAndHotWaterElement.DistributionAndStorageElements.HeatRecoveryUnit.AirToAirHeatRecovery
  a bigg:BuildingSystemElementType, skos:Concept;
  rdfs:comment "A balanced system in which the heat in extract air is recovered and transferred to the supply air";
  skos:broader bigg:HVACAndHotWaterElement.DistributionAndStorageElements.HeatRecoveryUnit .

bigg:HVACAndHotWaterElement.DistributionAndStorageElements.AirHandlingUnit a bigg:BuildingSystemElementType,
    skos:Concept;
  rdfs:comment "An apparatus that performs functions such as circulating, cleaning, humidifying, heating, cooling or mixing of air";
  skos:broader bigg:HVACAndHotWaterElement.DistributionAndStorageElements .

bigg:HVACAndHotWaterElement.DistributionAndStorageElements.OtherDistributionAndStorageElement
  a bigg:BuildingSystemElementType, skos:Concept;
  rdfs:comment "Other elements of the HVAC and hot water system involved in the distribution process";
  skos:broader bigg:HVACAndHotWaterElement.DistributionAndStorageElements .

bigg:HVACAndHotWaterElement.FinalElements a bigg:BuildingSystemElementType, skos:Concept;
  rdfs:comment "Final elements of the HVAC and hot water system ";
  skos:broader bigg:HVACAndHotWaterElement .

bigg:HVACAndHotWaterElement.FinalElements.IfcSpaceHeater a bigg:BuildingSystemElementType,
    skos:Concept;
  rdfs:comment "Space heaters utilize a combination of radiation and/or natural convection using a heating source such as electricity, steam or hot water to heat a limited space or area. ";
  skos:broader bigg:HVACAndHotWaterElement.FinalElements .

bigg:HVACAndHotWaterElement.FinalElements.IfcSpaceHeater.Radiator a bigg:BuildingSystemElementType,
    skos:Concept;
  rdfs:comment "An heat exchanger used to transfer thermal energy from one medium to another for the purpose of space heating";
  skos:broader bigg:HVACAndHotWaterElement.FinalElements.IfcSpaceHeater .

bigg:HVACAndHotWaterElement.FinalElements.ConvectorHeater a bigg:BuildingSystemElementType,
    skos:Concept;
  rdfs:comment "A type of heater that uses convection currents to heat and circulate air";
  skos:broader bigg:HVACAndHotWaterElement.FinalElements .

bigg:HVACAndHotWaterElement.FinalElements.RadiantFloorOrCeiling a bigg:BuildingSystemElementType,
    skos:Concept;
  rdfs:comment "Pipework  system installed below the floor or ceiling for the purpose of space heating or cooling";
  skos:broader bigg:HVACAndHotWaterElement.FinalElements .

bigg:HVACAndHotWaterElement.FinalElements.TapWaterSavingDevices a bigg:BuildingSystemElementType,
    skos:Concept;
  rdfs:comment "Installation of devices that reduce water consumption to taps and faucets (eg. aerators)";
  skos:broader bigg:HVACAndHotWaterElement.FinalElements .

bigg:HVACAndHotWaterElement.FinalElements.CooledBeam a bigg:BuildingSystemElementType,
    skos:Concept;
  rdfs:comment "Long rectangular finned tubes mounted at high level at regular intervals within a space that provide quiet draught-free cooling";
  skos:broader bigg:HVACAndHotWaterElement.FinalElements .

bigg:HVACAndHotWaterElement.FinalElements.OtherFinalElement a bigg:BuildingSystemElementType,
    skos:Concept;
  rdfs:comment "Other final elements of the HVAC and hot water system ";
  skos:broader bigg:HVACAndHotWaterElement.FinalElements .

bigg:HVACAndHotWaterElement.ControlElements a bigg:BuildingSystemElementType, skos:Concept;
  rdfs:comment "Elements of the HVAC and hot water system involved in the control of its subsystems that are not devices";
  skos:broader bigg:HVACAndHotWaterElement .

bigg:HVACAndHotWaterElement.ControlElements.ThermostaticValve a bigg:BuildingSystemElementType,
    skos:Concept;
  rdfs:comment "A thermostatic radiator valve (TRV) is a self-regulating valve fitted to hot water heating system radiator, to control the temperature of a room by changing the flow of hot water to the radiator.";
  skos:broader bigg:HVACAndHotWaterElement.ControlElements .

bigg:HVACAndHotWaterElement.ControlElements.Thermostat a bigg:BuildingSystemElementType,
    skos:Concept;
  rdfs:comment "A thermostat is a device that automatically regulates temperature, or that activates a device when the temperature reaches a certain point.";
  skos:broader bigg:HVACAndHotWaterElement.ControlElements .

bigg:HVACAndHotWaterElement.ControlElements.OtherControlElement a bigg:BuildingSystemElementType,
    skos:Concept;
  rdfs:comment "Other elements of the HVAC and hot water system involved in the control of its subsystems that are not devices";
  skos:broader bigg:HVACAndHotWaterElement.ControlElements .

bigg:BuildingFabricElement a bigg:BuildingSystemElementType, skos:Concept;
  rdfs:comment "Elements of the building fabric that are not construction elements" .

bigg:BuildingFabricElement.AirCurtain a bigg:BuildingSystemElementType, skos:Concept;
  rdfs:comment "A fan-powered device that creates an air barrier over a doorway or window to prevent to the loss of warm or cold air";
  skos:broader bigg:BuildingFabricElement .

bigg:BuildingFabricElement.OtherBuildingFabricElement a bigg:BuildingSystemElementType,
    skos:Concept;
  rdfs:comment "Other elements of the building fabric that are not construction elements";
  skos:broader bigg:BuildingFabricElement .

bigg:ElectricPowerElement a bigg:BuildingSystemElementType, skos:Concept;
  rdfs:comment "Elements of the electric power system of the building" .

bigg:ElectricPowerElement.PowerSystemElement a bigg:BuildingSystemElementType, skos:Concept;
  rdfs:comment "Elements of the electric power system of the building";
  skos:broader bigg:ElectricPowerElement .

bigg:ElectricPowerElement.PowerSystemElement.Transformer a bigg:BuildingSystemElementType,
    skos:Concept;
  rdfs:comment "An inductive stationary device that transfers electrical energy from one circuit to another and is used to transform electric power";
  skos:broader bigg:ElectricPowerElement.PowerSystemElement .

bigg:ElectricPowerElement.PowerSystemElement.Battery a bigg:BuildingSystemElementType,
    skos:Concept;
  rdfs:comment "An energy storage systems consisting of one or more cells, in which chemical energy is converted into electricity and used as a source of power";
  skos:broader bigg:ElectricPowerElement.PowerSystemElement .

bigg:ElectricPowerElement.PowerSystemElement.ElectricDistributionPanel a bigg:BuildingSystemElementType,
    skos:Concept;
  rdfs:comment "A component of an electricity supply system that divides the electrical power feed into subsidiary circuits, while providing a protective fuse or circuit breaker for each circuit in a common enclosure";
  skos:broader bigg:ElectricPowerElement.PowerSystemElement .

bigg:ElectricPowerElement.PowerSystemElement.UninterruptiblePowerSupplySystem a bigg:BuildingSystemElementType,
    skos:Concept;
  rdfs:comment "Uninterruptible Power Supply (UPS) is a combination of converters, switches, and energy storage devices (such as batteries) constituting a power system for maintaining continuity of load power in case of input power failure.";
  skos:broader bigg:ElectricPowerElement.PowerSystemElement .

bigg:ElectricPowerElement.PowerSystemElement.ElectricTimeControl a bigg:BuildingSystemElementType,
    skos:Concept;
  rdfs:comment "A device that applies control to the provision or flow of electrical energy over time";
  skos:broader bigg:ElectricPowerElement.PowerSystemElement .

bigg:ElectricPowerElement.PowerSystemElement.ProtectiveDevice a bigg:BuildingSystemElementType,
    skos:Concept;
  rdfs:comment "Breaks an electrical circuit when a stated electric current that passes through it is exceeded";
  skos:broader bigg:ElectricPowerElement.PowerSystemElement .

bigg:ElectricPowerElement.PowerSystemElement.SwitchingDevice a bigg:BuildingSystemElementType,
    skos:Concept;
  rdfs:comment "A switch is used in a cable distribution system (electrical circuit) to control or modulate the flow of electricity";
  skos:broader bigg:ElectricPowerElement.PowerSystemElement .

bigg:ElectricPowerElement.PowerSystemElement.OtherPowerSystemElement a bigg:BuildingSystemElementType,
    skos:Concept;
  rdfs:comment "Other elements of the electric power system of the building";
  skos:broader bigg:ElectricPowerElement.PowerSystemElement .

bigg:ElectricPowerElement.ElectricEquipmentElement a bigg:BuildingSystemElementType,
    skos:Concept;
  rdfs:comment "Any machine powered by electricity";
  skos:broader bigg:ElectricPowerElement .

bigg:ElectricPowerElement.ElectricEquipmentElement.ElectricAppliance a bigg:BuildingSystemElementType,
    skos:Concept;
  rdfs:comment "A device intended for consumer usage that is powered by electricity (provided from an electric circuit or a battery)";
  skos:broader bigg:ElectricPowerElement.ElectricEquipmentElement .

bigg:ElectricPowerElement.ElectricEquipmentElement.ElectricAppliance.VendingMachine
  a bigg:BuildingSystemElementType, skos:Concept;
  rdfs:comment "A machine that dispenses small articles such as food or drinks and that may require refrigeration capabilities";
  skos:broader bigg:ElectricPowerElement.ElectricEquipmentElement.ElectricAppliance .

bigg:ElectricPowerElement.ElectricEquipmentElement.ElectricAppliance.Elevator a bigg:BuildingSystemElementType,
    skos:Concept;
  rdfs:comment "An elevator is a platform or compartment housed in a shaft for raising and lowering people or things to different floors or levels";
  skos:broader bigg:ElectricPowerElement.ElectricEquipmentElement.ElectricAppliance .

bigg:ElectricPowerElement.ElectricEquipmentElement.ElectricAppliance.OtherElectricAppliance
  a bigg:BuildingSystemElementType, skos:Concept;
  rdfs:comment "Other electric appliance";
  skos:broader bigg:ElectricPowerElement.ElectricEquipmentElement.ElectricAppliance .

bigg:ElectricPowerElement.ICTEquipment a bigg:BuildingSystemElementType, skos:Concept;
  rdfs:comment "Any appliance that transmits and receives electronic or digital information as data or sound";
  skos:broader bigg:ElectricPowerElement .

bigg:ElectricPowerElement.ICTEquipment.Computer a bigg:BuildingSystemElementType,
    skos:Concept;
  rdfs:comment "A device which performs logical operations and processes data";
  skos:broader bigg:ElectricPowerElement.ICTEquipment .

bigg:ElectricPowerElement.ICTEquipment.Server a bigg:BuildingSystemElementType, skos:Concept;
  rdfs:comment "A computer server that is bundled with a pre-installed OS and application software that is used to perform a dedicated function or set of tightly coupled functions. Server appliances deliver services through one or more networks (e.g., IP or SAN), and are typically managed through a web or command line interface. Server appliance hardware and software configurations are customized by the vendor to perform a specific task (e.g., name services, firewall services, authentication services, encryption services, and voice-over-IP (VoIP) services), and are not intended to execute user-supplied software.";
  skos:broader bigg:ElectricPowerElement.ICTEquipment .

bigg:ElectricPowerElement.ICTEquipment.Printer a bigg:BuildingSystemElementType, skos:Concept;
  rdfs:comment "Generates paper output from electronic input. A printer is capable of receiving information from single-user or networked computers, or other input devices (e.g., digital cameras).";
  skos:broader bigg:ElectricPowerElement.ICTEquipment .

bigg:ElectricPowerElement.ICTEquipment.OtherICTEquipment a bigg:BuildingSystemElementType,
    skos:Concept;
  rdfs:comment "Other ICT equipment";
  skos:broader bigg:ElectricPowerElement.ICTEquipment .

bigg:RefrigerationElement a bigg:BuildingSystemElementType, skos:Concept;
  rdfs:comment "Elements of the refrigeration system of the building (does not include space cooling system elements)" .

bigg:RefrigerationElement.RefrigerationCompressor a bigg:BuildingSystemElementType,
    skos:Concept;
  rdfs:comment "A device that uses pistons or some other method to compress the refrigerant gas";
  skos:broader bigg:RefrigerationElement .

bigg:RefrigerationElement.RefrigerationCondenser a bigg:BuildingSystemElementType,
    skos:Concept;
  rdfs:comment "A device or unit used to condense a substance from its gaseous to its liquid state, by cooling it. In so doing, the latent heat is given up by the substance, and will transfer to the condenser coolant.";
  skos:broader bigg:RefrigerationElement .

bigg:RefrigerationElement.DefrostingSubsystem a bigg:BuildingSystemElementType, skos:Concept;
  rdfs:comment "System used for commercial refrigerated display and storage cabinets. Designed to remove frost (ice) from cooling coils of a refrigerating system.";
  skos:broader bigg:RefrigerationElement .

bigg:RefrigerationElement.FloatingHeadPressureController a bigg:BuildingSystemElementType,
    skos:Concept;
  rdfs:comment "A controller that allows the head pressure of the system to follow the ambient dry bulb temperature instead of a preset on/off operation and allows to achieve savings then occur from the load reduction of the refrigeration system";
  skos:broader bigg:RefrigerationElement .

bigg:RefrigerationElement.RefrigerationSpaceDoorsOrCurtains a bigg:BuildingSystemElementType,
    skos:Concept;
  rdfs:comment "Doors or curtains used to insulate a cold room from non-refrigerated areas of the building";
  skos:broader bigg:RefrigerationElement .

bigg:RefrigerationElement.OtherRefrigerationElement a bigg:BuildingSystemElementType,
    skos:Concept;
  rdfs:comment "Other element of the refrigeration system";
  skos:broader bigg:RefrigerationElement .

bigg:RenewableGenerationElement a bigg:BuildingSystemElementType, skos:Concept;
  rdfs:comment "Elements of the renewable generation system of the building" .

bigg:RenewableGenerationElement.SolarPhotovoltaicPanel a bigg:BuildingSystemElementType,
    skos:Concept;
  rdfs:comment "Photovoltaic (PV) panel that derive energy from incoming solar radiation";
  skos:broader bigg:RenewableGenerationElement .

bigg:RenewableGenerationElement.SolarThermalCollector a bigg:BuildingSystemElementType,
    skos:Concept;
  rdfs:comment "Collector used to heat air or water";
  skos:broader bigg:RenewableGenerationElement .

bigg:RenewableGenerationElement.OtherRenewableGenerationElement a bigg:BuildingSystemElementType,
    skos:Concept;
  rdfs:comment "Other element used for the generation of renewable energy";
  skos:broader bigg:RenewableGenerationElement .

bigg:IfcActuator a bigg:BuildingSystemElementType, skos:Concept .

bigg:IfcAlarm a bigg:BuildingSystemElementType, skos:Concept .

bigg:IfcController a bigg:BuildingSystemElementType, skos:Concept .

bigg:IfcElectricFlowStorageDevice a bigg:BuildingSystemElementType, skos:Concept;
  rdfs:comment "An electric flow storage device is a device in which electrical energy is stored and from which energy may be progressively released." .

bigg:IfcEnergyConversionDevice a bigg:BuildingSystemElementType, skos:Concept;
  rdfs:comment "Defines the occurrence of a device used to perform energy conversion or heat transfer and typically participates in a flow distribution system." .

bigg:IfcEnergyConversionDevice.IfcAirToAirHeatRecovery a bigg:BuildingSystemElementType,
    skos:Concept;
  rdfs:comment "Employs a counter-flow heat exchanger between inbound and outbound air flow.";
  skos:broader bigg:IfcEnergyConversionDevice .

bigg:IfcEnergyConversionDevice.IfcBoiler a bigg:BuildingSystemElementType, skos:Concept;
  rdfs:comment "A boiler is a closed, pressure-rated vessel in which water or other fluid is heated using an energy source such as natural gas, heating oil, or electricity.";
  skos:broader bigg:IfcEnergyConversionDevice .

bigg:IfcEnergyConversionDevice.IfcBurner a bigg:BuildingSystemElementType, skos:Concept;
  rdfs:comment "A burner is a device that converts fuel into heat through combustion. It includes gas, oil, and wood burners.";
  skos:broader bigg:IfcEnergyConversionDevice .

bigg:IfcEnergyConversionDevice.IfcChiller a bigg:BuildingSystemElementType, skos:Concept;
  rdfs:comment "A chiller is a device used to remove heat from a liquid via a vapor-compression or absorption refrigeration cycle to cool a fluid, typically water or a mixture of water and glycol. ";
  skos:broader bigg:IfcEnergyConversionDevice .

bigg:IfcEnergyConversionDevice.IfcCoil a bigg:BuildingSystemElementType, skos:Concept;
  rdfs:comment "A coil is a device used to provide heat transfer between non-mixing media.";
  skos:broader bigg:IfcEnergyConversionDevice .

bigg:IfcEnergyConversionDevice.IfcCondenser a bigg:BuildingSystemElementType, skos:Concept;
  rdfs:comment "A condenser is a device that is used to dissipate heat, typically by condensing a substance such as a refrigerant from its gaseous to its liquid state.";
  skos:broader bigg:IfcEnergyConversionDevice .

bigg:IfcEnergyConversionDevice.IfcCooledBeam a bigg:BuildingSystemElementType, skos:Concept;
  rdfs:comment "A cooled beam (or chilled beam) is a device typically used to cool air by circulating a fluid such as chilled water through exposed finned tubes above a space. ";
  skos:broader bigg:IfcEnergyConversionDevice .

bigg:IfcEnergyConversionDevice.IfcCoolingTower a bigg:BuildingSystemElementType, skos:Concept;
  rdfs:comment "A cooling tower is a device which rejects heat to ambient air by circulating a fluid such as water through it to reduce its temperature by partial evaporation.";
  skos:broader bigg:IfcEnergyConversionDevice .

bigg:IfcEnergyConversionDevice.IfcElectricGenerator a bigg:BuildingSystemElementType,
    skos:Concept;
  rdfs:comment "An electric generator is an engine that is a machine for converting mechanical energy into electrical energy.";
  skos:broader bigg:IfcEnergyConversionDevice .

bigg:IfcEnergyConversionDevice.IfcElectricMotor a bigg:BuildingSystemElementType,
    skos:Concept;
  rdfs:comment "An electric motor is an engine that is a machine for converting electrical energy into mechanical energy.";
  skos:broader bigg:IfcEnergyConversionDevice .

bigg:IfcEnergyConversionDevice.IfcEngine a bigg:BuildingSystemElementType, skos:Concept;
  rdfs:comment "An engine is a device that converts fuel into mechanical energy through combustion.";
  skos:broader bigg:IfcEnergyConversionDevice .

bigg:IfcEnergyConversionDevice.IfcEvaporativeCooler a bigg:BuildingSystemElementType,
    skos:Concept;
  rdfs:comment "An evaporative cooler is a device that cools air by saturating it with water vapor.";
  skos:broader bigg:IfcEnergyConversionDevice .

bigg:IfcEnergyConversionDevice.IfcEvaporator a bigg:BuildingSystemElementType, skos:Concept;
  rdfs:comment "An evaporator is a device in which a liquid refrigerent is vaporized and absorbs heat from the surrounding fluid.";
  skos:broader bigg:IfcEnergyConversionDevice .

bigg:IfcEnergyConversionDevice.IfcHeatExchanger a bigg:BuildingSystemElementType,
    skos:Concept;
  rdfs:comment "A heat exchanger is a device used to provide heat transfer between non-mixing media such as plate and shell and tube heat exchangers.";
  skos:broader bigg:IfcEnergyConversionDevice .

bigg:IfcEnergyConversionDevice.IfcHumidifier a bigg:BuildingSystemElementType, skos:Concept;
  rdfs:comment "A humidifier is a device that adds moisture into the air.";
  skos:broader bigg:IfcEnergyConversionDevice .

bigg:IfcEnergyConversionDevice.IfcMotorConnection a bigg:BuildingSystemElementType,
    skos:Concept;
  rdfs:comment "A motor connection provides the means for connecting a motor as the driving device to the driven device.";
  skos:broader bigg:IfcEnergyConversionDevice .

bigg:IfcEnergyConversionDevice.IfcSolarDevice a bigg:BuildingSystemElementType, skos:Concept;
  rdfs:comment "A solar device converts solar radiation into other energy such as electric current or thermal energy.";
  skos:broader bigg:IfcEnergyConversionDevice .

bigg:IfcEnergyConversionDevice.IfcTransformer a bigg:BuildingSystemElementType, skos:Concept;
  rdfs:comment "A transformer is an inductive stationary device that transfers electrical energy from one circuit to another.";
  skos:broader bigg:IfcEnergyConversionDevice .

bigg:IfcEnergyConversionDevice.IfcTubeBundle a bigg:BuildingSystemElementType, skos:Concept;
  rdfs:comment "A tube bundle is a device consisting of tubes and bundles of tubes used for heat transfer and contained typically within other energy conversion devices, such as a chiller or coil.";
  skos:broader bigg:IfcEnergyConversionDevice .

bigg:IfcEnergyConversionDevice.IfcUnitaryEquipment a bigg:BuildingSystemElementType,
    skos:Concept;
  rdfs:comment "Unitary equipment typically combine a number of components into a single product, such as air handlers, pre-packaged rooftop air-conditioning units, heat pumps, and split systems.";
  skos:broader bigg:IfcEnergyConversionDevice .

bigg:IfcFlowController a bigg:BuildingSystemElementType, skos:Concept;
  rdfs:comment "The distribution flow element IfcFlowController defines the occurrence of elements of a distribution system that are used to regulate flow through a distribution system. " .

bigg:IfcFlowController.IfcAirTerminalBox a bigg:BuildingSystemElementType, skos:Concept;
  rdfs:comment "An air terminal box typically participates in an HVAC duct distribution system and is used to control or modulate the amount of air delivered to its downstream ductwork. ";
  skos:broader bigg:IfcFlowController .

bigg:IfcFlowController.IfcDamper a bigg:BuildingSystemElementType, skos:Concept;
  rdfs:comment "A damper typically participates in an HVAC duct distribution system and is used to control or modulate the flow of air.";
  skos:broader bigg:IfcFlowController .

bigg:IfcFlowController.IfcElectricDistributionBoard a bigg:BuildingSystemElementType,
    skos:Concept;
  rdfs:comment "A distribution board is a flow controller in which instances of electrical devices are brought together at a single place for a particular purpose.";
  skos:broader bigg:IfcFlowController .

bigg:IfcFlowController.IfcElectricTimeControl a bigg:BuildingSystemElementType, skos:Concept;
  rdfs:comment "An electric time control is a device that applies control to the provision or flow of electrical energy over time.";
  skos:broader bigg:IfcFlowController .

bigg:IfcFlowController.IfcProtectiveDevice a bigg:BuildingSystemElementType, skos:Concept;
  rdfs:comment "A protective device breaks an electrical circuit when a stated electric current that passes through it is exceeded.";
  skos:broader bigg:IfcFlowController .

bigg:IfcFlowController.IfcSwitchingDevice a bigg:BuildingSystemElementType, skos:Concept;
  rdfs:comment "A switch is used in a cable distribution system (electrical circuit) to control or modulate the flow of electricity.";
  skos:broader bigg:IfcFlowController .

bigg:IfcFlowController.IfcValve a bigg:BuildingSystemElementType, skos:Concept;
  rdfs:comment "A valve is used in a building services piping distribution system to control or modulate the flow of the fluid.";
  skos:broader bigg:IfcFlowController .

bigg:IfcFlowMovingDevice a bigg:BuildingSystemElementType, skos:Concept;
  rdfs:comment "defines the occurrence of an apparatus used to distribute, circulate or perform conveyance of fluids, including liquids and gases (such as a pump or fan), and typically participates in a flow distribution system." .

bigg:IfcFlowMovingDevice.IfcCompressor a bigg:BuildingSystemElementType, skos:Concept;
  rdfs:comment "A compressor is a device that compresses a fluid typically used in a refrigeration circuit.";
  skos:broader bigg:IfcFlowMovingDevice .

bigg:IfcFlowMovingDevice.IfcFan a bigg:BuildingSystemElementType, skos:Concept;
  rdfs:comment "A fan is a device which imparts mechanical work on a gas. A typical usage of a fan is to induce airflow in a building services air distribution system.";
  skos:broader bigg:IfcFlowMovingDevice .

bigg:IfcFlowMovingDevice a bigg:BuildingSystemElementType, skos:Concept;
  rdfs:comment "defines the occurrence of an apparatus used to distribute, circulate or perform conveyance of fluids, including liquids and gases (such as a pump or fan), and typically participates in a flow distribution system." .

bigg:IfcFlowMovingDevice.IfcPump a bigg:BuildingSystemElementType, skos:Concept;
  rdfs:comment "A pump is a device which imparts mechanical work on fluids or slurries to move them through a channel or pipeline.";
  skos:broader bigg:IfcFlowMovingDevice .

bigg:IfcUnitaryControlElement a bigg:BuildingSystemElementType, skos:Concept .

bigg:BuildingEnergyManagementSystem a bigg:DeviceType, skos:Concept;
  rdfs:comment "A software system to automate building controls, also known as an Energy Management Control Systems (EMCS)." .

bigg:IfcDistributionControlElement a bigg:DeviceType, skos:Concept;
  rdfs:comment "A building automation device that is used to impart control over elements of one of its systems" .

bigg:IfcDistributionControlElement.IfcFlowInstrument a bigg:DeviceType, skos:Concept;
  rdfs:comment "A flow instrument reads and displays the value of a particular property of a system at a point, or displays the difference in the value of a property between two points.";
  skos:broader bigg:IfcDistributionControlElement .

bigg:IfcDistributionControlElement.IfcSensor a bigg:DeviceType, skos:Concept;
  rdfs:comment "A device that measures a physical quantity and converts it into a signal which can be read by an observer or by an instrument";
  skos:broader bigg:IfcDistributionControlElement .

bigg:IfcDistributionControlElement.IfcSensor.LightSensor a bigg:DeviceType, skos:Concept;
  rdfs:comment "A passive device that convert photons into an electrical signal output";
  skos:broader bigg:IfcDistributionControlElement.IfcSensor .

bigg:IfcDistributionControlElement.IfcSensor.OccupancySensor a bigg:DeviceType, skos:Concept;
  rdfs:comment "A motion detecting device used to detect the presence of a person, oftern used to automatically control one of the building systems";
  skos:broader bigg:IfcDistributionControlElement.IfcSensor .

bigg:IfcDistributionControlElement.IfcSensor.TemperatureSensor a bigg:DeviceType,
    skos:Concept;
  rdfs:comment "An electronic device that converts the measurement of the temperature of its environment into electronic data";
  skos:broader bigg:IfcDistributionControlElement.IfcSensor .

bigg:IfcDistributionControlElement.IfcSensor.PressureSensor a bigg:DeviceType, skos:Concept;
  rdfs:comment "An electronic device that converts the measurement of the pressure of its environment into electronic data";
  skos:broader bigg:IfcDistributionControlElement.IfcSensor .

bigg:IfcDistributionControlElement.Timer a bigg:DeviceType, skos:Concept;
  rdfs:comment "An automatic mechanism for activating a device at a preset time";
  skos:broader bigg:IfcDistributionControlElement .

bigg:IfcDistributionControlElement.Thermostat a bigg:DeviceType, skos:Concept;
  rdfs:comment "A device that automatically regulates temperature, or that activates a device when the temperature reaches a certain point";
  skos:broader bigg:IfcDistributionControlElement .

bigg:Meter a bigg:DeviceType, skos:Concept;
  rdfs:comment "A device built to accurately detect and display a quantity in a form readable by a human being" .

bigg:Meter.IfcFlowMeter a bigg:DeviceType, skos:Concept;
  rdfs:comment "A flow meter is a device that is used to measure the flow rate in a system.";
  skos:broader bigg:Meter .

bigg:Meter.EnergyMeter a bigg:DeviceType, skos:Concept;
  skos:broader bigg:Meter .

bigg:Meter.EnergyMeter.SmartMeter a bigg:DeviceType, skos:Concept;
  rdfs:comment "A smart meter is usually an electronic device that records consumption of electric energy in intervals of an hour or less and communicates that information at least daily back to the utility for monitoring and billing.";
  skos:broader bigg:Meter.EnergyMeter .

bigg:Meter.EnergyMeter.AnalogMeter a bigg:DeviceType, skos:Concept;
  skos:broader bigg:Meter.EnergyMeter .

bigg:OtherDevice a bigg:DeviceType, skos:Concept;
  rdfs:comment "Other device type" .

bigg:LightingMeasure a bigg:EnergyEfficiencyMeasureType, skos:Concept;
  rdfs:comment "Measure that affects the lighting system of the building" .

bigg:LightingMeasure.LightingIndoorMeasure a bigg:EnergyEfficiencyMeasureType, skos:Concept;
  rdfs:comment "Measure that affects the indoor lighting system of the building";
  skos:broader bigg:LightingMeasure .

bigg:LightingMeasure.LightingIndoorMeasure.IndoorRelamp a bigg:EnergyEfficiencyMeasureType,
    skos:Concept;
  rdfs:comment "Replacement of the indoor lighting units or of their subcomponents";
  skos:broader bigg:LightingMeasure.LightingIndoorMeasure .

bigg:LightingMeasure.LightingIndoorMeasure.IndoorRelamp.IndoorRelampToLED a bigg:EnergyEfficiencyMeasureType,
    skos:Concept;
  rdfs:comment "Replacement of the lighting units with LED ones";
  skos:broader bigg:LightingMeasure.LightingIndoorMeasure.IndoorRelamp .

bigg:LightingMeasure.LightingIndoorMeasure.IndoorRelamp.IndoorRelampToT5 a bigg:EnergyEfficiencyMeasureType,
    skos:Concept;
  rdfs:comment "Replacement of the lighting units with T5 ones";
  skos:broader bigg:LightingMeasure.LightingIndoorMeasure.IndoorRelamp .

bigg:LightingMeasure.LightingIndoorMeasure.IndoorRelamp.IndoorBallastReplacement a
    bigg:EnergyEfficiencyMeasureType, skos:Concept;
  rdfs:comment "Replacement of hemagnetic ballasts with electronic ones";
  skos:broader bigg:LightingMeasure.LightingIndoorMeasure.IndoorRelamp .

bigg:LightingMeasure.LightingIndoorMeasure.IndoorRelamp.OtherIndoorRelamp a bigg:EnergyEfficiencyMeasureType,
    skos:Concept;
  rdfs:comment "Other indoor relamp measure";
  skos:broader bigg:LightingMeasure.LightingIndoorMeasure.IndoorRelamp .

bigg:LightingMeasure.LightingIndoorMeasure.IndoorLightingTechnicalOptimization a bigg:EnergyEfficiencyMeasureType,
    skos:Concept;
  rdfs:comment "Technical optimization of the indoor lighting system by component renewal, supplement, or maintenance";
  skos:broader bigg:LightingMeasure.LightingIndoorMeasure .

bigg:LightingMeasure.LightingIndoorMeasure.IndoorLightingTechnicalOptimization.IndoorReflectorsInstallation
  a bigg:EnergyEfficiencyMeasureType, skos:Concept;
  rdfs:comment "Installation of light reflectors";
  skos:broader bigg:LightingMeasure.LightingIndoorMeasure.IndoorLightingTechnicalOptimization .

bigg:LightingMeasure.LightingIndoorMeasure.IndoorLightingTechnicalOptimization.IndoorLightSourcesReduction
  a bigg:EnergyEfficiencyMeasureType, skos:Concept;
  rdfs:comment "Reduction of the number of light sources";
  skos:broader bigg:LightingMeasure.LightingIndoorMeasure.IndoorLightingTechnicalOptimization .

bigg:LightingMeasure.LightingIndoorMeasure.IndoorLightingTechnicalOptimization.OtherIndoorTechnicalOptimization
  a bigg:EnergyEfficiencyMeasureType, skos:Concept;
  rdfs:comment "Other indoor lighting technical optimization measure";
  skos:broader bigg:LightingMeasure.LightingIndoorMeasure.IndoorLightingTechnicalOptimization .

bigg:LightingMeasure.LightingIndoorMeasure.IndoorLightingOperationalOptimization a
    bigg:EnergyEfficiencyMeasureType, skos:Concept;
  rdfs:comment "Operational optimization by controls and automation or maintenance";
  skos:broader bigg:LightingMeasure.LightingIndoorMeasure .

bigg:LightingMeasure.LightingIndoorMeasure.IndoorLightingOperationalOptimization.IndoorNaturalLightMaximization
  a bigg:EnergyEfficiencyMeasureType, skos:Concept;
  rdfs:comment "Maximization of natural light use";
  skos:broader bigg:LightingMeasure.LightingIndoorMeasure.IndoorLightingOperationalOptimization .

bigg:LightingMeasure.LightingIndoorMeasure.IndoorLightingOperationalOptimization.IndoorLightingUnitsCleaning
  a bigg:EnergyEfficiencyMeasureType, skos:Concept;
  rdfs:comment "Cleaning of the lamps or luminaries ";
  skos:broader bigg:LightingMeasure.LightingIndoorMeasure.IndoorLightingOperationalOptimization .

bigg:LightingMeasure.LightingIndoorMeasure.IndoorLightingOperationalOptimization.IndoorOccupancySensorInstallation
  a bigg:EnergyEfficiencyMeasureType, skos:Concept;
  rdfs:comment "Installation of occupancy sensor to automate the turning on/off of the lighting units";
  skos:broader bigg:LightingMeasure.LightingIndoorMeasure.IndoorLightingOperationalOptimization .

bigg:LightingMeasure.LightingIndoorMeasure.IndoorLightingOperationalOptimization.IndoorLightingTimersInstallation
  a bigg:EnergyEfficiencyMeasureType, skos:Concept;
  rdfs:comment "Installation of timers to automate the turning on/off of the lighting units";
  skos:broader bigg:LightingMeasure.LightingIndoorMeasure.IndoorLightingOperationalOptimization .

bigg:LightingMeasure.LightingIndoorMeasure.IndoorLightingOperationalOptimization.IndoorLightControlInstallation
  a bigg:EnergyEfficiencyMeasureType, skos:Concept;
  rdfs:comment "Installation of light sensors or dimmers to automate the turning on/off or intensity of the lighting units";
  skos:broader bigg:LightingMeasure.LightingIndoorMeasure.IndoorLightingOperationalOptimization .

bigg:LightingMeasure.LightingIndoorMeasure.IndoorLightingOperationalOptimization.OtherIndoorOperationalOptimization
  a bigg:EnergyEfficiencyMeasureType, skos:Concept;
  rdfs:comment "Other indoor lighting operational optimization measure";
  skos:broader bigg:LightingMeasure.LightingIndoorMeasure.IndoorLightingOperationalOptimization .

bigg:LightingMeasure.LightingOutdoorMeasure a bigg:EnergyEfficiencyMeasureType, skos:Concept;
  rdfs:comment "Measure that affects the outdoor lighting system of the building";
  skos:broader bigg:LightingMeasure .

bigg:LightingMeasure.LightingOutdoorMeasure.OutdoorRelamp a bigg:EnergyEfficiencyMeasureType,
    skos:Concept;
  rdfs:comment "Replacement of the outdoor lighting units or of their subcomponents";
  skos:broader bigg:LightingMeasure.LightingOutdoorMeasure .

bigg:LightingMeasure.LightingOutdoorMeasure.OutdoorRelamp.OutdoorRelampToLED a bigg:EnergyEfficiencyMeasureType,
    skos:Concept;
  rdfs:comment "Replacement of the units with LED ones";
  skos:broader bigg:LightingMeasure.LightingOutdoorMeasure.OutdoorRelamp .

bigg:LightingMeasure.LightingOutdoorMeasure.OutdoorRelamp.OutdoorRelampToT5 a bigg:EnergyEfficiencyMeasureType,
    skos:Concept;
  rdfs:comment "Replacement of the lighting units with T5 ones";
  skos:broader bigg:LightingMeasure.LightingOutdoorMeasure.OutdoorRelamp .

bigg:LightingMeasure.LightingOutdoorMeasure.OutdoorRelamp.OutdoorBallastReplacement
  a bigg:EnergyEfficiencyMeasureType, skos:Concept;
  rdfs:comment "Replacement of  hemagnetic ballasts with electronic ones";
  skos:broader bigg:LightingMeasure.LightingOutdoorMeasure.OutdoorRelamp .

bigg:LightingMeasure.LightingOutdoorMeasure.OutdoorRelamp.OtherOutdoorRelamp a bigg:EnergyEfficiencyMeasureType,
    skos:Concept;
  rdfs:comment "Other outdoor relamp measure";
  skos:broader bigg:LightingMeasure.LightingOutdoorMeasure.OutdoorRelamp .

bigg:LightingMeasure.LightingOutdoorMeasure.OutdoorLightingTechnicalOptimization a
    bigg:EnergyEfficiencyMeasureType, skos:Concept;
  rdfs:comment "Technical optimization of the outdoor lighting system by component renewal, supplement, or maintenance";
  skos:broader bigg:LightingMeasure.LightingOutdoorMeasure .

bigg:LightingMeasure.LightingOutdoorMeasure.OutdoorLightingTechnicalOptimization.OutdoorReflectorsInstallation
  a bigg:EnergyEfficiencyMeasureType, skos:Concept;
  rdfs:comment "Installation of light reflectors";
  skos:broader bigg:LightingMeasure.LightingOutdoorMeasure.OutdoorLightingTechnicalOptimization .

bigg:LightingMeasure.LightingOutdoorMeasure.OutdoorLightingTechnicalOptimization.OutdoorLightSourcesReduction
  a bigg:EnergyEfficiencyMeasureType, skos:Concept;
  rdfs:comment "Reduction of the number of light sources";
  skos:broader bigg:LightingMeasure.LightingOutdoorMeasure.OutdoorLightingTechnicalOptimization .

bigg:LightingMeasure.LightingOutdoorMeasure.OutdoorLightingTechnicalOptimization.OtherOutdoorTechnicalOptimization
  a bigg:EnergyEfficiencyMeasureType, skos:Concept;
  rdfs:comment "Other outdoor lighting technical optimization measure";
  skos:broader bigg:LightingMeasure.LightingOutdoorMeasure.OutdoorLightingTechnicalOptimization .

bigg:LightingMeasure.LightingOutdoorMeasure.OutdoorLightingOperationalOptimization
  a bigg:EnergyEfficiencyMeasureType, skos:Concept;
  rdfs:comment "Operational optimization by controls and automation or maintenance";
  skos:broader bigg:LightingMeasure.LightingOutdoorMeasure .

bigg:LightingMeasure.LightingOutdoorMeasure.OutdoorLightingOperationalOptimization.OutdoorNaturalLightMaximization
  a bigg:EnergyEfficiencyMeasureType, skos:Concept;
  rdfs:comment "Maximization of natural light use";
  skos:broader bigg:LightingMeasure.LightingOutdoorMeasure.OutdoorLightingOperationalOptimization .

bigg:LightingMeasure.LightingOutdoorMeasure.OutdoorLightingOperationalOptimization.OutdoorLightingUnitsCleaning
  a bigg:EnergyEfficiencyMeasureType, skos:Concept;
  rdfs:comment "Cleaning of the lamps or luminaries ";
  skos:broader bigg:LightingMeasure.LightingOutdoorMeasure.OutdoorLightingOperationalOptimization .

bigg:LightingMeasure.LightingOutdoorMeasure.OutdoorLightingOperationalOptimization.OutdoorOccupancySensorInstallation
  a bigg:EnergyEfficiencyMeasureType, skos:Concept;
  rdfs:comment "Installation of occupancy sensor to automate the turning on/off of the lighting units";
  skos:broader bigg:LightingMeasure.LightingOutdoorMeasure.OutdoorLightingOperationalOptimization .

bigg:LightingMeasure.LightingOutdoorMeasure.OutdoorLightingOperationalOptimization.OutdoorLightingTimersInstallation
  a bigg:EnergyEfficiencyMeasureType, skos:Concept;
  rdfs:comment "Installation of timers to automate the turning on/off of the lighting units";
  skos:broader bigg:LightingMeasure.LightingOutdoorMeasure.OutdoorLightingOperationalOptimization .

bigg:LightingMeasure.LightingOutdoorMeasure.OutdoorLightingOperationalOptimization.OutdoorLightControlInstallation
  a bigg:EnergyEfficiencyMeasureType, skos:Concept;
  rdfs:comment "Installation of light sensors or dimmers to automate the turning on/off or intensity of the lighting units";
  skos:broader bigg:LightingMeasure.LightingOutdoorMeasure.OutdoorLightingOperationalOptimization .

bigg:LightingMeasure.LightingOutdoorMeasure.OutdoorLightingOperationalOptimization.OtherOutdoorOperationalOptimization
  a bigg:EnergyEfficiencyMeasureType, skos:Concept;
  rdfs:comment "Other outdoor lighting operational optimization measure";
  skos:broader bigg:LightingMeasure.LightingOutdoorMeasure.OutdoorLightingOperationalOptimization .

bigg:HVACAndHotWaterMeasure a bigg:EnergyEfficiencyMeasureType, skos:Concept;
  rdfs:comment "Measure that affects the space heating, ventilation, air conditioning, or water heating system of the building" .

bigg:HVACAndHotWaterMeasure.HeatingSystemMeasure a bigg:EnergyEfficiencyMeasureType,
    skos:Concept;
  rdfs:comment "Measure that only affects the space heating system of the building";
  skos:broader bigg:HVACAndHotWaterMeasure .

bigg:HVACAndHotWaterMeasure.HeatingSystemMeasure.HeatProductionMeasure a bigg:EnergyEfficiencyMeasureType,
    skos:Concept;
  rdfs:comment "Measure that affects the heat production subsystem of space heating";
  skos:broader bigg:HVACAndHotWaterMeasure.HeatingSystemMeasure .

bigg:HVACAndHotWaterMeasure.HeatingSystemMeasure.HeatProductionMeasure.HeatingBoilerReplacement
  a bigg:EnergyEfficiencyMeasureType, skos:Concept;
  rdfs:comment "Replacement of the boiler with a more efficient one that uses the same fuel";
  skos:broader bigg:HVACAndHotWaterMeasure.HeatingSystemMeasure.HeatProductionMeasure .

bigg:HVACAndHotWaterMeasure.HeatingSystemMeasure.HeatProductionMeasure.HeatingHeatPumpReplacement
  a bigg:EnergyEfficiencyMeasureType, skos:Concept;
  rdfs:comment "Replacement of the heat pump with a more efficient one";
  skos:broader bigg:HVACAndHotWaterMeasure.HeatingSystemMeasure.HeatProductionMeasure .

bigg:HVACAndHotWaterMeasure.HeatingSystemMeasure.HeatProductionMeasure.HeatProductionFuelConversion
  a bigg:EnergyEfficiencyMeasureType, skos:Concept;
  rdfs:comment "Replacement of the heat production system with one that operates with a different fuel source ";
  skos:broader bigg:HVACAndHotWaterMeasure.HeatingSystemMeasure.HeatProductionMeasure .

bigg:HVACAndHotWaterMeasure.HeatingSystemMeasure.HeatProductionMeasure.HeatingHeatExchangersReplacement
  a bigg:EnergyEfficiencyMeasureType, skos:Concept;
  rdfs:comment "Replacement of heat exchangers ";
  skos:broader bigg:HVACAndHotWaterMeasure.HeatingSystemMeasure.HeatProductionMeasure .

bigg:HVACAndHotWaterMeasure.HeatingSystemMeasure.HeatProductionMeasure.HeatingBurnerReplacement
  a bigg:EnergyEfficiencyMeasureType, skos:Concept;
  rdfs:comment "Replacement of the burner";
  skos:broader bigg:HVACAndHotWaterMeasure.HeatingSystemMeasure.HeatProductionMeasure .

bigg:HVACAndHotWaterMeasure.HeatingSystemMeasure.HeatProductionMeasure.HeatingOtherElementReplacement
  a bigg:EnergyEfficiencyMeasureType, skos:Concept;
  rdfs:comment "Change of another single component in the heat production system";
  skos:broader bigg:HVACAndHotWaterMeasure.HeatingSystemMeasure.HeatProductionMeasure .

bigg:HVACAndHotWaterMeasure.HeatingSystemMeasure.HeatProductionMeasure.HeatProductionSystemInsulation
  a bigg:EnergyEfficiencyMeasureType, skos:Concept;
  rdfs:comment "Improvement of the heat production elements insulation";
  skos:broader bigg:HVACAndHotWaterMeasure.HeatingSystemMeasure.HeatProductionMeasure .

bigg:HVACAndHotWaterMeasure.HeatingSystemMeasure.HeatProductionMeasure.DistrictHeatingConnection
  a bigg:EnergyEfficiencyMeasureType, skos:Concept;
  rdfs:comment "Connection of the building space heating system to district heating";
  skos:broader bigg:HVACAndHotWaterMeasure.HeatingSystemMeasure.HeatProductionMeasure .

bigg:HVACAndHotWaterMeasure.HeatingSystemMeasure.HeatProductionMeasure.OtherHeatProductionMeasure
  a bigg:EnergyEfficiencyMeasureType, skos:Concept;
  rdfs:comment "Other measure on the heat production system";
  skos:broader bigg:HVACAndHotWaterMeasure.HeatingSystemMeasure.HeatProductionMeasure .

bigg:HVACAndHotWaterMeasure.HeatingSystemMeasure.HeatingDistributionAndStorageMeasure
  a bigg:EnergyEfficiencyMeasureType, skos:Concept;
  rdfs:comment "Measure that affects the distribution or the storage subsystems of space heating ";
  skos:broader bigg:HVACAndHotWaterMeasure.HeatingSystemMeasure .

bigg:HVACAndHotWaterMeasure.HeatingSystemMeasure.HeatingDistributionAndStorageMeasure.HeatingDistributionSystemReplacement
  a bigg:EnergyEfficiencyMeasureType, skos:Concept;
  rdfs:comment "Complete change of the heating distribution system ";
  skos:broader bigg:HVACAndHotWaterMeasure.HeatingSystemMeasure.HeatingDistributionAndStorageMeasure .

bigg:HVACAndHotWaterMeasure.HeatingSystemMeasure.HeatingDistributionAndStorageMeasure.HeatingDistributionPumpReplacement
  a bigg:EnergyEfficiencyMeasureType, skos:Concept;
  rdfs:comment "Replacement of a pump";
  skos:broader bigg:HVACAndHotWaterMeasure.HeatingSystemMeasure.HeatingDistributionAndStorageMeasure .

bigg:HVACAndHotWaterMeasure.HeatingSystemMeasure.HeatingDistributionAndStorageMeasure.HeatingDistributionFanReplacement
  a bigg:EnergyEfficiencyMeasureType, skos:Concept;
  rdfs:comment "Replacement of a fan";
  skos:broader bigg:HVACAndHotWaterMeasure.HeatingSystemMeasure.HeatingDistributionAndStorageMeasure .

bigg:HVACAndHotWaterMeasure.HeatingSystemMeasure.HeatingDistributionAndStorageMeasure.HeatingDistibutionVariableSpeedDrivesInstallation
  a bigg:EnergyEfficiencyMeasureType, skos:Concept;
  rdfs:comment "Installation of variable speed drives for the control of heating distribution elements (eg. Pumps, fans,…)";
  skos:broader bigg:HVACAndHotWaterMeasure.HeatingSystemMeasure.HeatingDistributionAndStorageMeasure .

bigg:HVACAndHotWaterMeasure.HeatingSystemMeasure.HeatingDistributionAndStorageMeasure.HeatingDistributionOtherComponentReplacement
  a bigg:EnergyEfficiencyMeasureType, skos:Concept;
  rdfs:comment "Replacement or installation of other distribution elements (eg. valves or filters)";
  skos:broader bigg:HVACAndHotWaterMeasure.HeatingSystemMeasure.HeatingDistributionAndStorageMeasure .

bigg:HVACAndHotWaterMeasure.HeatingSystemMeasure.HeatingDistributionAndStorageMeasure.HeatingDistributionBalancingAndFlowRegulation
  a bigg:EnergyEfficiencyMeasureType, skos:Concept;
  rdfs:comment "Optimization of the heating distribution through regulation of the water/airflow (eg. by means of balancing valves or dampers) ";
  skos:broader bigg:HVACAndHotWaterMeasure.HeatingSystemMeasure.HeatingDistributionAndStorageMeasure .

bigg:HVACAndHotWaterMeasure.HeatingSystemMeasure.HeatingDistributionAndStorageMeasure.HeatingPipesSubstitution
  a bigg:EnergyEfficiencyMeasureType, skos:Concept;
  rdfs:comment "Substitution of the pipes";
  skos:broader bigg:HVACAndHotWaterMeasure.HeatingSystemMeasure.HeatingDistributionAndStorageMeasure .

bigg:HVACAndHotWaterMeasure.HeatingSystemMeasure.HeatingDistributionAndStorageMeasure.HeatingPipesInsulation
  a bigg:EnergyEfficiencyMeasureType, skos:Concept;
  rdfs:comment "Improvement of the insulation of the pipes";
  skos:broader bigg:HVACAndHotWaterMeasure.HeatingSystemMeasure.HeatingDistributionAndStorageMeasure .

bigg:HVACAndHotWaterMeasure.HeatingSystemMeasure.HeatingDistributionAndStorageMeasure.HeatingDuctsSubstitution
  a bigg:EnergyEfficiencyMeasureType, skos:Concept;
  rdfs:comment "Substitution of the ducts";
  skos:broader bigg:HVACAndHotWaterMeasure.HeatingSystemMeasure.HeatingDistributionAndStorageMeasure .

bigg:HVACAndHotWaterMeasure.HeatingSystemMeasure.HeatingDistributionAndStorageMeasure.HeatingDuctsInsulation
  a bigg:EnergyEfficiencyMeasureType, skos:Concept;
  rdfs:comment "Improvement of the insulation of the ducts";
  skos:broader bigg:HVACAndHotWaterMeasure.HeatingSystemMeasure.HeatingDistributionAndStorageMeasure .

bigg:HVACAndHotWaterMeasure.HeatingSystemMeasure.HeatingDistributionAndStorageMeasure.HeatingStorageTankInstallation
  a bigg:EnergyEfficiencyMeasureType, skos:Concept;
  rdfs:comment "Installation or substitution of the hot water storage tank";
  skos:broader bigg:HVACAndHotWaterMeasure.HeatingSystemMeasure.HeatingDistributionAndStorageMeasure .

bigg:HVACAndHotWaterMeasure.HeatingSystemMeasure.HeatingDistributionAndStorageMeasure.HeatingStorageTankInsulation
  a bigg:EnergyEfficiencyMeasureType, skos:Concept;
  rdfs:comment "Improvement of the insulation of the hot water storage tank";
  skos:broader bigg:HVACAndHotWaterMeasure.HeatingSystemMeasure.HeatingDistributionAndStorageMeasure .

bigg:HVACAndHotWaterMeasure.HeatingSystemMeasure.HeatingDistributionAndStorageMeasure.OtherDistributionAndStorageMeasure
  a bigg:EnergyEfficiencyMeasureType, skos:Concept;
  rdfs:comment "Other measure on the heating distribution or storage systems";
  skos:broader bigg:HVACAndHotWaterMeasure.HeatingSystemMeasure.HeatingDistributionAndStorageMeasure .

bigg:HVACAndHotWaterMeasure.HeatingSystemMeasure.HeatingFinalElementsMeasure a bigg:EnergyEfficiencyMeasureType,
    skos:Concept;
  rdfs:comment "Measure that affects the heating system final elements (eg. radiators)";
  skos:broader bigg:HVACAndHotWaterMeasure.HeatingSystemMeasure .

bigg:HVACAndHotWaterMeasure.HeatingSystemMeasure.HeatingFinalElementsMeasure.HeatingFinalElementsReplacement
  a bigg:EnergyEfficiencyMeasureType, skos:Concept;
  rdfs:comment "Replacement of the final elements of the heating system";
  skos:broader bigg:HVACAndHotWaterMeasure.HeatingSystemMeasure.HeatingFinalElementsMeasure .

bigg:HVACAndHotWaterMeasure.HeatingSystemMeasure.HeatingFinalElementsMeasure.HeatingFinalElementsRelocation
  a bigg:EnergyEfficiencyMeasureType, skos:Concept;
  rdfs:comment "Change of the location of the final elements of the heating system";
  skos:broader bigg:HVACAndHotWaterMeasure.HeatingSystemMeasure.HeatingFinalElementsMeasure .

bigg:HVACAndHotWaterMeasure.HeatingSystemMeasure.HeatingFinalElementsMeasure.HeatingUnderfloorInstallation
  a bigg:EnergyEfficiencyMeasureType, skos:Concept;
  rdfs:comment "Installation of an underfloor heating system ";
  skos:broader bigg:HVACAndHotWaterMeasure.HeatingSystemMeasure.HeatingFinalElementsMeasure .

bigg:HVACAndHotWaterMeasure.HeatingSystemMeasure.HeatingFinalElementsMeasure.OtherHeatingFinalElementsMeasure
  a bigg:EnergyEfficiencyMeasureType, skos:Concept;
  rdfs:comment "Other measure on the final elements of the hating system";
  skos:broader bigg:HVACAndHotWaterMeasure.HeatingSystemMeasure.HeatingFinalElementsMeasure .

bigg:HVACAndHotWaterMeasure.HeatingSystemMeasure.HeatingControlMeasure a bigg:EnergyEfficiencyMeasureType,
    skos:Concept;
  rdfs:comment "Measure that affects the automation and controls of the heating system";
  skos:broader bigg:HVACAndHotWaterMeasure.HeatingSystemMeasure .

bigg:HVACAndHotWaterMeasure.HeatingSystemMeasure.HeatingControlMeasure.HeatingStopStartOptimization
  a bigg:EnergyEfficiencyMeasureType, skos:Concept;
  rdfs:comment "Implementation of a control to optimize the start/stop of the heating system to reach the temperature setpoint ";
  skos:broader bigg:HVACAndHotWaterMeasure.HeatingSystemMeasure.HeatingControlMeasure .

bigg:HVACAndHotWaterMeasure.HeatingSystemMeasure.HeatingControlMeasure.HeatingTimeControlImplementation
  a bigg:EnergyEfficiencyMeasureType, skos:Concept;
  rdfs:comment "Installation of a timer to control the turn on/off of the heating system";
  skos:broader bigg:HVACAndHotWaterMeasure.HeatingSystemMeasure.HeatingControlMeasure .

bigg:HVACAndHotWaterMeasure.HeatingSystemMeasure.HeatingControlMeasure.HeatingTemperatureSensorInstallation
  a bigg:EnergyEfficiencyMeasureType, skos:Concept;
  rdfs:comment "Installation of temperature sensors to control the turn on/off of the heating system";
  skos:broader bigg:HVACAndHotWaterMeasure.HeatingSystemMeasure.HeatingControlMeasure .

bigg:HVACAndHotWaterMeasure.HeatingSystemMeasure.HeatingControlMeasure.HeatingThermostaticValvesInstallation
  a bigg:EnergyEfficiencyMeasureType, skos:Concept;
  rdfs:comment "Installation of thermostatic valves to the final elements of the heating system";
  skos:broader bigg:HVACAndHotWaterMeasure.HeatingSystemMeasure.HeatingControlMeasure .

bigg:HVACAndHotWaterMeasure.HeatingSystemMeasure.HeatingControlMeasure.HeatingThermostatInstallation
  a bigg:EnergyEfficiencyMeasureType, skos:Concept;
  rdfs:comment "Installation of a thermostat for the control of the heating system";
  skos:broader bigg:HVACAndHotWaterMeasure.HeatingSystemMeasure.HeatingControlMeasure .

bigg:HVACAndHotWaterMeasure.HeatingSystemMeasure.HeatingControlMeasure.OtherHeatingControlMeasure
  a bigg:EnergyEfficiencyMeasureType, skos:Concept;
  rdfs:comment "Other measure for the control and automation of the heating system";
  skos:broader bigg:HVACAndHotWaterMeasure.HeatingSystemMeasure.HeatingControlMeasure .

bigg:HVACAndHotWaterMeasure.CombinedHeatingCoolingSystemMeasure a bigg:EnergyEfficiencyMeasureType,
    skos:Concept;
  rdfs:comment "Measure with a combined effect on the space heating and cooling systems of the building";
  skos:broader bigg:HVACAndHotWaterMeasure .

bigg:HVACAndHotWaterMeasure.CombinedHeatingCoolingSystemMeasure.HeatAndCoolProductionMeasure
  a bigg:EnergyEfficiencyMeasureType, skos:Concept;
  rdfs:comment "Measure that affects the heat/cool production equipment of a combined heating/cooling system";
  skos:broader bigg:HVACAndHotWaterMeasure.CombinedHeatingCoolingSystemMeasure .

bigg:HVACAndHotWaterMeasure.CombinedHeatingCoolingSystemMeasure.HeatAndCoolProductionMeasure.HeatAndCoolHeatPumpReplacement
  a bigg:EnergyEfficiencyMeasureType, skos:Concept;
  rdfs:comment "Replacement of the heat pump with a more efficient one";
  skos:broader bigg:HVACAndHotWaterMeasure.CombinedHeatingCoolingSystemMeasure.HeatAndCoolProductionMeasure .

bigg:HVACAndHotWaterMeasure.CombinedHeatingCoolingSystemMeasure.HeatAndCoolProductionMeasure.HeatAndCoolProductionFuelConversion
  a bigg:EnergyEfficiencyMeasureType, skos:Concept;
  rdfs:comment "Replacement of the system with one that operates with a different fuel source ";
  skos:broader bigg:HVACAndHotWaterMeasure.CombinedHeatingCoolingSystemMeasure.HeatAndCoolProductionMeasure .

bigg:HVACAndHotWaterMeasure.CombinedHeatingCoolingSystemMeasure.HeatAndCoolProductionMeasure.HeatAndCoolHeatExchangersReplacement
  a bigg:EnergyEfficiencyMeasureType, skos:Concept;
  rdfs:comment "Replacement of heat exchangers ";
  skos:broader bigg:HVACAndHotWaterMeasure.CombinedHeatingCoolingSystemMeasure.HeatAndCoolProductionMeasure .

bigg:HVACAndHotWaterMeasure.CombinedHeatingCoolingSystemMeasure.HeatAndCoolProductionMeasure.HeatAndCoolCompressorReplacement
  a bigg:EnergyEfficiencyMeasureType, skos:Concept;
  rdfs:comment "Replacement of the compressor";
  skos:broader bigg:HVACAndHotWaterMeasure.CombinedHeatingCoolingSystemMeasure.HeatAndCoolProductionMeasure .

bigg:HVACAndHotWaterMeasure.CombinedHeatingCoolingSystemMeasure.HeatAndCoolProductionMeasure.HeatingAndCoolingOtherElementReplacement
  a bigg:EnergyEfficiencyMeasureType, skos:Concept;
  rdfs:comment "Change of another single component in the heat/cool production subsystem";
  skos:broader bigg:HVACAndHotWaterMeasure.CombinedHeatingCoolingSystemMeasure.HeatAndCoolProductionMeasure .

bigg:HVACAndHotWaterMeasure.CombinedHeatingCoolingSystemMeasure.HeatAndCoolProductionMeasure.HeatAndCoolProductionSystemInsulation
  a bigg:EnergyEfficiencyMeasureType, skos:Concept;
  rdfs:comment "Improvement of the heat/cool production elements insulation";
  skos:broader bigg:HVACAndHotWaterMeasure.CombinedHeatingCoolingSystemMeasure.HeatAndCoolProductionMeasure .

bigg:HVACAndHotWaterMeasure.CombinedHeatingCoolingSystemMeasure.HeatAndCoolProductionMeasure.DistrictCombinedHeatingAndCoolingConnection
  a bigg:EnergyEfficiencyMeasureType, skos:Concept;
  rdfs:comment "Connection of the building space heating and cooling system to district heating and cooling";
  skos:broader bigg:HVACAndHotWaterMeasure.CombinedHeatingCoolingSystemMeasure.HeatAndCoolProductionMeasure .

bigg:HVACAndHotWaterMeasure.CombinedHeatingCoolingSystemMeasure.HeatAndCoolProductionMeasure.OtherHeatAndCoolProductionMeasure
  a bigg:EnergyEfficiencyMeasureType, skos:Concept;
  rdfs:comment "Other measure on the heat/cool production system";
  skos:broader bigg:HVACAndHotWaterMeasure.CombinedHeatingCoolingSystemMeasure.HeatAndCoolProductionMeasure .

bigg:HVACAndHotWaterMeasure.CombinedHeatingCoolingSystemMeasure.HeatingAndCoolingDistributionMeasure
  a bigg:EnergyEfficiencyMeasureType, skos:Concept;
  rdfs:comment "Measure that affects the space heating and cooling distribution subsystem";
  skos:broader bigg:HVACAndHotWaterMeasure.CombinedHeatingCoolingSystemMeasure .

bigg:HVACAndHotWaterMeasure.CombinedHeatingCoolingSystemMeasure.HeatingAndCoolingDistributionMeasure.HeatingAndCoolingDistributionSystemReplacement
  a bigg:EnergyEfficiencyMeasureType, skos:Concept;
  rdfs:comment "Complete change of the heating and cooling distribution system ";
  skos:broader bigg:HVACAndHotWaterMeasure.CombinedHeatingCoolingSystemMeasure.HeatingAndCoolingDistributionMeasure .

bigg:HVACAndHotWaterMeasure.CombinedHeatingCoolingSystemMeasure.HeatingAndCoolingDistributionMeasure.HeatingAndCoolingDistributionPumpReplacement
  a bigg:EnergyEfficiencyMeasureType, skos:Concept;
  rdfs:comment "Replacement of a pump";
  skos:broader bigg:HVACAndHotWaterMeasure.CombinedHeatingCoolingSystemMeasure.HeatingAndCoolingDistributionMeasure .

bigg:HVACAndHotWaterMeasure.CombinedHeatingCoolingSystemMeasure.HeatingAndCoolingDistributionMeasure.HeatingAndCoolingDistributionFanReplacement
  a bigg:EnergyEfficiencyMeasureType, skos:Concept;
  rdfs:comment "Replacement of a fan";
  skos:broader bigg:HVACAndHotWaterMeasure.CombinedHeatingCoolingSystemMeasure.HeatingAndCoolingDistributionMeasure .

bigg:HVACAndHotWaterMeasure.CombinedHeatingCoolingSystemMeasure.HeatingAndCoolingDistributionMeasure.HeatingAndCoolingDistibutionVariableSpeedDrivesInstallation
  a bigg:EnergyEfficiencyMeasureType, skos:Concept;
  rdfs:comment "Installation of variable speed drives for the control of heating/cooling distribution elements (eg. pumps, fans,…)";
  skos:broader bigg:HVACAndHotWaterMeasure.CombinedHeatingCoolingSystemMeasure.HeatingAndCoolingDistributionMeasure .

bigg:HVACAndHotWaterMeasure.CombinedHeatingCoolingSystemMeasure.HeatingAndCoolingDistributionMeasure.HeatingAndCoolingDistributionOtherComponentReplacement
  a bigg:EnergyEfficiencyMeasureType, skos:Concept;
  rdfs:comment "Replacement or installation of other distribution elements (eg. valves or filters)";
  skos:broader bigg:HVACAndHotWaterMeasure.CombinedHeatingCoolingSystemMeasure.HeatingAndCoolingDistributionMeasure .

bigg:HVACAndHotWaterMeasure.CombinedHeatingCoolingSystemMeasure.HeatingAndCoolingDistributionMeasure.HeatingAndCoolingDistributionBalancingAndFlowRegulation
  a bigg:EnergyEfficiencyMeasureType, skos:Concept;
  rdfs:comment "Optimization of the heating/cooling distribution through regulation of the water/airflow (eg. by means of balancing valves or dampers) ";
  skos:broader bigg:HVACAndHotWaterMeasure.CombinedHeatingCoolingSystemMeasure.HeatingAndCoolingDistributionMeasure .

bigg:HVACAndHotWaterMeasure.CombinedHeatingCoolingSystemMeasure.HeatingAndCoolingDistributionMeasure.HeatingAndCoolingPipesSubstitution
  a bigg:EnergyEfficiencyMeasureType, skos:Concept;
  rdfs:comment "Substitution of the pipes";
  skos:broader bigg:HVACAndHotWaterMeasure.CombinedHeatingCoolingSystemMeasure.HeatingAndCoolingDistributionMeasure .

bigg:HVACAndHotWaterMeasure.CombinedHeatingCoolingSystemMeasure.HeatingAndCoolingDistributionMeasure.HeatingAndCoolingPipesInsulation
  a bigg:EnergyEfficiencyMeasureType, skos:Concept;
  rdfs:comment "Improvement of the insulation of the pipes";
  skos:broader bigg:HVACAndHotWaterMeasure.CombinedHeatingCoolingSystemMeasure.HeatingAndCoolingDistributionMeasure .

bigg:HVACAndHotWaterMeasure.CombinedHeatingCoolingSystemMeasure.HeatingAndCoolingDistributionMeasure.HeatingAndCoolingDuctsSubstitution
  a bigg:EnergyEfficiencyMeasureType, skos:Concept;
  rdfs:comment "Substitution of the ducts";
  skos:broader bigg:HVACAndHotWaterMeasure.CombinedHeatingCoolingSystemMeasure.HeatingAndCoolingDistributionMeasure .

bigg:HVACAndHotWaterMeasure.CombinedHeatingCoolingSystemMeasure.HeatingAndCoolingDistributionMeasure.HeatingAndCoolingDuctsInsulation
  a bigg:EnergyEfficiencyMeasureType, skos:Concept;
  rdfs:comment "Improvement of the insulation of the ducts";
  skos:broader bigg:HVACAndHotWaterMeasure.CombinedHeatingCoolingSystemMeasure.HeatingAndCoolingDistributionMeasure .

bigg:HVACAndHotWaterMeasure.CombinedHeatingCoolingSystemMeasure.HeatingAndCoolingDistributionMeasure.OtherHeatingAndCoolingDistributionMeasure
  a bigg:EnergyEfficiencyMeasureType, skos:Concept;
  rdfs:comment "Other measure on the heating and cooling distribution system";
  skos:broader bigg:HVACAndHotWaterMeasure.CombinedHeatingCoolingSystemMeasure.HeatingAndCoolingDistributionMeasure .

bigg:HVACAndHotWaterMeasure.CombinedHeatingCoolingSystemMeasure.HeatingAndCoolingFinalElementsMeasure
  a bigg:EnergyEfficiencyMeasureType, skos:Concept;
  rdfs:comment "Measure that affects the heating and cooling system final elements (eg. convectors)";
  skos:broader bigg:HVACAndHotWaterMeasure.CombinedHeatingCoolingSystemMeasure .

bigg:HVACAndHotWaterMeasure.CombinedHeatingCoolingSystemMeasure.HeatingAndCoolingFinalElementsMeasure.HeatingAndCoolingFinalElementsReplacement
  a bigg:EnergyEfficiencyMeasureType, skos:Concept;
  rdfs:comment "Replacement of the final elements of the heating and cooling system";
  skos:broader bigg:HVACAndHotWaterMeasure.CombinedHeatingCoolingSystemMeasure.HeatingAndCoolingFinalElementsMeasure .

bigg:HVACAndHotWaterMeasure.CombinedHeatingCoolingSystemMeasure.HeatingAndCoolingFinalElementsMeasure.HeatingAndCoolingFinalElementsRelocation
  a bigg:EnergyEfficiencyMeasureType, skos:Concept;
  rdfs:comment "Change of the location of the final elements of the heating and cooling system";
  skos:broader bigg:HVACAndHotWaterMeasure.CombinedHeatingCoolingSystemMeasure.HeatingAndCoolingFinalElementsMeasure .

bigg:HVACAndHotWaterMeasure.CombinedHeatingCoolingSystemMeasure.HeatingAndCoolingFinalElementsMeasure.HeatingAndCoolingUnderfloorInstallation
  a bigg:EnergyEfficiencyMeasureType, skos:Concept;
  rdfs:comment "Installation of an underfloor heating/cooling system ";
  skos:broader bigg:HVACAndHotWaterMeasure.CombinedHeatingCoolingSystemMeasure.HeatingAndCoolingFinalElementsMeasure .

bigg:HVACAndHotWaterMeasure.CombinedHeatingCoolingSystemMeasure.HeatingAndCoolingFinalElementsMeasure.OtherHeatingAndCoolingFinalElementsMeasure
  a bigg:EnergyEfficiencyMeasureType, skos:Concept;
  rdfs:comment "Other measure on the final elements of the heating/cooling system";
  skos:broader bigg:HVACAndHotWaterMeasure.CombinedHeatingCoolingSystemMeasure.HeatingAndCoolingFinalElementsMeasure .

bigg:HVACAndHotWaterMeasure.CombinedHeatingCoolingSystemMeasure.HeatingAndCoolingControlMeasure
  a bigg:EnergyEfficiencyMeasureType, skos:Concept;
  rdfs:comment "Measure that affects the automation and controls of the heating/cooling system";
  skos:broader bigg:HVACAndHotWaterMeasure.CombinedHeatingCoolingSystemMeasure .

bigg:HVACAndHotWaterMeasure.CombinedHeatingCoolingSystemMeasure.HeatingAndCoolingControlMeasure.HeatingAndCoolingTemperatureSensorInstallation
  a bigg:EnergyEfficiencyMeasureType, skos:Concept;
  rdfs:comment "Installation of temperature sensors to control the turn on/off of the heating and cooling system";
  skos:broader bigg:HVACAndHotWaterMeasure.CombinedHeatingCoolingSystemMeasure.HeatingAndCoolingControlMeasure .

bigg:HVACAndHotWaterMeasure.CombinedHeatingCoolingSystemMeasure.HeatingAndCoolingControlMeasure.HeatingAndCoolingThermostatInstallation
  a bigg:EnergyEfficiencyMeasureType, skos:Concept;
  rdfs:comment "Installation of thermostatic valves to the final elements of the heating and cooling system";
  skos:broader bigg:HVACAndHotWaterMeasure.CombinedHeatingCoolingSystemMeasure.HeatingAndCoolingControlMeasure .

bigg:HVACAndHotWaterMeasure.CombinedHeatingCoolingSystemMeasure.HeatingAndCoolingControlMeasure.OtherHeatingAndCoolingControlMeasure
  a bigg:EnergyEfficiencyMeasureType, skos:Concept;
  rdfs:comment "Other measure for the control and automation of the heating and cooling system";
  skos:broader bigg:HVACAndHotWaterMeasure.CombinedHeatingCoolingSystemMeasure.HeatingAndCoolingControlMeasure .

bigg:HVACAndHotWaterMeasure.CoolingSystemMeasure a bigg:EnergyEfficiencyMeasureType,
    skos:Concept;
  rdfs:comment "Measure that only affects the space cooling system of the building";
  skos:broader bigg:HVACAndHotWaterMeasure .

bigg:HVACAndHotWaterMeasure.CoolingSystemMeasure.CoolProductionMeasure a bigg:EnergyEfficiencyMeasureType,
    skos:Concept;
  rdfs:comment "Measure that affects the cooling production subsystem of space cooling";
  skos:broader bigg:HVACAndHotWaterMeasure.CoolingSystemMeasure .

bigg:HVACAndHotWaterMeasure.CoolingSystemMeasure.CoolProductionMeasure.CoolingHeatPumpReplacement
  a bigg:EnergyEfficiencyMeasureType, skos:Concept;
  rdfs:comment "Replacement of the heat pump with a more efficient one";
  skos:broader bigg:HVACAndHotWaterMeasure.CoolingSystemMeasure.CoolProductionMeasure .

bigg:HVACAndHotWaterMeasure.CoolingSystemMeasure.CoolProductionMeasure.CoolingChillerReplacement
  a bigg:EnergyEfficiencyMeasureType, skos:Concept;
  rdfs:comment "Replacement of the chiller with a more efficient one";
  skos:broader bigg:HVACAndHotWaterMeasure.CoolingSystemMeasure.CoolProductionMeasure .

bigg:HVACAndHotWaterMeasure.CoolingSystemMeasure.CoolProductionMeasure.CoolingHeatExchangerReplacement
  a bigg:EnergyEfficiencyMeasureType, skos:Concept;
  rdfs:comment "Replacement of heat exchangers ";
  skos:broader bigg:HVACAndHotWaterMeasure.CoolingSystemMeasure.CoolProductionMeasure .

bigg:HVACAndHotWaterMeasure.CoolingSystemMeasure.CoolProductionMeasure.CoolingCompressorReplacement
  a bigg:EnergyEfficiencyMeasureType, skos:Concept;
  rdfs:comment "Replacement of the compressor";
  skos:broader bigg:HVACAndHotWaterMeasure.CoolingSystemMeasure.CoolProductionMeasure .

bigg:HVACAndHotWaterMeasure.CoolingSystemMeasure.CoolProductionMeasure.CoolingOtherElementReplacement
  a bigg:EnergyEfficiencyMeasureType, skos:Concept;
  rdfs:comment "Change of another single component in the cooling production system";
  skos:broader bigg:HVACAndHotWaterMeasure.CoolingSystemMeasure.CoolProductionMeasure .

bigg:HVACAndHotWaterMeasure.CoolingSystemMeasure.CoolProductionMeasure.CoolingProductionSystemInsulation
  a bigg:EnergyEfficiencyMeasureType, skos:Concept;
  rdfs:comment "Improvement of the cooling production elements insulation";
  skos:broader bigg:HVACAndHotWaterMeasure.CoolingSystemMeasure.CoolProductionMeasure .

bigg:HVACAndHotWaterMeasure.CoolingSystemMeasure.CoolProductionMeasure.DistrictCoolingConnection
  a bigg:EnergyEfficiencyMeasureType, skos:Concept;
  rdfs:comment "Connection of the building space heating system to district heating";
  skos:broader bigg:HVACAndHotWaterMeasure.CoolingSystemMeasure.CoolProductionMeasure .

bigg:HVACAndHotWaterMeasure.CoolingSystemMeasure.CoolProductionMeasure.OtherCoolProductionMeasure
  a bigg:EnergyEfficiencyMeasureType, skos:Concept;
  rdfs:comment "Other measure on the cooling production system";
  skos:broader bigg:HVACAndHotWaterMeasure.CoolingSystemMeasure.CoolProductionMeasure .

bigg:HVACAndHotWaterMeasure.CoolingSystemMeasure.CoolingDistributionAndStorageMeasure
  a bigg:EnergyEfficiencyMeasureType, skos:Concept;
  rdfs:comment "Measure that affects the distribution or the storage subsystems of space cooling ";
  skos:broader bigg:HVACAndHotWaterMeasure.CoolingSystemMeasure .

bigg:HVACAndHotWaterMeasure.CoolingSystemMeasure.CoolingDistributionAndStorageMeasure.CoolingDistributionSystemReplacement
  a bigg:EnergyEfficiencyMeasureType, skos:Concept;
  rdfs:comment "Complete change of the cooling distribution system ";
  skos:broader bigg:HVACAndHotWaterMeasure.CoolingSystemMeasure.CoolingDistributionAndStorageMeasure .

bigg:HVACAndHotWaterMeasure.CoolingSystemMeasure.CoolingDistributionAndStorageMeasure.CoolingDistributionPumpReplacement
  a bigg:EnergyEfficiencyMeasureType, skos:Concept;
  rdfs:comment "Replacement of a pump";
  skos:broader bigg:HVACAndHotWaterMeasure.CoolingSystemMeasure.CoolingDistributionAndStorageMeasure .

bigg:HVACAndHotWaterMeasure.CoolingSystemMeasure.CoolingDistributionAndStorageMeasure.CoolingDistributionFanReplacement
  a bigg:EnergyEfficiencyMeasureType, skos:Concept;
  rdfs:comment "Replacement of a fan";
  skos:broader bigg:HVACAndHotWaterMeasure.CoolingSystemMeasure.CoolingDistributionAndStorageMeasure .

bigg:HVACAndHotWaterMeasure.CoolingSystemMeasure.CoolingDistributionAndStorageMeasure.CoolingDistibutionVariableSpeedDrivesInstallation
  a bigg:EnergyEfficiencyMeasureType, skos:Concept;
  rdfs:comment "Installation of variable speed drives for the control of cooling distribution elements (eg. pumps, fans,…)";
  skos:broader bigg:HVACAndHotWaterMeasure.CoolingSystemMeasure.CoolingDistributionAndStorageMeasure .

bigg:HVACAndHotWaterMeasure.CoolingSystemMeasure.CoolingDistributionAndStorageMeasure.CoolingDistributionOtherComponentReplacement
  a bigg:EnergyEfficiencyMeasureType, skos:Concept;
  rdfs:comment "Replacement or installation of other distribution elements (eg. valves or filters)";
  skos:broader bigg:HVACAndHotWaterMeasure.CoolingSystemMeasure.CoolingDistributionAndStorageMeasure .

bigg:HVACAndHotWaterMeasure.CoolingSystemMeasure.CoolingDistributionAndStorageMeasure.CoolingDistributionBalancingAndFlowRegulation
  a bigg:EnergyEfficiencyMeasureType, skos:Concept;
  rdfs:comment "Optimization of the cooling distribution through regulation of the water/airflow (eg. by means of balancing valves or dampers) ";
  skos:broader bigg:HVACAndHotWaterMeasure.CoolingSystemMeasure.CoolingDistributionAndStorageMeasure .

bigg:HVACAndHotWaterMeasure.CoolingSystemMeasure.CoolingDistributionAndStorageMeasure.CoolingPipesSubstitution
  a bigg:EnergyEfficiencyMeasureType, skos:Concept;
  rdfs:comment "Substitution of the pipes";
  skos:broader bigg:HVACAndHotWaterMeasure.CoolingSystemMeasure.CoolingDistributionAndStorageMeasure .

bigg:HVACAndHotWaterMeasure.CoolingSystemMeasure.CoolingDistributionAndStorageMeasure.CoolingPipesInsulation
  a bigg:EnergyEfficiencyMeasureType, skos:Concept;
  rdfs:comment "Improvement of the insulation of the pipes";
  skos:broader bigg:HVACAndHotWaterMeasure.CoolingSystemMeasure.CoolingDistributionAndStorageMeasure .

bigg:HVACAndHotWaterMeasure.CoolingSystemMeasure.CoolingDistributionAndStorageMeasure.CoolingDuctsSubstitution
  a bigg:EnergyEfficiencyMeasureType, skos:Concept;
  rdfs:comment "Substitution of the ducts";
  skos:broader bigg:HVACAndHotWaterMeasure.CoolingSystemMeasure.CoolingDistributionAndStorageMeasure .

bigg:HVACAndHotWaterMeasure.CoolingSystemMeasure.CoolingDistributionAndStorageMeasure.CoolingDuctsInsulation
  a bigg:EnergyEfficiencyMeasureType, skos:Concept;
  rdfs:comment "Improvement of the insulation of the ducts";
  skos:broader bigg:HVACAndHotWaterMeasure.CoolingSystemMeasure.CoolingDistributionAndStorageMeasure .

bigg:HVACAndHotWaterMeasure.CoolingSystemMeasure.CoolingDistributionAndStorageMeasure.CoolingStorageTankInstallation
  a bigg:EnergyEfficiencyMeasureType, skos:Concept;
  rdfs:comment "Installation or substitution of the cold water storage tank";
  skos:broader bigg:HVACAndHotWaterMeasure.CoolingSystemMeasure.CoolingDistributionAndStorageMeasure .

bigg:HVACAndHotWaterMeasure.CoolingSystemMeasure.CoolingDistributionAndStorageMeasure.CoolingStorageTankInsulation
  a bigg:EnergyEfficiencyMeasureType, skos:Concept;
  rdfs:comment "Improvement of the insulation of the cold water storage tank";
  skos:broader bigg:HVACAndHotWaterMeasure.CoolingSystemMeasure.CoolingDistributionAndStorageMeasure .

bigg:HVACAndHotWaterMeasure.CoolingSystemMeasure.CoolingDistributionAndStorageMeasure.OtherCoolingDistributionAndStorageMeasure
  a bigg:EnergyEfficiencyMeasureType, skos:Concept;
  rdfs:comment "Other measure on the cooling distribution or storage systems";
  skos:broader bigg:HVACAndHotWaterMeasure.CoolingSystemMeasure.CoolingDistributionAndStorageMeasure .

bigg:HVACAndHotWaterMeasure.CoolingSystemMeasure.CoolingFinalElementsMeasure a bigg:EnergyEfficiencyMeasureType,
    skos:Concept;
  rdfs:comment "Measure that affects the final elements used for space cooling (eg. fans, convectors, ...)";
  skos:broader bigg:HVACAndHotWaterMeasure.CoolingSystemMeasure .

bigg:HVACAndHotWaterMeasure.CoolingSystemMeasure.CoolingFinalElementsMeasure.CoolingFinalElementsReplacement
  a bigg:EnergyEfficiencyMeasureType, skos:Concept;
  rdfs:comment "Replacement of the final elements of the cooling system";
  skos:broader bigg:HVACAndHotWaterMeasure.CoolingSystemMeasure.CoolingFinalElementsMeasure .

bigg:HVACAndHotWaterMeasure.CoolingSystemMeasure.CoolingFinalElementsMeasure.CoolingFinalElementsRelocation
  a bigg:EnergyEfficiencyMeasureType, skos:Concept;
  rdfs:comment "Change of the location of the final elements of the cooling system";
  skos:broader bigg:HVACAndHotWaterMeasure.CoolingSystemMeasure.CoolingFinalElementsMeasure .

bigg:HVACAndHotWaterMeasure.CoolingSystemMeasure.CoolingFinalElementsMeasure.CoolingUnderfloorInstallation
  a bigg:EnergyEfficiencyMeasureType, skos:Concept;
  rdfs:comment "Installation of an underfloor cooling system ";
  skos:broader bigg:HVACAndHotWaterMeasure.CoolingSystemMeasure.CoolingFinalElementsMeasure .

bigg:HVACAndHotWaterMeasure.CoolingSystemMeasure.CoolingFinalElementsMeasure.OtherCoolingFinalElementsMeasure
  a bigg:EnergyEfficiencyMeasureType, skos:Concept;
  rdfs:comment "Other measure on the final elements of the cooling system";
  skos:broader bigg:HVACAndHotWaterMeasure.CoolingSystemMeasure.CoolingFinalElementsMeasure .

bigg:HVACAndHotWaterMeasure.CoolingSystemMeasure.CoolingControlMeasure a bigg:EnergyEfficiencyMeasureType,
    skos:Concept;
  rdfs:comment "Measure that affects the automation and controls of the cooling system";
  skos:broader bigg:HVACAndHotWaterMeasure.CoolingSystemMeasure .

bigg:HVACAndHotWaterMeasure.CoolingSystemMeasure.CoolingControlMeasure.CoolingStopStartOptimization
  a bigg:EnergyEfficiencyMeasureType, skos:Concept;
  rdfs:comment "Implementation of a control to optimize the start/stop of the cooling system to reach the temperature setpoint ";
  skos:broader bigg:HVACAndHotWaterMeasure.CoolingSystemMeasure.CoolingControlMeasure .

bigg:HVACAndHotWaterMeasure.CoolingSystemMeasure.CoolingControlMeasure.CoolingTimeControl
  a bigg:EnergyEfficiencyMeasureType, skos:Concept;
  rdfs:comment "Installation of a timer to control the turn on/off of the cooling system";
  skos:broader bigg:HVACAndHotWaterMeasure.CoolingSystemMeasure.CoolingControlMeasure .

bigg:HVACAndHotWaterMeasure.CoolingSystemMeasure.CoolingControlMeasure.CoolingTemperatureSensorInstallation
  a bigg:EnergyEfficiencyMeasureType, skos:Concept;
  rdfs:comment "Installation of temperature sensors to control the turn on/off of the cooling system";
  skos:broader bigg:HVACAndHotWaterMeasure.CoolingSystemMeasure.CoolingControlMeasure .

bigg:HVACAndHotWaterMeasure.CoolingSystemMeasure.CoolingControlMeasure.CoolingThermostatInstallation
  a bigg:EnergyEfficiencyMeasureType, skos:Concept;
  rdfs:comment "Installation of a thermostat for the control of the cooling system";
  skos:broader bigg:HVACAndHotWaterMeasure.CoolingSystemMeasure.CoolingControlMeasure .

bigg:HVACAndHotWaterMeasure.CoolingSystemMeasure.CoolingControlMeasure.OtherCoolingControlMeasure
  a bigg:EnergyEfficiencyMeasureType, skos:Concept;
  rdfs:comment "Other measure for the control and automation of the cooling system";
  skos:broader bigg:HVACAndHotWaterMeasure.CoolingSystemMeasure.CoolingControlMeasure .

bigg:HVACAndHotWaterMeasure.HotWaterSystemMeasure a bigg:EnergyEfficiencyMeasureType,
    skos:Concept;
  rdfs:comment "Measure that only affects the water heating system of the building";
  skos:broader bigg:HVACAndHotWaterMeasure .

bigg:HVACAndHotWaterMeasure.HotWaterSystemMeasure.HotWaterProductionMeasure a bigg:EnergyEfficiencyMeasureType,
    skos:Concept;
  rdfs:comment "Measure that affects the heat production subsystem of space heating";
  skos:broader bigg:HVACAndHotWaterMeasure.HotWaterSystemMeasure .

bigg:HVACAndHotWaterMeasure.HotWaterSystemMeasure.HotWaterProductionMeasure.HotWaterBoilerReplacement
  a bigg:EnergyEfficiencyMeasureType, skos:Concept;
  rdfs:comment "Replacement of the boiler with a more efficient one that uses the same fuel";
  skos:broader bigg:HVACAndHotWaterMeasure.HotWaterSystemMeasure.HotWaterProductionMeasure .

bigg:HVACAndHotWaterMeasure.HotWaterSystemMeasure.HotWaterProductionMeasure.HotWaterHeatPumpReplacement
  a bigg:EnergyEfficiencyMeasureType, skos:Concept;
  rdfs:comment "Replacement of the heat pump with a more efficient one";
  skos:broader bigg:HVACAndHotWaterMeasure.HotWaterSystemMeasure.HotWaterProductionMeasure .

bigg:HVACAndHotWaterMeasure.HotWaterSystemMeasure.HotWaterProductionMeasure.HotWaterProductionFuelConversion
  a bigg:EnergyEfficiencyMeasureType, skos:Concept;
  rdfs:comment "Replacement of the heat production system with one that operates with a different fuel source ";
  skos:broader bigg:HVACAndHotWaterMeasure.HotWaterSystemMeasure.HotWaterProductionMeasure .

bigg:HVACAndHotWaterMeasure.HotWaterSystemMeasure.HotWaterProductionMeasure.HotWaterHeatExchangersReplacement
  a bigg:EnergyEfficiencyMeasureType, skos:Concept;
  rdfs:comment "Replacement of heat exchangers ";
  skos:broader bigg:HVACAndHotWaterMeasure.HotWaterSystemMeasure.HotWaterProductionMeasure .

bigg:HVACAndHotWaterMeasure.HotWaterSystemMeasure.HotWaterProductionMeasure.HotWaterBurnerReplacement
  a bigg:EnergyEfficiencyMeasureType, skos:Concept;
  rdfs:comment "Replacement of the burner";
  skos:broader bigg:HVACAndHotWaterMeasure.HotWaterSystemMeasure.HotWaterProductionMeasure .

bigg:HVACAndHotWaterMeasure.HotWaterSystemMeasure.HotWaterProductionMeasure.HotWaterOtherElementReplacement
  a bigg:EnergyEfficiencyMeasureType, skos:Concept;
  rdfs:comment "Change of another single component in the hot water production system";
  skos:broader bigg:HVACAndHotWaterMeasure.HotWaterSystemMeasure.HotWaterProductionMeasure .

bigg:HVACAndHotWaterMeasure.HotWaterSystemMeasure.HotWaterProductionMeasure.HotWaterProductionSystemInsulation
  a bigg:EnergyEfficiencyMeasureType, skos:Concept;
  rdfs:comment "Improvement of the hot water production elements insulation";
  skos:broader bigg:HVACAndHotWaterMeasure.HotWaterSystemMeasure.HotWaterProductionMeasure .

bigg:HVACAndHotWaterMeasure.HotWaterSystemMeasure.HotWaterProductionMeasure.OtherHotWaterProductionMeasure
  a bigg:EnergyEfficiencyMeasureType, skos:Concept;
  rdfs:comment "Other measure on the hot water production system";
  skos:broader bigg:HVACAndHotWaterMeasure.HotWaterSystemMeasure.HotWaterProductionMeasure .

bigg:HVACAndHotWaterMeasure.HotWaterSystemMeasure.HotWaterDistributionAndStorageMeasure
  a bigg:EnergyEfficiencyMeasureType, skos:Concept;
  rdfs:comment "Measure that affects the distribution or the storage subsystems of water heating ";
  skos:broader bigg:HVACAndHotWaterMeasure.HotWaterSystemMeasure .

bigg:HVACAndHotWaterMeasure.HotWaterSystemMeasure.HotWaterDistributionAndStorageMeasure.HotWaterDistributionSystemReplacement
  a bigg:EnergyEfficiencyMeasureType, skos:Concept;
  rdfs:comment "Complete change of the hot water distribution system ";
  skos:broader bigg:HVACAndHotWaterMeasure.HotWaterSystemMeasure.HotWaterDistributionAndStorageMeasure .

bigg:HVACAndHotWaterMeasure.HotWaterSystemMeasure.HotWaterDistributionAndStorageMeasure.HotWaterDistributionPumpReplacement
  a bigg:EnergyEfficiencyMeasureType, skos:Concept;
  rdfs:comment "Replacement of a pump";
  skos:broader bigg:HVACAndHotWaterMeasure.HotWaterSystemMeasure.HotWaterDistributionAndStorageMeasure .

bigg:HVACAndHotWaterMeasure.HotWaterSystemMeasure.HotWaterDistributionAndStorageMeasure.HotWaterDistibutionVariableSpeedDrivesInstallation
  a bigg:EnergyEfficiencyMeasureType, skos:Concept;
  rdfs:comment "Installation of variable speed drives for the control of hot water distribution elements (eg. pumps)";
  skos:broader bigg:HVACAndHotWaterMeasure.HotWaterSystemMeasure.HotWaterDistributionAndStorageMeasure .

bigg:HVACAndHotWaterMeasure.HotWaterSystemMeasure.HotWaterDistributionAndStorageMeasure.HotWaterDistributionOtherComponentReplacement
  a bigg:EnergyEfficiencyMeasureType, skos:Concept;
  rdfs:comment "Replacement or installation of other distribution elements (eg. valves or filters)";
  skos:broader bigg:HVACAndHotWaterMeasure.HotWaterSystemMeasure.HotWaterDistributionAndStorageMeasure .

bigg:HVACAndHotWaterMeasure.HotWaterSystemMeasure.HotWaterDistributionAndStorageMeasure.HotWaterDistributionBalancingAndFlowRegulation
  a bigg:EnergyEfficiencyMeasureType, skos:Concept;
  rdfs:comment "Optimization of the hot water distribution through regulation of the water flow by means of balancing valves";
  skos:broader bigg:HVACAndHotWaterMeasure.HotWaterSystemMeasure.HotWaterDistributionAndStorageMeasure .

bigg:HVACAndHotWaterMeasure.HotWaterSystemMeasure.HotWaterDistributionAndStorageMeasure.HotWaterPipesSubstitution
  a bigg:EnergyEfficiencyMeasureType, skos:Concept;
  rdfs:comment "Substitution of the pipes";
  skos:broader bigg:HVACAndHotWaterMeasure.HotWaterSystemMeasure.HotWaterDistributionAndStorageMeasure .

bigg:HVACAndHotWaterMeasure.HotWaterSystemMeasure.HotWaterDistributionAndStorageMeasure.HotWaterPipesInsulation
  a bigg:EnergyEfficiencyMeasureType, skos:Concept;
  rdfs:comment "Improvement of the insulation of the pipes";
  skos:broader bigg:HVACAndHotWaterMeasure.HotWaterSystemMeasure.HotWaterDistributionAndStorageMeasure .

bigg:HVACAndHotWaterMeasure.HotWaterSystemMeasure.HotWaterDistributionAndStorageMeasure.HotWaterStorageTankInstallation
  a bigg:EnergyEfficiencyMeasureType, skos:Concept;
  rdfs:comment "Installation or substitution of the hot water storage tank";
  skos:broader bigg:HVACAndHotWaterMeasure.HotWaterSystemMeasure.HotWaterDistributionAndStorageMeasure .

bigg:HVACAndHotWaterMeasure a bigg:EnergyEfficiencyMeasureType, skos:Concept;
  rdfs:comment "Measure that affects the space heating, ventilation, air conditioning, or water heating system of the building" .

bigg:HVACAndHotWaterMeasure.HotWaterSystemMeasure a bigg:EnergyEfficiencyMeasureType,
    skos:Concept;
  rdfs:comment "Measure that only affects the water heating system of the building";
  skos:broader bigg:HVACAndHotWaterMeasure .

bigg:HVACAndHotWaterMeasure.HotWaterSystemMeasure.HotWaterDistributionAndStorageMeasure
  a bigg:EnergyEfficiencyMeasureType, skos:Concept;
  rdfs:comment "Measure that affects the distribution or the storage subsystems of water heating ";
  skos:broader bigg:HVACAndHotWaterMeasure.HotWaterSystemMeasure .

bigg:HVACAndHotWaterMeasure.HotWaterSystemMeasure.HotWaterDistributionAndStorageMeasure.HotWaterStorageTankInsulation
  a bigg:EnergyEfficiencyMeasureType, skos:Concept;
  rdfs:comment "Improvement of the insulation of the hot water storage tank";
  skos:broader bigg:HVACAndHotWaterMeasure.HotWaterSystemMeasure.HotWaterDistributionAndStorageMeasure .

bigg:HVACAndHotWaterMeasure.HotWaterSystemMeasure.HotWaterDistributionAndStorageMeasure.OtherHotWaterDistributionAndStorageMeasure
  a bigg:EnergyEfficiencyMeasureType, skos:Concept;
  rdfs:comment "Other measure on the hot water distribution or storage systems";
  skos:broader bigg:HVACAndHotWaterMeasure.HotWaterSystemMeasure.HotWaterDistributionAndStorageMeasure .

bigg:HVACAndHotWaterMeasure.HotWaterSystemMeasure.HotWaterFinalElementsMeasure a bigg:EnergyEfficiencyMeasureType,
    skos:Concept;
  rdfs:comment "Measure that affects the water heating system final elements  (eg. taps)";
  skos:broader bigg:HVACAndHotWaterMeasure.HotWaterSystemMeasure .

bigg:HVACAndHotWaterMeasure.HotWaterSystemMeasure.HotWaterFinalElementsMeasure.HotWaterTapSavingDeviceInstallation
  a bigg:EnergyEfficiencyMeasureType, skos:Concept;
  rdfs:comment "Installation of saving devices to hot water taps or shower (eg. tap aerators)";
  skos:broader bigg:HVACAndHotWaterMeasure.HotWaterSystemMeasure.HotWaterFinalElementsMeasure .

bigg:HVACAndHotWaterMeasure.HotWaterSystemMeasure.HotWaterFinalElementsMeasure.OtherHotWaterFinalElementsMeasure
  a bigg:EnergyEfficiencyMeasureType, skos:Concept;
  rdfs:comment "Other measure on the final elements of the water heating system";
  skos:broader bigg:HVACAndHotWaterMeasure.HotWaterSystemMeasure.HotWaterFinalElementsMeasure .

bigg:HVACAndHotWaterMeasure.HotWaterSystemMeasure.HotWaterControlMeasure a bigg:EnergyEfficiencyMeasureType,
    skos:Concept;
  rdfs:comment "Measure that affects the automation and controls of the water heating system";
  skos:broader bigg:HVACAndHotWaterMeasure.HotWaterSystemMeasure .

bigg:HVACAndHotWaterMeasure.HotWaterSystemMeasure.HotWaterControlMeasure.HotWaterTimeControl
  a bigg:EnergyEfficiencyMeasureType, skos:Concept;
  rdfs:comment "Installation of a timer to control the turn on/off of the water heating system";
  skos:broader bigg:HVACAndHotWaterMeasure.HotWaterSystemMeasure.HotWaterControlMeasure .

bigg:HVACAndHotWaterMeasure.HotWaterSystemMeasure.HotWaterControlMeasure.HotWaterTemperatureSensorInstallation
  a bigg:EnergyEfficiencyMeasureType, skos:Concept;
  rdfs:comment "Installation of temperature sensors to control the turn on/off of the water heating system";
  skos:broader bigg:HVACAndHotWaterMeasure.HotWaterSystemMeasure.HotWaterControlMeasure .

bigg:HVACAndHotWaterMeasure.HotWaterSystemMeasure.HotWaterControlMeasure.OtherHotWaterControlMeasure
  a bigg:EnergyEfficiencyMeasureType, skos:Concept;
  rdfs:comment "Other measure for the control and automation of the water heating system";
  skos:broader bigg:HVACAndHotWaterMeasure.HotWaterSystemMeasure.HotWaterControlMeasure .

bigg:HVACAndHotWaterMeasure.CombinedHeatingHotWaterSystemMeasure a bigg:EnergyEfficiencyMeasureType,
    skos:Concept;
  rdfs:comment "Measure with a combined effect onthe space and water heating systems of the building";
  skos:broader bigg:HVACAndHotWaterMeasure .

bigg:HVACAndHotWaterMeasure.CombinedHeatingHotWaterSystemMeasure.HeatAndHotWaterProductionMeasure
  a bigg:EnergyEfficiencyMeasureType, skos:Concept;
  rdfs:comment "Measure that affects the hot  water production system";
  skos:broader bigg:HVACAndHotWaterMeasure.CombinedHeatingHotWaterSystemMeasure .

bigg:HVACAndHotWaterMeasure.CombinedHeatingHotWaterSystemMeasure.HeatAndHotWaterProductionMeasure.HeatAndHotWaterBoilerReplacement
  a bigg:EnergyEfficiencyMeasureType, skos:Concept;
  rdfs:comment "Replacement of the boiler with a more efficient one that uses the same fuel";
  skos:broader bigg:HVACAndHotWaterMeasure.CombinedHeatingHotWaterSystemMeasure.HeatAndHotWaterProductionMeasure .

bigg:HVACAndHotWaterMeasure.CombinedHeatingHotWaterSystemMeasure.HeatAndHotWaterProductionMeasure.HeatAndHotWaterHeatPumpReplacement
  a bigg:EnergyEfficiencyMeasureType, skos:Concept;
  rdfs:comment "Replacement of the heat pump with a more efficient one";
  skos:broader bigg:HVACAndHotWaterMeasure.CombinedHeatingHotWaterSystemMeasure.HeatAndHotWaterProductionMeasure .

bigg:HVACAndHotWaterMeasure.CombinedHeatingHotWaterSystemMeasure.HeatAndHotWaterProductionMeasure.HeatAndHotWaterProductionFuelConversion
  a bigg:EnergyEfficiencyMeasureType, skos:Concept;
  rdfs:comment "Replacement of the hot water production system with one that operates with a different fuel source ";
  skos:broader bigg:HVACAndHotWaterMeasure.CombinedHeatingHotWaterSystemMeasure.HeatAndHotWaterProductionMeasure .

bigg:HVACAndHotWaterMeasure.CombinedHeatingHotWaterSystemMeasure.HeatAndHotWaterProductionMeasure.HeatAndHotWaterHeatExchangersReplacement
  a bigg:EnergyEfficiencyMeasureType, skos:Concept;
  rdfs:comment "Replacement of heat exchangers ";
  skos:broader bigg:HVACAndHotWaterMeasure.CombinedHeatingHotWaterSystemMeasure.HeatAndHotWaterProductionMeasure .

bigg:HVACAndHotWaterMeasure.CombinedHeatingHotWaterSystemMeasure.HeatAndHotWaterProductionMeasure.HeatAndHotWaterBurnerReplacement
  a bigg:EnergyEfficiencyMeasureType, skos:Concept;
  rdfs:comment "Replacement of the burner";
  skos:broader bigg:HVACAndHotWaterMeasure.CombinedHeatingHotWaterSystemMeasure.HeatAndHotWaterProductionMeasure .

bigg:HVACAndHotWaterMeasure.CombinedHeatingHotWaterSystemMeasure.HeatAndHotWaterProductionMeasure.HeatAndHotWaterOtherElementReplacement
  a bigg:EnergyEfficiencyMeasureType, skos:Concept;
  rdfs:comment "Change of another single component in the hot water production system";
  skos:broader bigg:HVACAndHotWaterMeasure.CombinedHeatingHotWaterSystemMeasure.HeatAndHotWaterProductionMeasure .

bigg:HVACAndHotWaterMeasure.CombinedHeatingHotWaterSystemMeasure.HeatAndHotWaterProductionMeasure.HeatAndHotWaterProductionSystemInsulation
  a bigg:EnergyEfficiencyMeasureType, skos:Concept;
  rdfs:comment "Improvement of the hot water production elements insulation";
  skos:broader bigg:HVACAndHotWaterMeasure.CombinedHeatingHotWaterSystemMeasure.HeatAndHotWaterProductionMeasure .

bigg:HVACAndHotWaterMeasure.CombinedHeatingHotWaterSystemMeasure.HeatAndHotWaterProductionMeasure.OtherHeatAndHotWaterProductionMeasure
  a bigg:EnergyEfficiencyMeasureType, skos:Concept;
  rdfs:comment "Other measure on the hot water production system";
  skos:broader bigg:HVACAndHotWaterMeasure.CombinedHeatingHotWaterSystemMeasure.HeatAndHotWaterProductionMeasure .

bigg:HVACAndHotWaterMeasure.CombinedHeatingHotWaterSystemMeasure.HeatingAndHotWaterDistributionAndStorageMeasure
  a bigg:EnergyEfficiencyMeasureType, skos:Concept;
  rdfs:comment "Measure that affects the distribution subsystems of space/water heating ";
  skos:broader bigg:HVACAndHotWaterMeasure.CombinedHeatingHotWaterSystemMeasure .

bigg:HVACAndHotWaterMeasure.CombinedHeatingHotWaterSystemMeasure.HeatingAndHotWaterDistributionAndStorageMeasure.HeatAndHotWaterDistributionSystemReplacement
  a bigg:EnergyEfficiencyMeasureType, skos:Concept;
  rdfs:comment "Complete change of the hot water distribution system ";
  skos:broader bigg:HVACAndHotWaterMeasure.CombinedHeatingHotWaterSystemMeasure.HeatingAndHotWaterDistributionAndStorageMeasure .

bigg:HVACAndHotWaterMeasure.CombinedHeatingHotWaterSystemMeasure.HeatingAndHotWaterDistributionAndStorageMeasure.HeatAndHotWaterDistributionPumpReplacement
  a bigg:EnergyEfficiencyMeasureType, skos:Concept;
  rdfs:comment "Replacement of a pump";
  skos:broader bigg:HVACAndHotWaterMeasure.CombinedHeatingHotWaterSystemMeasure.HeatingAndHotWaterDistributionAndStorageMeasure .

bigg:HVACAndHotWaterMeasure.CombinedHeatingHotWaterSystemMeasure.HeatingAndHotWaterDistributionAndStorageMeasure.HeatingAndHotWaterDistributionVariableSpeedDrivesInstallation
  a bigg:EnergyEfficiencyMeasureType, skos:Concept;
  rdfs:comment "Installation of variable speed drives for the control of hot water distribution elements (eg. pumps)";
  skos:broader bigg:HVACAndHotWaterMeasure.CombinedHeatingHotWaterSystemMeasure.HeatingAndHotWaterDistributionAndStorageMeasure .

bigg:HVACAndHotWaterMeasure.CombinedHeatingHotWaterSystemMeasure.HeatingAndHotWaterDistributionAndStorageMeasure.HeatAndHotWaterDistributionOtherComponentReplacement
  a bigg:EnergyEfficiencyMeasureType, skos:Concept;
  rdfs:comment "Replacement or installation of other distribution elements (eg. valves or filters)";
  skos:broader bigg:HVACAndHotWaterMeasure.CombinedHeatingHotWaterSystemMeasure.HeatingAndHotWaterDistributionAndStorageMeasure .

bigg:HVACAndHotWaterMeasure.CombinedHeatingHotWaterSystemMeasure.HeatingAndHotWaterDistributionAndStorageMeasure.HeatingAndHotWaterDistributionBalancingAndFlowRegulation
  a bigg:EnergyEfficiencyMeasureType, skos:Concept;
  rdfs:comment "Optimization of the hot water distribution through regulation of the water flow by means of balancing valves";
  skos:broader bigg:HVACAndHotWaterMeasure.CombinedHeatingHotWaterSystemMeasure.HeatingAndHotWaterDistributionAndStorageMeasure .

bigg:HVACAndHotWaterMeasure.CombinedHeatingHotWaterSystemMeasure.HeatingAndHotWaterDistributionAndStorageMeasure.HeatAndHotWaterPipesSubstitution
  a bigg:EnergyEfficiencyMeasureType, skos:Concept;
  rdfs:comment "Substitution of the pipes";
  skos:broader bigg:HVACAndHotWaterMeasure.CombinedHeatingHotWaterSystemMeasure.HeatingAndHotWaterDistributionAndStorageMeasure .

bigg:HVACAndHotWaterMeasure.CombinedHeatingHotWaterSystemMeasure.HeatingAndHotWaterDistributionAndStorageMeasure.HeatAndHotWaterPipesInsulation
  a bigg:EnergyEfficiencyMeasureType, skos:Concept;
  rdfs:comment "Improvement of the insulation of the pipes";
  skos:broader bigg:HVACAndHotWaterMeasure.CombinedHeatingHotWaterSystemMeasure.HeatingAndHotWaterDistributionAndStorageMeasure .

bigg:HVACAndHotWaterMeasure.CombinedHeatingHotWaterSystemMeasure.HeatingAndHotWaterDistributionAndStorageMeasure.HeatAndHotWaterStorageTankInstallation
  a bigg:EnergyEfficiencyMeasureType, skos:Concept;
  rdfs:comment "Installation or substitution of the hot water storage tank";
  skos:broader bigg:HVACAndHotWaterMeasure.CombinedHeatingHotWaterSystemMeasure.HeatingAndHotWaterDistributionAndStorageMeasure .

bigg:HVACAndHotWaterMeasure.CombinedHeatingHotWaterSystemMeasure.HeatingAndHotWaterDistributionAndStorageMeasure.HeatAndHotWaterStorageTankInsulation
  a bigg:EnergyEfficiencyMeasureType, skos:Concept;
  rdfs:comment "Improvement of the insulation of the hot water storage tank";
  skos:broader bigg:HVACAndHotWaterMeasure.CombinedHeatingHotWaterSystemMeasure.HeatingAndHotWaterDistributionAndStorageMeasure .

bigg:HVACAndHotWaterMeasure.CombinedHeatingHotWaterSystemMeasure.HeatingAndHotWaterDistributionAndStorageMeasure.OtherHeatAndHotWaterDistributionMeasure
  a bigg:EnergyEfficiencyMeasureType, skos:Concept;
  rdfs:comment "Other measure on the space/water heating distribution or storage systems";
  skos:broader bigg:HVACAndHotWaterMeasure.CombinedHeatingHotWaterSystemMeasure.HeatingAndHotWaterDistributionAndStorageMeasure .

bigg:HVACAndHotWaterMeasure.CombinedHeatingHotWaterSystemMeasure.HeatingAndHotWaterControlMeasure
  a bigg:EnergyEfficiencyMeasureType, skos:Concept;
  rdfs:comment "Measure that affects the automation and controls of the space/water heating system";
  skos:broader bigg:HVACAndHotWaterMeasure.CombinedHeatingHotWaterSystemMeasure .

bigg:HVACAndHotWaterMeasure.CombinedHeatingHotWaterSystemMeasure.HeatingAndHotWaterControlMeasure.HeatingAndHotWaterTemperatureSensorInstallation
  a bigg:EnergyEfficiencyMeasureType, skos:Concept;
  rdfs:comment "Installation of temperature sensors to control the turn on/off of the space/water heating system";
  skos:broader bigg:HVACAndHotWaterMeasure.CombinedHeatingHotWaterSystemMeasure.HeatingAndHotWaterControlMeasure .

bigg:HVACAndHotWaterMeasure.CombinedHeatingHotWaterSystemMeasure.HeatingAndHotWaterControlMeasure.OtherHeatingAndHotWaterControlMeasure
  a bigg:EnergyEfficiencyMeasureType, skos:Concept;
  rdfs:comment "Other measure for the control and automation of the pace/water heating system";
  skos:broader bigg:HVACAndHotWaterMeasure.CombinedHeatingHotWaterSystemMeasure.HeatingAndHotWaterControlMeasure .

bigg:HVACAndHotWaterMeasure.MechanicalVentilationSystemMeasure a bigg:EnergyEfficiencyMeasureType,
    skos:Concept;
  rdfs:comment "Measure that affects the mechanical ventilation system of the building";
  skos:broader bigg:HVACAndHotWaterMeasure .

bigg:HVACAndHotWaterMeasure.MechanicalVentilationSystemMeasure.MechanicalVentilationDistributionMeasure
  a bigg:EnergyEfficiencyMeasureType, skos:Concept;
  rdfs:comment "Measure that affects the air distribution ";
  skos:broader bigg:HVACAndHotWaterMeasure.MechanicalVentilationSystemMeasure .

bigg:HVACAndHotWaterMeasure.MechanicalVentilationSystemMeasure.MechanicalVentilationDistributionMeasure.VentilationSystemReplacement
  a bigg:EnergyEfficiencyMeasureType, skos:Concept;
  rdfs:comment "Installation or replacement of a mechanical ventilation system";
  skos:broader bigg:HVACAndHotWaterMeasure.MechanicalVentilationSystemMeasure.MechanicalVentilationDistributionMeasure .

bigg:HVACAndHotWaterMeasure.MechanicalVentilationSystemMeasure.MechanicalVentilationDistributionMeasure.VentilationFansOrMotorReplacement
  a bigg:EnergyEfficiencyMeasureType, skos:Concept;
  rdfs:comment "Replacement of motors or fans";
  skos:broader bigg:HVACAndHotWaterMeasure.MechanicalVentilationSystemMeasure.MechanicalVentilationDistributionMeasure .

bigg:HVACAndHotWaterMeasure.MechanicalVentilationSystemMeasure.MechanicalVentilationDistributionMeasure.VentilationVariableSpeedDrivesInstallation
  a bigg:EnergyEfficiencyMeasureType, skos:Concept;
  rdfs:comment "Installation of variable speed drives for the control of air distribution elements (eg. fans)";
  skos:broader bigg:HVACAndHotWaterMeasure.MechanicalVentilationSystemMeasure.MechanicalVentilationDistributionMeasure .

bigg:HVACAndHotWaterMeasure.MechanicalVentilationSystemMeasure.MechanicalVentilationDistributionMeasure.VentilationHeatRecoveryInstallation
  a bigg:EnergyEfficiencyMeasureType, skos:Concept;
  rdfs:comment "Installation of a recovery system that uses the heat exhaust air to preheat incoming fresh air";
  skos:broader bigg:HVACAndHotWaterMeasure.MechanicalVentilationSystemMeasure.MechanicalVentilationDistributionMeasure .

bigg:HVACAndHotWaterMeasure.MechanicalVentilationSystemMeasure.MechanicalVentilationDistributionMeasure.AirHandlingUnitReplacement
  a bigg:EnergyEfficiencyMeasureType, skos:Concept;
  rdfs:comment "Replacement of the Air Handling Unit (AHU) of the building";
  skos:broader bigg:HVACAndHotWaterMeasure.MechanicalVentilationSystemMeasure.MechanicalVentilationDistributionMeasure .

bigg:HVACAndHotWaterMeasure.MechanicalVentilationSystemMeasure.MechanicalVentilationDistributionMeasure.VentilationDistributionFlowRegulation
  a bigg:EnergyEfficiencyMeasureType, skos:Concept;
  rdfs:comment "Optimization of the air distribution through flow regulation (eg. by means of dampers)";
  skos:broader bigg:HVACAndHotWaterMeasure.MechanicalVentilationSystemMeasure.MechanicalVentilationDistributionMeasure .

bigg:HVACAndHotWaterMeasure.MechanicalVentilationSystemMeasure.MechanicalVentilationDistributionMeasure.VentilationDuctsSubstitution
  a bigg:EnergyEfficiencyMeasureType, skos:Concept;
  rdfs:comment "Substitution of the ducts";
  skos:broader bigg:HVACAndHotWaterMeasure.MechanicalVentilationSystemMeasure.MechanicalVentilationDistributionMeasure .

bigg:HVACAndHotWaterMeasure.MechanicalVentilationSystemMeasure.MechanicalVentilationDistributionMeasure.VentilationDuctsInsulation
  a bigg:EnergyEfficiencyMeasureType, skos:Concept;
  rdfs:comment "Improvement of the insulation of the ducts";
  skos:broader bigg:HVACAndHotWaterMeasure.MechanicalVentilationSystemMeasure.MechanicalVentilationDistributionMeasure .

bigg:HVACAndHotWaterMeasure.MechanicalVentilationSystemMeasure.MechanicalVentilationDistributionMeasure.OtherMechanicalVentilationMeasure
  a bigg:EnergyEfficiencyMeasureType, skos:Concept;
  rdfs:comment "Other measure on the air distribution system";
  skos:broader bigg:HVACAndHotWaterMeasure.MechanicalVentilationSystemMeasure.MechanicalVentilationDistributionMeasure .

bigg:BuildingFabricMeasure a bigg:EnergyEfficiencyMeasureType, skos:Concept;
  rdfs:comment "Measure that affects the building fabric or envelope" .

bigg:BuildingFabricMeasure.WallMeasure a bigg:EnergyEfficiencyMeasureType, skos:Concept;
  rdfs:comment "Measure that affects the building walls";
  skos:broader bigg:BuildingFabricMeasure .

bigg:BuildingFabricMeasure.WallMeasure.WallExternalInsulation a bigg:EnergyEfficiencyMeasureType,
    skos:Concept;
  rdfs:comment "External walls insulation addition or replacement";
  skos:broader bigg:BuildingFabricMeasure.WallMeasure .

bigg:BuildingFabricMeasure.WallMeasure.WallWaterproofing a bigg:EnergyEfficiencyMeasureType,
    skos:Concept;
  rdfs:comment "Addition of a waterproof layer to the building walls to prevent the penetration of water into the structure ";
  skos:broader bigg:BuildingFabricMeasure.WallMeasure .

bigg:BuildingFabricMeasure.WallMeasure.WallCavityInsulation a bigg:EnergyEfficiencyMeasureType,
    skos:Concept;
  rdfs:comment "Wall cavities insulation addition or replacement";
  skos:broader bigg:BuildingFabricMeasure.WallMeasure .

bigg:BuildingFabricMeasure.WallMeasure.WallInternalInsulation a bigg:EnergyEfficiencyMeasureType,
    skos:Concept;
  rdfs:comment "Internal walls insulation addition or replacement";
  skos:broader bigg:BuildingFabricMeasure.WallMeasure .

bigg:BuildingFabricMeasure.WallMeasure.OtherWallMeasure a bigg:EnergyEfficiencyMeasureType,
    skos:Concept;
  rdfs:comment "Other measure on the building walls";
  skos:broader bigg:BuildingFabricMeasure.WallMeasure .

bigg:BuildingFabricMeasure.RoofAndCeilingMeasure a bigg:EnergyEfficiencyMeasureType,
    skos:Concept;
  rdfs:comment "Measure that affects the building roof or ceiling";
  skos:broader bigg:BuildingFabricMeasure .

bigg:BuildingFabricMeasure.RoofAndCeilingMeasure.PitchedRoofInsulation a bigg:EnergyEfficiencyMeasureType,
    skos:Concept;
  rdfs:comment "Insulation of a roof that is formed by surfaces sloping downward with an angle of more than 20°";
  skos:broader bigg:BuildingFabricMeasure.RoofAndCeilingMeasure .

bigg:BuildingFabricMeasure.RoofAndCeilingMeasure.FlatRoofInsulation a bigg:EnergyEfficiencyMeasureType,
    skos:Concept;
  rdfs:comment "Insulation of a roof that is flat or formed by surfaces sloping downward with an angle of less than 20°";
  skos:broader bigg:BuildingFabricMeasure.RoofAndCeilingMeasure .

bigg:BuildingFabricMeasure.RoofAndCeilingMeasure.ReflectiveRoofCoating a bigg:EnergyEfficiencyMeasureType,
    skos:Concept;
  rdfs:comment "Application of a coating to the roof to reflect more sunlight and decrease the heat absorbed by the structure";
  skos:broader bigg:BuildingFabricMeasure.RoofAndCeilingMeasure .

bigg:BuildingFabricMeasure.RoofAndCeilingMeasure.RoofWaterproofing a bigg:EnergyEfficiencyMeasureType,
    skos:Concept;
  rdfs:comment "Addition of a waterproof layer to the building roof to prevent the penetration of water into the structure ";
  skos:broader bigg:BuildingFabricMeasure.RoofAndCeilingMeasure .

bigg:BuildingFabricMeasure.RoofAndCeilingMeasure.GreenRoofInstallation a bigg:EnergyEfficiencyMeasureType,
    skos:Concept;
  rdfs:comment "Installation on the roof of a layer of vegetation planted over a waterproofing system.";
  skos:broader bigg:BuildingFabricMeasure.RoofAndCeilingMeasure .

bigg:BuildingFabricMeasure.RoofAndCeilingMeasure.CeilingLoftInsulation a bigg:EnergyEfficiencyMeasureType,
    skos:Concept;
  rdfs:comment "Installation of insulating material over the loft floor or between the roof rafters";
  skos:broader bigg:BuildingFabricMeasure.RoofAndCeilingMeasure .

bigg:BuildingFabricMeasure.RoofAndCeilingMeasure.OtherRoofAndCeilingMeasure a bigg:EnergyEfficiencyMeasureType,
    skos:Concept;
  rdfs:comment "Other measure on the building roof or ceiling";
  skos:broader bigg:BuildingFabricMeasure.RoofAndCeilingMeasure .

bigg:BuildingFabricMeasure.FloorMeasure a bigg:EnergyEfficiencyMeasureType, skos:Concept;
  rdfs:comment "Measure that affects the building floor";
  skos:broader bigg:BuildingFabricMeasure .

bigg:BuildingFabricMeasure.FloorMeasure.SuspendedFloorInsulation a bigg:EnergyEfficiencyMeasureType,
    skos:Concept;
  rdfs:comment "Installation of insulating material between the suspended floor supporting structure";
  skos:broader bigg:BuildingFabricMeasure.FloorMeasure .

bigg:BuildingFabricMeasure.FloorMeasure.SolidFloorInsulation a bigg:EnergyEfficiencyMeasureType,
    skos:Concept;
  rdfs:comment "Installation of an insulation layer between the concrete slab and the floor";
  skos:broader bigg:BuildingFabricMeasure.FloorMeasure .

bigg:BuildingFabricMeasure.FloorMeasure.OtherFloorMeasure a bigg:EnergyEfficiencyMeasureType,
    skos:Concept;
  rdfs:comment "Other measure that affects the building floor";
  skos:broader bigg:BuildingFabricMeasure.FloorMeasure .

bigg:BuildingFabricMeasure.WindowMeasure a bigg:EnergyEfficiencyMeasureType, skos:Concept;
  rdfs:comment "Measure that affects the windows of the building";
  skos:broader bigg:BuildingFabricMeasure .

bigg:BuildingFabricMeasure.WindowMeasure.WindowReplacement a bigg:EnergyEfficiencyMeasureType,
    skos:Concept;
  rdfs:comment "Replacement of the whole windows with more energy-efficient ones (eg. simple to double glass or to low emissive double glass)";
  skos:broader bigg:BuildingFabricMeasure.WindowMeasure .

bigg:BuildingFabricMeasure.WindowMeasure.WindowsGlassReplacement a bigg:EnergyEfficiencyMeasureType,
    skos:Concept;
  rdfs:comment "Replacement of the windows’ glass panes (eg. simple to double glass or to low emissive double glass)";
  skos:broader bigg:BuildingFabricMeasure.WindowMeasure .

bigg:BuildingFabricMeasure.WindowMeasure.WindowCoatingInstallation a bigg:EnergyEfficiencyMeasureType,
    skos:Concept;
  rdfs:comment "Installation of tinted or reflective coating over the windows' glass panes";
  skos:broader bigg:BuildingFabricMeasure.WindowMeasure .

bigg:BuildingFabricMeasure.WindowMeasure.WindowsSealingImprovement a bigg:EnergyEfficiencyMeasureType,
    skos:Concept;
  rdfs:comment "Improvement of the sealing of windows (eg. adhesive sealing)";
  skos:broader bigg:BuildingFabricMeasure.WindowMeasure .

bigg:BuildingFabricMeasure.WindowMeasure.OtherWindowMeasure a bigg:EnergyEfficiencyMeasureType,
    skos:Concept;
  rdfs:comment "Other measure that affects the windows of the building";
  skos:broader bigg:BuildingFabricMeasure.WindowMeasure .

bigg:BuildingFabricMeasure.SkylightsMeasure a bigg:EnergyEfficiencyMeasureType, skos:Concept;
  rdfs:comment "Measure that affects the skylights of the building";
  skos:broader bigg:BuildingFabricMeasure .

bigg:BuildingFabricMeasure.SkylightsMeasure.SkylightReplacement a bigg:EnergyEfficiencyMeasureType,
    skos:Concept;
  rdfs:comment "Replacement of the whole skylights with more energy-efficient ones (eg. simple to double glass or to low emissive double glass)";
  skos:broader bigg:BuildingFabricMeasure.SkylightsMeasure .

bigg:BuildingFabricMeasure.SkylightsMeasure.SkylightGlassReplacement a bigg:EnergyEfficiencyMeasureType,
    skos:Concept;
  rdfs:comment "Replacement of the skylights’ glass panes (eg. simple to double glass or to low emissive double glass)";
  skos:broader bigg:BuildingFabricMeasure.SkylightsMeasure .

bigg:BuildingFabricMeasure.SkylightsMeasure.SkylightCoatingInstallation a bigg:EnergyEfficiencyMeasureType,
    skos:Concept;
  rdfs:comment "Installation of tinted or reflective coating over the skylights' glass panes";
  skos:broader bigg:BuildingFabricMeasure.SkylightsMeasure .

bigg:BuildingFabricMeasure.SkylightsMeasure.OtherSkylightMeasure a bigg:EnergyEfficiencyMeasureType,
    skos:Concept;
  rdfs:comment "Other measure that affects the skylights of the building";
  skos:broader bigg:BuildingFabricMeasure.SkylightsMeasure .

bigg:BuildingFabricMeasure.DoorsMeasure a bigg:EnergyEfficiencyMeasureType, skos:Concept;
  rdfs:comment "Measure that affects the doors of the building";
  skos:broader bigg:BuildingFabricMeasure .

bigg:BuildingFabricMeasure.DoorsMeasure.DoorsReplacement a bigg:EnergyEfficiencyMeasureType,
    skos:Concept;
  rdfs:comment "Replacement of the whole door(s)";
  skos:broader bigg:BuildingFabricMeasure.DoorsMeasure .

bigg:BuildingFabricMeasure.DoorsMeasure.AutomaticDoorInstallation a bigg:EnergyEfficiencyMeasureType,
    skos:Concept;
  rdfs:comment "Installation of mechanical drives to automatically close the doors that lead to the exterior or to non-climatized spaces";
  skos:broader bigg:BuildingFabricMeasure.DoorsMeasure .

bigg:BuildingFabricMeasure.DoorsMeasure.DoorGlassReplacement a bigg:EnergyEfficiencyMeasureType,
    skos:Concept;
  rdfs:comment "Replacement of the doors’ glasses (simple to double glass or to low emissive double glass)";
  skos:broader bigg:BuildingFabricMeasure.DoorsMeasure .

bigg:BuildingFabricMeasure.DoorsMeasure.DoorGlassCoatingInstallation a bigg:EnergyEfficiencyMeasureType,
    skos:Concept;
  rdfs:comment "Installation of tinted or reflective coating over the doors' glass panes";
  skos:broader bigg:BuildingFabricMeasure.DoorsMeasure .

bigg:BuildingFabricMeasure.DoorsMeasure.DoorsSealingImprovement a bigg:EnergyEfficiencyMeasureType,
    skos:Concept;
  rdfs:comment "Improvement of the sealing of doors (eg. adhesive sealing)";
  skos:broader bigg:BuildingFabricMeasure.DoorsMeasure .

bigg:BuildingFabricMeasure.DoorsMeasure.OtherDoorMeasure a bigg:EnergyEfficiencyMeasureType,
    skos:Concept;
  rdfs:comment "Other measure that affects the doors of the building";
  skos:broader bigg:BuildingFabricMeasure.DoorsMeasure .

bigg:BuildingFabricMeasure.AirInfiltrationMeasure a bigg:EnergyEfficiencyMeasureType,
    skos:Concept;
  rdfs:comment "Measure that aims at reducing the air infiltrations through the building envelope";
  skos:broader bigg:BuildingFabricMeasure .

bigg:BuildingFabricMeasure.AirInfiltrationMeasure.DraughtProofing a bigg:EnergyEfficiencyMeasureType,
    skos:Concept;
  rdfs:comment "Installation of internal draught-proofing elements to prevent the infiltration of external air through the surface elements of the building";
  skos:broader bigg:BuildingFabricMeasure.AirInfiltrationMeasure .

bigg:BuildingFabricMeasure.AirInfiltrationMeasure.AirCurtainsInstallation a bigg:EnergyEfficiencyMeasureType,
    skos:Concept;
  rdfs:comment "Installation of a fan-powered air curtain over openings that lead to the exterior or to non-climatized spaces ";
  skos:broader bigg:BuildingFabricMeasure.AirInfiltrationMeasure .

bigg:BuildingFabricMeasure.AirInfiltrationMeasure.OtherAirInfiltrationMeasure a bigg:EnergyEfficiencyMeasureType,
    skos:Concept;
  rdfs:comment "Other measure that aims at reducing the air infiltrations through the building envelope";
  skos:broader bigg:BuildingFabricMeasure.AirInfiltrationMeasure .

bigg:BuildingFabricMeasure.ShadingMeasure a bigg:EnergyEfficiencyMeasureType, skos:Concept;
  rdfs:comment "Measure that aims at preventing overheating due to solar light";
  skos:broader bigg:BuildingFabricMeasure .

bigg:BuildingFabricMeasure.ShadingMeasure.ExternalShadingInstallation a bigg:EnergyEfficiencyMeasureType,
    skos:Concept;
  rdfs:comment "Installation of shading devices on the building façade glazing elements to reduce solar heat gain";
  skos:broader bigg:BuildingFabricMeasure.ShadingMeasure .

bigg:BuildingFabricMeasure.ShadingMeasure.InternalShadingInstallation a bigg:EnergyEfficiencyMeasureType,
    skos:Concept;
  rdfs:comment "Installation of blinds or curtains to reduce solar heat gain";
  skos:broader bigg:BuildingFabricMeasure.ShadingMeasure .

bigg:BuildingFabricMeasure.ShadingMeasure.AutomaticShadingSystemInstallation a bigg:EnergyEfficiencyMeasureType,
    skos:Concept;
  rdfs:comment "Implementation of a programmable system for the automated opening/closing of solar shading devices";
  skos:broader bigg:BuildingFabricMeasure.ShadingMeasure .

bigg:BuildingFabricMeasure.ShadingMeasure.OtherShadingMeasure a bigg:EnergyEfficiencyMeasureType,
    skos:Concept;
  rdfs:comment "Other measure that aims at preventing overheating due to solar light";
  skos:broader bigg:BuildingFabricMeasure.ShadingMeasure .

bigg:BuildingFabricMeasure.ComprehensiveBuildingFabricRenovation a bigg:EnergyEfficiencyMeasureType,
    skos:Concept;
  rdfs:comment "Comprehensive intervention on the building fabric that aims at improving the energy efficiency of the building (eg. modernization, retroﬁt, or upgrade)";
  skos:broader bigg:BuildingFabricMeasure .

bigg:ElectricPowerSystemMeasure a bigg:EnergyEfficiencyMeasureType, skos:Concept;
  rdfs:comment "Measure that affects the building power system or the electric equipment that it contains" .

bigg:ElectricPowerSystemMeasure.PowerSystemMeasure a bigg:EnergyEfficiencyMeasureType,
    skos:Concept;
  rdfs:comment "Measure that affects the building power system ";
  skos:broader bigg:ElectricPowerSystemMeasure .

bigg:ElectricPowerSystemMeasure.PowerSystemMeasure.PowerSystemCompleteUpgrade a bigg:EnergyEfficiencyMeasureType,
    skos:Concept;
  rdfs:comment "Complete upgrade and renovation of the building electric power system ";
  skos:broader bigg:ElectricPowerSystemMeasure.PowerSystemMeasure .

bigg:ElectricPowerSystemMeasure.PowerSystemMeasure.PowerSystemVoltageOptimization
  a bigg:EnergyEfficiencyMeasureType, skos:Concept;
  rdfs:comment "Installation of technologies to regulate, clean and condition the incoming power supply to reduce the voltage to the optimum level for the on-site electrical equipment and appliances";
  skos:broader bigg:ElectricPowerSystemMeasure.PowerSystemMeasure .

bigg:ElectricPowerSystemMeasure.PowerSystemMeasure.PowerFactorCorrection a bigg:EnergyEfficiencyMeasureType,
    skos:Concept;
  rdfs:comment "Installation power factor correction capacitor banks to reduce the electrical current drawn for inductive loads";
  skos:broader bigg:ElectricPowerSystemMeasure.PowerSystemMeasure .

bigg:ElectricPowerSystemMeasure.PowerSystemMeasure.PowerSystemTransformersReplacement
  a bigg:EnergyEfficiencyMeasureType, skos:Concept;
  rdfs:comment "Installation of new, more energy-efficient transformers";
  skos:broader bigg:ElectricPowerSystemMeasure.PowerSystemMeasure .

bigg:ElectricPowerSystemMeasure.PowerSystemMeasure.ElectricDistributionPanelReplacement
  a bigg:EnergyEfficiencyMeasureType, skos:Concept;
  rdfs:comment "Replacement or upgrade of the electricity distribution panel";
  skos:broader bigg:ElectricPowerSystemMeasure.PowerSystemMeasure .

bigg:ElectricPowerSystemMeasure.PowerSystemMeasure.UninterruptiblePowerSupplyInstallation
  a bigg:EnergyEfficiencyMeasureType, skos:Concept;
  rdfs:comment "Installation of an Uninterruptible Power Supply (UPS) backup system";
  skos:broader bigg:ElectricPowerSystemMeasure.PowerSystemMeasure .

bigg:ElectricPowerSystemMeasure.PowerSystemMeasure.OtherPowerSystemMeasure a bigg:EnergyEfficiencyMeasureType,
    skos:Concept;
  rdfs:comment "Other measure that affects the building power system ";
  skos:broader bigg:ElectricPowerSystemMeasure.PowerSystemMeasure .

bigg:ElectricPowerSystemMeasure.ElectricEquipmentMeasure a bigg:EnergyEfficiencyMeasureType,
    skos:Concept;
  rdfs:comment "Measure that affects the electric equipment contained in the building";
  skos:broader bigg:ElectricPowerSystemMeasure .

bigg:ElectricPowerSystemMeasure.ElectricEquipmentMeasure.ElectricApplianceMeasure
  a bigg:EnergyEfficiencyMeasureType, skos:Concept;
  rdfs:comment "Replacement of electrical appliances with more efficient ones or other appliance measures";
  skos:broader bigg:ElectricPowerSystemMeasure.ElectricEquipmentMeasure .

bigg:ElectricPowerSystemMeasure.ElectricEquipmentMeasure.ElectricApplianceMeasure.VendingMachinesReplacement
  a bigg:EnergyEfficiencyMeasureType, skos:Concept;
  rdfs:comment "Replacement of the vending machines with more efficient ones";
  skos:broader bigg:ElectricPowerSystemMeasure.ElectricEquipmentMeasure.ElectricApplianceMeasure .

bigg:ElectricPowerSystemMeasure.ElectricEquipmentMeasure.ElectricApplianceMeasure.ElevatorReplacement
  a bigg:EnergyEfficiencyMeasureType, skos:Concept;
  rdfs:comment "Replacement or installation of an elevator";
  skos:broader bigg:ElectricPowerSystemMeasure.ElectricEquipmentMeasure.ElectricApplianceMeasure .

bigg:ElectricPowerSystemMeasure.ElectricEquipmentMeasure.ElectricApplianceMeasure.OtherElectricApplianceMeasure
  a bigg:EnergyEfficiencyMeasureType, skos:Concept;
  rdfs:comment "Other replacement or measure on electric appliances";
  skos:broader bigg:ElectricPowerSystemMeasure.ElectricEquipmentMeasure.ElectricApplianceMeasure .

bigg:ElectricPowerSystemMeasure.ElectricEquipmentMeasure.ICTEquipmentMeasure a bigg:EnergyEfficiencyMeasureType,
    skos:Concept;
  rdfs:comment "Measure that affects the Information and Communication Technology (ICT) equipment in the building";
  skos:broader bigg:ElectricPowerSystemMeasure.ElectricEquipmentMeasure .

bigg:ElectricPowerSystemMeasure.ElectricEquipmentMeasure.ICTEquipmentMeasure.ServersFreeCooling
  a bigg:EnergyEfficiencyMeasureType, skos:Concept;
  rdfs:comment "Installation of equipment to cool the servers by using naturally cool air or water instead of mechanical refrigeration";
  skos:broader bigg:ElectricPowerSystemMeasure.ElectricEquipmentMeasure.ICTEquipmentMeasure .

bigg:ElectricPowerSystemMeasure.ElectricEquipmentMeasure.ICTEquipmentMeasure.ServersVirtualization
  a bigg:EnergyEfficiencyMeasureType, skos:Concept;
  rdfs:comment "Conversion of physical servers into multiple virtual machines to reduce power consumption and heat generation";
  skos:broader bigg:ElectricPowerSystemMeasure.ElectricEquipmentMeasure.ICTEquipmentMeasure .

bigg:ElectricPowerSystemMeasure.ElectricEquipmentMeasure.ICTEquipmentMeasure.ServersReplacement
  a bigg:EnergyEfficiencyMeasureType, skos:Concept;
  rdfs:comment "Replacement or upgrade of the servers";
  skos:broader bigg:ElectricPowerSystemMeasure.ElectricEquipmentMeasure.ICTEquipmentMeasure .

bigg:ElectricPowerSystemMeasure.ElectricEquipmentMeasure.ICTEquipmentMeasure.PrintersReplacement
  a bigg:EnergyEfficiencyMeasureType, skos:Concept;
  rdfs:comment "Replacement or upgrade of the printers";
  skos:broader bigg:ElectricPowerSystemMeasure.ElectricEquipmentMeasure.ICTEquipmentMeasure .

bigg:ElectricPowerSystemMeasure.ElectricEquipmentMeasure.ICTEquipmentMeasure.ComputersReplacement
  a bigg:EnergyEfficiencyMeasureType, skos:Concept;
  rdfs:comment "Replacement of computers (eg. desktop to laptop)";
  skos:broader bigg:ElectricPowerSystemMeasure.ElectricEquipmentMeasure.ICTEquipmentMeasure .

bigg:ElectricPowerSystemMeasure.ElectricEquipmentMeasure.ICTEquipmentMeasure.ComputersPowerManagement
  a bigg:EnergyEfficiencyMeasureType, skos:Concept;
  rdfs:comment "Implementation of a control to reduce the power usage of computers";
  skos:broader bigg:ElectricPowerSystemMeasure.ElectricEquipmentMeasure.ICTEquipmentMeasure .

bigg:ElectricPowerSystemMeasure.ElectricEquipmentMeasure.ICTEquipmentMeasure.OtherICTEquipmentMeasure
  a bigg:EnergyEfficiencyMeasureType, skos:Concept;
  rdfs:comment "Other measure that affects the Information and Communication Technology (ICT) equipment in the building";
  skos:broader bigg:ElectricPowerSystemMeasure.ElectricEquipmentMeasure.ICTEquipmentMeasure .

bigg:RefrigerationSystemsMeasure a bigg:EnergyEfficiencyMeasureType, skos:Concept;
  rdfs:comment "Measure that affects building refrigeration system in the building (does not include space cooling)" .

bigg:RefrigerationSystemsMeasure.RefrigerationTechnicalOptimization a bigg:EnergyEfficiencyMeasureType,
    skos:Concept;
  rdfs:comment "Technical optimization of the refrigeration system by component renewal, supplement, or maintenance";
  skos:broader bigg:RefrigerationSystemsMeasure .

bigg:RefrigerationSystemsMeasure.RefrigerationTechnicalOptimization.RefrigerationSystemEfficiencyImprovement
  a bigg:EnergyEfficiencyMeasureType, skos:Concept;
  rdfs:comment "Measure that aims at improving the overall efficiency of the refrigeration system";
  skos:broader bigg:RefrigerationSystemsMeasure.RefrigerationTechnicalOptimization .

bigg:RefrigerationSystemsMeasure.RefrigerationTechnicalOptimization.RefrigerationCompressorsReplacement
  a bigg:EnergyEfficiencyMeasureType, skos:Concept;
  rdfs:comment "Replacement of the compressor";
  skos:broader bigg:RefrigerationSystemsMeasure.RefrigerationTechnicalOptimization .

bigg:RefrigerationSystemsMeasure.RefrigerationTechnicalOptimization.RefrigeratedSpaceDoorsOrCurtainsInstallation
  a bigg:EnergyEfficiencyMeasureType, skos:Concept;
  rdfs:comment "Installation of doors or curtains to separate the fridges or refrigerated rooms from areas at ambient temperature ";
  skos:broader bigg:RefrigerationSystemsMeasure.RefrigerationTechnicalOptimization .

bigg:RefrigerationSystemsMeasure.RefrigerationTechnicalOptimization.RefrigeratedSpaceInsulation
  a bigg:EnergyEfficiencyMeasureType, skos:Concept;
  rdfs:comment "Improvement of the insulation of the refrigerated space";
  skos:broader bigg:RefrigerationSystemsMeasure.RefrigerationTechnicalOptimization .

bigg:RefrigerationSystemsMeasure.RefrigerationTechnicalOptimization.OtherRefrigerationTechnicalOptimization
  a bigg:EnergyEfficiencyMeasureType, skos:Concept;
  rdfs:comment "Other technical optimization of the refrigeration system";
  skos:broader bigg:RefrigerationSystemsMeasure.RefrigerationTechnicalOptimization .

bigg:RefrigerationSystemsMeasure.RefrigerationOperationalOptimization a bigg:EnergyEfficiencyMeasureType,
    skos:Concept;
  rdfs:comment "Operational optimization (controls and automation)";
  skos:broader bigg:RefrigerationSystemsMeasure .

bigg:RefrigerationSystemsMeasure.RefrigerationOperationalOptimization.RefrigerationControlImprovement
  a bigg:EnergyEfficiencyMeasureType, skos:Concept;
  rdfs:comment "Improvement of the controls of the refrigeration system";
  skos:broader bigg:RefrigerationSystemsMeasure.RefrigerationOperationalOptimization .

bigg:RefrigerationSystemsMeasure.RefrigerationOperationalOptimization.DefrostCycleControlOptimization
  a bigg:EnergyEfficiencyMeasureType, skos:Concept;
  rdfs:comment "Implementation of a defrost cycle control to improve performance of the system";
  skos:broader bigg:RefrigerationSystemsMeasure.RefrigerationOperationalOptimization .

bigg:RefrigerationSystemsMeasure.RefrigerationOperationalOptimization.RefrigerationCondensingUnitCapacityControlOptimization
  a bigg:EnergyEfficiencyMeasureType, skos:Concept;
  rdfs:comment "Implementation of a control to reduce the refrigeration load while maintaining the temperature setpoint";
  skos:broader bigg:RefrigerationSystemsMeasure.RefrigerationOperationalOptimization .

bigg:RefrigerationSystemsMeasure.RefrigerationOperationalOptimization.RefrigerationFloatingHeadPressureControlImplementation
  a bigg:EnergyEfficiencyMeasureType, skos:Concept;
  rdfs:comment "Implementation of a control to reduce the exit pressure of the compressor in function of the outside temperature ";
  skos:broader bigg:RefrigerationSystemsMeasure.RefrigerationOperationalOptimization .

bigg:RefrigerationSystemsMeasure.RefrigerationOperationalOptimization.OtherRefrigerationOperationalOptimization
  a bigg:EnergyEfficiencyMeasureType, skos:Concept;
  rdfs:comment "Other operational optimization of the refrigeration system";
  skos:broader bigg:RefrigerationSystemsMeasure.RefrigerationOperationalOptimization .

bigg:RefrigerationSystemsMeasure.RefrigerationSystemCompleteRenewal a bigg:EnergyEfficiencyMeasureType,
    skos:Concept;
  rdfs:comment "Complete renewal or substitution of the refrigeration system";
  skos:broader bigg:RefrigerationSystemsMeasure .

bigg:ManagementMeasure a bigg:EnergyEfficiencyMeasureType, skos:Concept;
  rdfs:comment "Management measure adopted to reduce the energy consumption of the building" .

bigg:ManagementMeasure.BuildingEnergyManagementSystemInstallation a bigg:EnergyEfficiencyMeasureType,
    skos:Concept;
  rdfs:comment "Installation or replacement of a Building Energy Management System (BEMS)";
  skos:broader bigg:ManagementMeasure .

bigg:ManagementMeasure.PersonnelTraining a bigg:EnergyEfficiencyMeasureType, skos:Concept;
  rdfs:comment "Training of the personnel and awareness-raising";
  skos:broader bigg:ManagementMeasure .

bigg:ManagementMeasure.EnergyManagerAppointment a bigg:EnergyEfficiencyMeasureType,
    skos:Concept;
  rdfs:comment "Appointment of an energy manager to evaluate energy use and design programs to increase efficiency and reduce energy consumption";
  skos:broader bigg:ManagementMeasure .

bigg:ManagementMeasure.EnergyManagementExternalization a bigg:EnergyEfficiencyMeasureType,
    skos:Concept;
  rdfs:comment "Externalization of the energy management service (eg. By contracting ESCOs)";
  skos:broader bigg:ManagementMeasure .

bigg:ManagementMeasure.OtherManagementMeasure a bigg:EnergyEfficiencyMeasureType,
    skos:Concept;
  rdfs:comment "Other management measure ";
  skos:broader bigg:ManagementMeasure .

bigg:RenewableGenerationMeasure a bigg:EnergyEfficiencyMeasureType, skos:Concept;
  rdfs:comment "Measure related to renewable energy generation" .

bigg:RenewableGenerationMeasure.SolarPhotovoltaicInstallation a bigg:EnergyEfficiencyMeasureType,
    skos:Concept;
  rdfs:comment "Installation or replacement of photovoltaic panels";
  skos:broader bigg:RenewableGenerationMeasure .

bigg:RenewableGenerationMeasure.SolarThermalForHeatingInstallation a bigg:EnergyEfficiencyMeasureType,
    skos:Concept;
  rdfs:comment "Installation or replacement of a solar thermal system for heating purposes";
  skos:broader bigg:RenewableGenerationMeasure .

bigg:RenewableGenerationMeasure.SolarThermalForCoolingInstallation a bigg:EnergyEfficiencyMeasureType,
    skos:Concept;
  rdfs:comment "Installation or replacement of a solar thermal system for combined heating and cooling purposes";
  skos:broader bigg:RenewableGenerationMeasure .

bigg:RenewableGenerationMeasure.SolarThermalForHeatingAndCoolingInstallation a bigg:EnergyEfficiencyMeasureType,
    skos:Concept;
  rdfs:comment "Installation or replacement of a solar thermal system for cooling purposes";
  skos:broader bigg:RenewableGenerationMeasure .

bigg:RenewableGenerationMeasure.SolarThermalForHotWaterInstallation a bigg:EnergyEfficiencyMeasureType,
    skos:Concept;
  rdfs:comment "Solar thermal installation or replacement";
  skos:broader bigg:RenewableGenerationMeasure .

bigg:RenewableGenerationMeasure.SolarThermalForHeatingAndHotWaterInstallation a bigg:EnergyEfficiencyMeasureType,
    skos:Concept;
  rdfs:comment "Installation or replacement of a solar thermal system for combined space and water heating";
  skos:broader bigg:RenewableGenerationMeasure .

bigg:RenewableGenerationMeasure.OtherRenewableGenerationMeasure a bigg:EnergyEfficiencyMeasureType,
    skos:Concept;
  rdfs:comment "Other measure related to renewable energy generation";
  skos:broader bigg:RenewableGenerationMeasure .

bigg:TotalEnergySaving a bigg:EnergySavingType, skos:Concept;
  rdfs:comment "Total annual final energy savings (considering all billed energy sources) in the reference period, kWh/year" .

bigg:GridElectricitySaving a bigg:EnergySavingType, skos:Concept;
  rdfs:comment "Annual energy savings over purchased grid electricity, kWh/year" .

bigg:GasSaving a bigg:EnergySavingType, skos:Concept;
  rdfs:comment "Annual energy savings over purchased gas, kWh/year" .

bigg:OilSaving a bigg:EnergySavingType, skos:Concept;
  rdfs:comment "Annual energy savings over purchased oil, kWh/year" .

bigg:CoalSaving a bigg:EnergySavingType, skos:Concept;
  rdfs:comment "Annual energy savings over purchased coal, kWh/year" .

bigg:DistrictHeatingSaving a bigg:EnergySavingType, skos:Concept;
  rdfs:comment "Annual energy savings over purchased district heating, kWh/year" .

bigg:DistrictCoolingSaving a bigg:EnergySavingType, skos:Concept;
  rdfs:comment "Annual energy savings over purchased district cooling, kWh/year" .

bigg:CHPSaving a bigg:EnergySavingType, skos:Concept;
  rdfs:comment "Annual energy savings over Combined Heat and Power (CHP), kWh/year" .

bigg:BiomassSaving a bigg:EnergySavingType, skos:Concept;
  rdfs:comment "Annual energy savings over purchased biomass, kWh/year" .

bigg:BiofuelsSaving a bigg:EnergySavingType, skos:Concept;
  rdfs:comment "Annual energy savings over purchased biofuels, kWh/year" .

bigg:RenewableElectricitySaving a bigg:EnergySavingType, skos:Concept;
  rdfs:comment "Annual energy savings over produced elctrcity from renewable sources, kWh/year" .

bigg:RenewableHeatSaving a bigg:EnergySavingType, skos:Concept;
  rdfs:comment "Annual energy savings over produced heat from renewable sources, kWh/year" .

bigg:TotalAdjustedEnergySaving a bigg:EnergySavingType, skos:Concept;
  rdfs:comment "Total annual final energy savings (considering all billed energy sources) adjusted for weather/season/production, kWh/year" .

bigg:AdjustedGridElectricitySaving a bigg:EnergySavingType, skos:Concept;
  rdfs:comment "Annual energy savings over purchased grid electricity adjusted for weather/season/production, kWh/year" .

bigg:AdjustedGasSaving a bigg:EnergySavingType, skos:Concept;
  rdfs:comment "Annual energy savings over purchased gas adjusted for weather/season/production, kWh/year" .

bigg:AdjustedOilSaving a bigg:EnergySavingType, skos:Concept;
  rdfs:comment "Annual energy savings over purchased oil adjusted for weather/season/production, kWh/year" .

bigg:AdjustedCoalSaving a bigg:EnergySavingType, skos:Concept;
  rdfs:comment "Annual energy savings over purchased coal adjusted for weather/season/production, kWh/year" .

bigg:AdjustedDistrictHeatingSaving a bigg:EnergySavingType, skos:Concept;
  rdfs:comment "Annual energy savings over purchased district heating adjusted for weather/season/production, kWh/year" .

bigg:AdjustedDistrictCoolingSaving a bigg:EnergySavingType, skos:Concept;
  rdfs:comment "Annual energy savings over purchased district cooling adjusted for weather/season/production, kWh/year" .

bigg:AdjustedCHPSaving a bigg:EnergySavingType, skos:Concept;
  rdfs:comment "Annual energy savings over Combined Heat and Power (CHP) adjusted for weather/season/production, kWh/year" .

bigg:AdjustedBiomassSaving a bigg:EnergySavingType, skos:Concept;
  rdfs:comment "Annual energy savings over purchased biomass adjusted for weather/season/production, kWh/year" .

bigg:AdjustedBiofuelsSaving a bigg:EnergySavingType, skos:Concept;
  rdfs:comment "Annual energy savings over purchased biofuels adjusted for weather/season/production, kWh/year" .

bigg:AdjustedRenewableElectricitySaving a bigg:EnergySavingType, skos:Concept;
  rdfs:comment "Annual energy savings over produced elctrcity from renewable sources adjusted for weather/season/production, kWh/year" .

bigg:AdjustedRenewableHeatSaving a bigg:EnergySavingType, skos:Concept;
  rdfs:comment "Annual energy savings over produced heat from renewable sources adjusted for weather/season/production, kWh/year" .

bigg:OtherSavings a bigg:EnergySavingType, skos:Concept;
  rdfs:comment "Annual energy savings on unknown or not listed sources, kWh/year" .

bigg:ThirdParty a bigg:EnergySavingVerificationSource, skos:Concept .

bigg:ESCO a bigg:EnergySavingVerificationSource, skos:Concept .

bigg:GRC_ZONE_A a bigg:AddressClimateZone, skos:Concept;
  rdfs:comment "Greece, zone A" .

bigg:GRC_ZONE_B a bigg:AddressClimateZone, skos:Concept;
  rdfs:comment "Greece, zone B" .

bigg:GRC_ZONE_C a bigg:AddressClimateZone, skos:Concept;
  rdfs:comment "Greece, zone C" .

bigg:GRC_ZONE_D a bigg:AddressClimateZone, skos:Concept;
  rdfs:comment "Greece, zone D" .

bigg:EnergyConsumptionOthers a bigg:MeasuredProperty, skos:Concept;
  rdfs:comment "Total energy consumption from other unspecified resources" .

bigg:EnergyConsumptionTotal a bigg:MeasuredProperty, skos:Concept;
  rdfs:comment "Total energy consumption" .

bigg:EnergyConsumptionGridElectricity a bigg:MeasuredProperty, skos:Concept;
  rdfs:comment "Total energy consumed from the electricity grid" .

bigg:EnergyConsumptionGas a bigg:MeasuredProperty, skos:Concept;
  rdfs:comment "Total energy consumed from gas resource" .

bigg:EnergyConsumptionOil a bigg:MeasuredProperty, skos:Concept;
  rdfs:comment "Total energy consumed from oil resource" .

bigg:EnergyConsumptionCoal a bigg:MeasuredProperty, skos:Concept;
  rdfs:comment "Total energy consumed from coal resource, including coal-based products" .

bigg:EnergyConsumptionDistrictHeating a bigg:MeasuredProperty, skos:Concept;
  rdfs:comment "Total energy consumed from district heating system" .

bigg:EnergyConsumptionDistrictCooling a bigg:MeasuredProperty, skos:Concept;
  rdfs:comment "Total energy consumed from district cooling system" .

bigg:EnergyConsumptionCHP a bigg:MeasuredProperty, skos:Concept;
  rdfs:comment "Total energy consumed from CHP" .

bigg:EnergyConsumptionBiomass a bigg:MeasuredProperty, skos:Concept;
  rdfs:comment "Total energy consumed from biomass resources" .

bigg:EnergyConsumptionBiofuels a bigg:MeasuredProperty, skos:Concept;
  rdfs:comment "Total energy consumed from biofuel resources" .

bigg:EnergyConsumptionRenewableElectricity a bigg:MeasuredProperty, skos:Concept;
  rdfs:comment "Total energy consumed from renewable electricity generation" .

bigg:EnergyConsumptionRenewableHeat a bigg:MeasuredProperty, skos:Concept;
  rdfs:comment "Total energy consumed from renewable heat generation" .

bigg:AdjustedEnergyConsumptionTotal a bigg:MeasuredProperty, skos:Concept;
  rdfs:comment "Adjusted total energy consumption" .

bigg:AdjustedEnergyConsumptionGridElectricity a bigg:MeasuredProperty, skos:Concept;
  rdfs:comment "Adjusted total energy consumed from the electricity grid" .

bigg:AdjustedEnergyConsumptionGas a bigg:MeasuredProperty, skos:Concept;
  rdfs:comment "Adjusted total energy consumed from gas resource" .

bigg:AdjustedEnergyConsumptionOil a bigg:MeasuredProperty, skos:Concept;
  rdfs:comment "Adjusted total energy consumed from oil resource" .

bigg:AdjustedEnergyConsumptionCoal a bigg:MeasuredProperty, skos:Concept;
  rdfs:comment "Adjusted total energy consumed from coal resource, including coal-based products" .

bigg:AdjustedEnergyConsumptionDistrictHeating a bigg:MeasuredProperty, skos:Concept;
  rdfs:comment "Adjusted total energy consumed from district heating system" .

bigg:AdjustedEnergyConsumptionDistrictCooling a bigg:MeasuredProperty, skos:Concept;
  rdfs:comment "Adjusted total energy consumed from district cooling system" .

bigg:AdjustedEnergyConsumptionCHP a bigg:MeasuredProperty, skos:Concept;
  rdfs:comment "Adjusted total energy consumed from CHP" .

bigg:AdjustedEnergyConsumptionBiomass a bigg:MeasuredProperty, skos:Concept;
  rdfs:comment "Adjusted total energy consumed from biomass resources" .

bigg:AdjustedEnergyConsumptionBiofuels a bigg:MeasuredProperty, skos:Concept;
  rdfs:comment "Adjusted total energy consumed from biofuel resources" .

bigg:AdjustedEnergyConsumptionRenewableElectricity a bigg:MeasuredProperty, skos:Concept;
  rdfs:comment "Adjusted total energy consumed from renewable electricity generation" .

bigg:AdjustedEnergyConsumptionRenewableHeat a bigg:MeasuredProperty, skos:Concept;
  rdfs:comment "Adjusted total energy consumed from renewable heat generation" .

bigg:EnergyConsumptionSpaceHeating a bigg:MeasuredProperty, skos:Concept;
  rdfs:comment "Total energy consumed for space heating end-use" .

bigg:EnergyConsumptionSpaceCooling a bigg:MeasuredProperty, skos:Concept;
  rdfs:comment "Total energy consumed for space cooling end-use" .

bigg:EnergyConsumptionWaterHeating a bigg:MeasuredProperty, skos:Concept;
  rdfs:comment "Total energy consumed for water heating end-use" .

bigg:EnergyConsumptionCombinedSpaceHeatingAndCooling a bigg:MeasuredProperty, skos:Concept;
  rdfs:comment "Total energy consumed for combined space heating and cooling end-use" .

bigg:EnergyConsumptionCombinedSpaceAndWaterHeating a bigg:MeasuredProperty, skos:Concept;
  rdfs:comment "Total energy consumed for combined space and water heating end-use" .

bigg:EnergyConsumptionVentilation a bigg:MeasuredProperty, skos:Concept;
  rdfs:comment "Total energy consumed for ventilation end-use" .

bigg:EnergyConsumptionRefrigeration a bigg:MeasuredProperty, skos:Concept;
  rdfs:comment "Total energy consumed for refrigeration (excluding space cooling) end-use" .

bigg:EnergyConsumptionLighting a bigg:MeasuredProperty, skos:Concept;
  rdfs:comment "Total energy consumed for lighting end-use" .

bigg:EnergyConsumptionAppliances a bigg:MeasuredProperty, skos:Concept;
  rdfs:comment "Total energy consumed for the use of appliances" .

bigg:AdjustedEnergyConsumptionSpaceHeating a bigg:MeasuredProperty, skos:Concept;
  rdfs:comment "Adjusted total energy consumed for space heating end-use" .

bigg:AdjustedEnergyConsumptionSpaceCooling a bigg:MeasuredProperty, skos:Concept;
  rdfs:comment "Adjusted total energy consumed for space cooling end-use" .

bigg:AdjustedEnergyConsumptionWaterHeating a bigg:MeasuredProperty, skos:Concept;
  rdfs:comment "Adjusted total energy consumed for water heating end-use" .

bigg:AdjustedEnergyConsumptionCombinedSpaceHeatingAndCooling a bigg:MeasuredProperty,
    skos:Concept;
  rdfs:comment "Adjusted total energy consumed for combined space heating and cooling end-use" .

bigg:AdjustedEnergyConsumptionCombinedSpaceAndWaterHeating a bigg:MeasuredProperty,
    skos:Concept;
  rdfs:comment "Adjusted total energy consumed for combined space and water heating end-use" .

bigg:AdjustedEnergyConsumptionVentilation a bigg:MeasuredProperty, skos:Concept;
  rdfs:comment "Adjusted total energy consumed for ventilation end-use" .

bigg:AdjustedEnergyConsumptionRefrigeration a bigg:MeasuredProperty, skos:Concept;
  rdfs:comment "Adjusted total energy consumed for refrigeration (excluding space cooling) end-use" .

bigg:AdjustedEnergyConsumptionLighting a bigg:MeasuredProperty, skos:Concept;
  rdfs:comment "Adjusted total energy consumed for lighting end-use" .

bigg:AdjustedEnergyConsumptionAppliances a bigg:MeasuredProperty, skos:Concept;
  rdfs:comment "Adjusted total energy consumed for the use of appliances" .

bigg:Humidity a bigg:MeasuredProperty, skos:Concept;
  rdfs:comment "The amount of water vapor in the air" .

bigg:Illuminance a bigg:MeasuredProperty, skos:Concept;
  rdfs:comment "The area density of the luminous flux incident at a point on a surface" .

bigg:Motion a bigg:MeasuredProperty, skos:Concept;
  rdfs:comment "The phenomenon for which an object changes its position over time" .

bigg:Occupancy a bigg:MeasuredProperty, skos:Concept;
  rdfs:comment "The action of occupying a place" .

bigg:Power a bigg:MeasuredProperty, skos:Concept;
  rdfs:comment "The amount of energy transferred or converted per unit time" .

bigg:StaticPressure a bigg:MeasuredProperty, skos:Concept;
  rdfs:comment "The perpendicular force per unit area" .

bigg:Price a bigg:MeasuredProperty, skos:Concept;
  rdfs:comment "The monetary value of a good, service or resource" .

bigg:Price.EnergyPriceTotal a bigg:MeasuredProperty, skos:Concept;
  rdfs:comment "Total energy price";
  skos:broader bigg:Price .

bigg:Price.EnergyPriceGridElectricity a bigg:MeasuredProperty, skos:Concept;
  rdfs:comment "Energy price for grid electricity";
  skos:broader bigg:Price .

bigg:Price.EnergyPriceGas a bigg:MeasuredProperty, skos:Concept;
  rdfs:comment "Energy price for gas";
  skos:broader bigg:Price .

bigg:Price.EnergyPriceOil a bigg:MeasuredProperty, skos:Concept;
  rdfs:comment "Energy price for oil";
  skos:broader bigg:Price .

bigg:Price.EnergyPriceCoal a bigg:MeasuredProperty, skos:Concept;
  rdfs:comment "Energy price for coal, including coal-based products";
  skos:broader bigg:Price .

bigg:Price.EnergyPriceDistrictHeating a bigg:MeasuredProperty, skos:Concept;
  rdfs:comment "Energy price for district heating";
  skos:broader bigg:Price .

bigg:Price.EnergyPriceDistrictCooling a bigg:MeasuredProperty, skos:Concept;
  rdfs:comment "Energy price for district cooling";
  skos:broader bigg:Price .

bigg:Price.EnergyPriceCHP a bigg:MeasuredProperty, skos:Concept;
  rdfs:comment "Energy price for CHP energy";
  skos:broader bigg:Price .

bigg:Price.EnergyPriceBiomass a bigg:MeasuredProperty, skos:Concept;
  rdfs:comment "Energy price for biomass";
  skos:broader bigg:Price .

bigg:Price.EnergyPriceBiofuels a bigg:MeasuredProperty, skos:Concept;
  rdfs:comment "Energy price for biofuels";
  skos:broader bigg:Price .

bigg:Price.EnergyPriceRenewableElectricity a bigg:MeasuredProperty, skos:Concept;
  rdfs:comment "Energy price for renewable-generated electricity";
  skos:broader bigg:Price .

bigg:Price.EnergyPriceRenewableHeat a bigg:MeasuredProperty, skos:Concept;
  rdfs:comment "Energy price for renewable-generated heat";
  skos:broader bigg:Price .

bigg:Smoke a bigg:MeasuredProperty, skos:Concept;
  rdfs:comment "The collection of airborne particulates and gases emitted by a material undergoing combustion or pyrolysis" .

bigg:Temperature a bigg:MeasuredProperty, skos:Concept;
  rdfs:comment "The expressions of the average kinetic energy of atoms and molecules in a system" .

bigg:Concentration a bigg:MeasuredProperty, skos:Concept;
  rdfs:comment "The quantity of solute present in a given quantity of solution" .

bigg:Sound a bigg:MeasuredProperty, skos:Concept;
  rdfs:comment "The mechanical disturbance from a state of equilibrium that propagates through an elastic material medium" .

bigg:Speed a bigg:MeasuredProperty, skos:Concept;
  rdfs:comment "The rate at which an object covers distance" .

bigg:Flow a bigg:MeasuredProperty, skos:Concept;
  rdfs:comment "The quantity of fluid (gas, liquid or vapour) that passes a point per unit of time" .

bigg:CoolingDegreeDays a bigg:MeasuredProperty, skos:Concept;
  rdfs:comment "The sum of the differences between daily average temperatures and the base temperature, calculated at the ASHRAE base temperature of 18°C (or 65°F)" .

bigg:HeatingDegreeDays a bigg:MeasuredProperty, skos:Concept;
  rdfs:comment "The sum of the differences between daily average temperatures and the base temperature, calculated at the ASHRAE base temperature of 10°C (50°F)" .

bigg:HumidityRatio a bigg:MeasuredProperty, skos:Concept;
  rdfs:comment "The ratio between the actual mass of water vapor present in moist air - to the mass of the dry air" .

bigg:RelativeHumidity a bigg:MeasuredProperty, skos:Concept;
  rdfs:comment "The amount of water vapour present in air expressed as a percentage of the amount needed for saturation at the same temperature" .

bigg:DiffuseHorizontalRadiation a bigg:MeasuredProperty, skos:Concept;
  rdfs:comment "The radiation component that strikes a horizontal plane from the sky" .

bigg:DirectNormalRadiation a bigg:MeasuredProperty, skos:Concept;
  rdfs:comment "The amount of solar radiation from the direction of the sun" .

bigg:DryBulbTemperature a bigg:MeasuredProperty, skos:Concept;
  rdfs:comment "The air temperature measured by a dry temperature sensor or thermometer" .

bigg:WetBulbTemperature a bigg:MeasuredProperty, skos:Concept;
  rdfs:comment "The temperature Indicated by a psychrometer when the bulb of one thermometer is covered with a water-saturated wick over which air is caused to flow at approximately 4.5 m/s (900 ft/min) to reach an equilibrium temperature of water evaporating into air, when the heat of vaporization is supplied by the sensible heat of the air" .

bigg:WindSpeed a bigg:MeasuredProperty, skos:Concept;
  rdfs:comment "The speed of wind for the site at a height of 10 meter" .

bigg:BoilerModulationLevel a bigg:MeasuredProperty, skos:Concept;
  rdfs:comment "Boiler modulation level" .

bigg:Naive a bigg:EstimationMethod, skos:Concept;
  bigg:considerEstimatedValues false .

bigg:Profiled a bigg:EstimationMethod, skos:Concept;
  bigg:considerEstimatedValues false .

bigg:Interpolated a bigg:EstimationMethod, skos:Concept ;
  bigg:considerEstimatedValues false .

bigg:TrustedModel a bigg:EstimationMethod, skos:Concept ;
  bigg:considerEstimatedValues true .

bigg:TrustedModel.RegressionModel a bigg:EstimationMethod, skos:Concept;
  skos:broader bigg:TrustedModel ;
  bigg:considerEstimatedValues true .

bigg:TrustedModel.ClassificationModel a bigg:EstimationMethod, skos:Concept;
  skos:broader bigg:TrustedModel ;
  bigg:considerEstimatedValues true .

bigg:TrustedModel.Other a bigg:EstimationMethod, skos:Concept;
  skos:broader bigg:TrustedModel ;
  bigg:considerEstimatedValues true .

bigg:SafetyAndHealth a bigg:NonEnergyBenefitType, skos:Concept .

bigg:QualityImprovement a bigg:NonEnergyBenefitType, skos:Concept .

bigg:CostsSavings a bigg:NonEnergyBenefitType, skos:Concept .

bigg:TimeSavings a bigg:NonEnergyBenefitType, skos:Concept .

bigg:ValuePropositionImprovement a bigg:NonEnergyBenefitType, skos:Concept .

bigg:RisksMitigation a bigg:NonEnergyBenefitType, skos:Concept .

bigg:CarbonEmissionsReduction a bigg:NonEnergyBenefitType, skos:Concept .

bigg:OtherEmissionsReduction a bigg:NonEnergyBenefitType, skos:Concept .

bigg:CorporateSocialResponsibility a bigg:NonEnergyBenefitType, skos:Concept .

bigg:EmployeeSatisfaction a bigg:NonEnergyBenefitType, skos:Concept .

bigg:MarketValueIncrease a bigg:NonEnergyBenefitType, skos:Concept .

bigg:ProductivityImprovement a bigg:NonEnergyBenefitType, skos:Concept .

bigg:MaintenanceReduction a bigg:NonEnergyBenefitType, skos:Concept .

bigg:CustomerBenefits a bigg:NonEnergyBenefitType, skos:Concept .

bigg:SiteValueEnhancement a bigg:NonEnergyBenefitType, skos:Concept .

bigg:ComfortImprovement a bigg:NonEnergyBenefitType, skos:Concept .

bigg:Compliance a bigg:NonEnergyBenefitType, skos:Concept .

bigg:NotMeasured a bigg:NonEnergyBenefitImpactEvaluation, skos:Concept .

bigg:Improved a bigg:NonEnergyBenefitImpactEvaluation, skos:Concept .

bigg:NoImpact a bigg:NonEnergyBenefitImpactEvaluation, skos:Concept .

bigg:Degraded a bigg:NonEnergyBenefitImpactEvaluation, skos:Concept .

bigg:Lighting a skos:Concept .

bigg:SpaceHeating a skos:Concept .

bigg:SpaceCooling a skos:Concept .

bigg:CombinedSpaceHeatingAndCooling a skos:Concept .

bigg:HotWater a skos:Concept .

bigg:CombinedSpaceAndWaterHeating a skos:Concept .

bigg:Ventilation a skos:Concept .

bigg:Electricity a skos:Concept .

bigg:Refrigeration a skos:Concept .

bigg:PublicBank a bigg:OrganizationType, skos:Concept;
  rdfs:comment "PublicBank" .

bigg:PrivateBank a bigg:OrganizationType, skos:Concept;
  rdfs:comment "PrivateBank" .

bigg:IFI a bigg:OrganizationType, skos:Concept;
  rdfs:comment "IFI" .

bigg:ESCO a bigg:OrganizationType, skos:Concept;
  rdfs:comment "ESCO" .

bigg:SchemeManager a bigg:OrganizationType, skos:Concept;
  rdfs:comment "SchemeManager" .

bigg:Supplier a bigg:OrganizationType, skos:Concept;
  rdfs:comment "Supplier" .

bigg:HostInvestor a bigg:OrganizationType, skos:Concept;
  rdfs:comment "HostInvestor" .

bigg:AfterEnergyAudit a bigg:ProjectMotivation, skos:Concept;
  rdfs:comment "The project followed a mandatory energy audit" .

bigg:PartOfImprovementWorks a bigg:ProjectMotivation, skos:Concept;
  rdfs:comment "The project is part of larger modernization or improvement work" .

bigg:ToImproveProductivity a bigg:ProjectMotivation, skos:Concept;
  rdfs:comment "The project aimed at improving productivity" .

bigg:ForCostSavings a bigg:ProjectMotivation, skos:Concept;
  rdfs:comment "The project aimed at producing economic savings" .

bigg:ForEnvironmentalPolicy a bigg:ProjectMotivation, skos:Concept;
  rdfs:comment "The project aimed at complying with environmental policy requirements " .

bigg:ForLegalRequirements a bigg:ProjectMotivation, skos:Concept;
  rdfs:comment "The project aimed at complying with other legal requirements " .

bigg:ToBenefitFromFinancialSupport a bigg:ProjectMotivation, skos:Concept;
  rdfs:comment "The project aimed at benefitting from grants or financial support" .

bigg:MultiLevelState a bigg:StateType, skos:Concept;
  rdfs:comment "The state type of a device that can be set to multiple states" .

bigg:OnOffState a bigg:StateType, skos:Concept;
  rdfs:comment "The state type of a device that can be either on or off" .

bigg:OpenCloseState a bigg:StateType, skos:Concept;
  rdfs:comment "The state type of a device that can be either open or closed" .

bigg:StartStopState a bigg:StateType, skos:Concept;
  rdfs:comment "The state type of a device that can be started and stopped" .

bigg:LightingSystem a bigg:SystemType, skos:Concept;
  rdfs:comment "System of the building that fullfils a lighting function" .

bigg:HVACandHotWaterSystem a bigg:SystemType, skos:Concept;
  rdfs:comment "System of the building that fullfils an HVAC and/or water heating function" .

bigg:HVACandHotWaterSystem.HeatingSystem a bigg:SystemType, skos:Concept;
  rdfs:comment "System of the building that fullfils only a space heating function";
  skos:broader bigg:HVACandHotWaterSystem .

bigg:HVACandHotWaterSystem.CombinedHeatingCoolingSystem a bigg:SystemType, skos:Concept;
  rdfs:comment "System of the building that fullfils both a space heating and cooling function";
  skos:broader bigg:HVACandHotWaterSystem .

bigg:HVACandHotWaterSystem.CoolingSystem a bigg:SystemType, skos:Concept;
  rdfs:comment "System of the building that fullfils only a cooling function";
  skos:broader bigg:HVACandHotWaterSystem .

bigg:HVACandHotWaterSystem.HotWaterSystem a bigg:SystemType, skos:Concept;
  rdfs:comment "System of the building that fullfils only a water heating function";
  skos:broader bigg:HVACandHotWaterSystem .

bigg:HVACandHotWaterSystem.CombinedHeatingHotWaterSystem a bigg:SystemType, skos:Concept;
  rdfs:comment "System of the building that fullfils both a space and water heatingfunction";
  skos:broader bigg:HVACandHotWaterSystem .

bigg:HVACandHotWaterSystem.MechanicalVentilationSystem a bigg:SystemType, skos:Concept;
  rdfs:comment "System of the building that fullfils a mechanical ventilation function";
  skos:broader bigg:HVACandHotWaterSystem .

bigg:BuildingFabricSystem a bigg:SystemType, skos:Concept;
  rdfs:comment "System of the building that constitutes (part of) the building fabric" .

bigg:ElectricPowerSystem a bigg:SystemType, skos:Concept;
  rdfs:comment "System of the building  that fullfils an electric power-related function in the building" .

bigg:RefrigerationSystem a bigg:SystemType, skos:Concept;
  rdfs:comment "System of the building that fullfils a refrigeration function (space cooling is excluded)" .

bigg:RenewableGenerationSystem a bigg:SystemType, skos:Concept;
  rdfs:comment "System of the building that fullfils a renewable energy generation function" .

bigg:RenewableGenerationSystem.SolarPhotovoltaicSystem a bigg:SystemType, skos:Concept;
  rdfs:comment "Photovoltaic (PV) systems that derives energy from incoming solar radiation ";
  skos:broader bigg:RenewableGenerationSystem .

bigg:RenewableGenerationSystem.SolarThermalSystem a bigg:SystemType, skos:Concept;
  rdfs:comment "System that heats air or water using solar collectors";
  skos:broader bigg:RenewableGenerationSystem .

bigg:RenewableGenerationSystem.OtherRenewableGenerationSystem a bigg:SystemType, skos:Concept;
  rdfs:comment "Other system that fullfils a renewable energy generation function";
  skos:broader bigg:RenewableGenerationSystem .

bigg:OtherSystem a bigg:SystemType, skos:Concept;
  rdfs:comment "Other system" .

bigg:Electricity a bigg:UtilityType, skos:Concept .

bigg:Gas a bigg:UtilityType, skos:Concept .

bigg:Water a bigg:UtilityType, skos:Concept .

bigg:Construction a bigg:ZoneType, skos:Concept;
  rdfs:comment "The zone is used to represent a construction zone for the production process." .

bigg:Firesafety a bigg:ZoneType, skos:Concept;
  rdfs:comment "The zone is used to represent a fire safety zone, or fire compartment." .

bigg:Lighting a bigg:ZoneType, skos:Concept;
  rdfs:comment "The zone is used to represent a lighting zone; a daylight zone, or an artificial lighting zone." .

bigg:Occupancy a bigg:ZoneType, skos:Concept;
  rdfs:comment "The zone is used to represent a zone of particular occupancy." .

bigg:Security a bigg:ZoneType, skos:Concept;
  rdfs:comment "The zone is used to represent a zone for security planning and maintenance work." .

bigg:Thermal a bigg:ZoneType, skos:Concept;
  rdfs:comment "The zone is used to represent a thermal zone." .

bigg:Transport a bigg:ZoneType, skos:Concept .

bigg:Ventilation a bigg:ZoneType, skos:Concept;
  rdfs:comment "The zone is used to represent a ventilation zone." .
